Set_Graphs/Graph_Algorithms/DFS_old.thy
@@ -33,7 +33,7 @@ locale DFS =
 
 for lookup :: "'adjmapmap\<Rightarrow> 'v \<Rightarrow> 'vset option" +
 
-fixes G::"'adjmapmap" and s::"'v" and P_T::"'v \<Rightarrow> bool"(*
+fixes G::"'adjmapmap" and s::"'v" and t::"'v" (*
 fixes T_diff::"'vset \<Rightarrow> 'vset \<Rightarrow> nat"
 and T_sel::"'vset \<Rightarrow> nat" and T_insert::"'v \<Rightarrow> 'vset \<Rightarrow> nat"
 and T_lookup::"'adjmapmap\<Rightarrow> 'v \<Rightarrow> nat" and T_G::nat and T_vset_empty::nat*)
@@ -41,7 +41,7 @@ and T_lookup::"'adjmapmap\<Rightarrow> 'v \<Rightarrow> nat" and T_G::nat and T_
 begin
 
 definition "DFS_axioms = ( Graph.graph_inv G \<and> Graph.finite_graph G \<and> Graph.finite_vsets
-                    \<and> s = s \<and> isin = isin \<and> \<emptyset>\<^sub>N = \<emptyset>\<^sub>N)"
+                         \<and> s \<in> dVs (Graph.digraph_abs G))"
 
 abbreviation "neighbourhood' v == Graph.neighbourhood G v"
 
@@ -52,7 +52,7 @@ subsection \<open>Using the function package to model while-loops\<close>
 function (domintros) DFS::"('v, 'vset) DFS_state \<Rightarrow> ('v, 'vset) DFS_state" where
   "DFS dfs_state = 
      (case (stack dfs_state) of (v # stack_tl) \<Rightarrow>
-       (if P_T v then 
+       (if v = t then 
           (dfs_state \<lparr>return := Reachable\<rparr>)
         else ((if (\<N>\<^sub>G v -\<^sub>G (seen dfs_state)) \<noteq> \<emptyset>\<^sub>N then
                   let u = (sel ((\<N>\<^sub>G v) -\<^sub>G (seen dfs_state)));
@@ -74,7 +74,7 @@ definition "initial_state = \<lparr>stack = [s], seen = insert s \<emptyset>\<^s
 
 definition "DFS_call_1_conds dfs_state = 
     (case stack dfs_state of (v # stack_tl) \<Rightarrow>
-       (if P_T v then 
+       (if v = t then 
           False
         else ((if ((\<N>\<^sub>G v) -\<^sub>G (seen dfs_state)) \<noteq> (\<emptyset>\<^sub>N) then
                   True
@@ -87,7 +87,7 @@ definition "DFS_call_1_conds dfs_state =
 lemma DFS_call_1_conds[call_cond_elims]: 
   "DFS_call_1_conds dfs_state \<Longrightarrow> 
    \<lbrakk>\<lbrakk>\<exists>v stack_tl. stack dfs_state = v # stack_tl;
-    \<not> P_T (hd (stack dfs_state));
+    hd (stack dfs_state) \<noteq> t;
     (\<N>\<^sub>G (hd (stack dfs_state))) -\<^sub>G (seen dfs_state) \<noteq> (\<emptyset>\<^sub>N)\<rbrakk> \<Longrightarrow> P\<rbrakk> \<Longrightarrow> 
    P"
   by(auto simp: DFS_call_1_conds_def split: list.splits option.splits if_splits)
@@ -104,7 +104,7 @@ definition "DFS_upd1 dfs_state = (
 
 definition "DFS_call_2_conds dfs_state =
 (case stack dfs_state of (v # stack_tl) \<Rightarrow>
-       (if P_T v then 
+       (if v = t then 
           False
         else (
                 (if ((\<N>\<^sub>G v) -\<^sub>G (seen dfs_state)) \<noteq> (\<emptyset>\<^sub>N) then
@@ -118,7 +118,7 @@ definition "DFS_call_2_conds dfs_state =
 lemma DFS_call_2_conds[call_cond_elims]: 
   "DFS_call_2_conds dfs_state \<Longrightarrow> 
    \<lbrakk>\<lbrakk>\<exists>v stack_tl. stack dfs_state = v # stack_tl;
-    \<not> P_T (hd (stack dfs_state));
+    hd (stack dfs_state) \<noteq> t;
     (\<N>\<^sub>G (hd (stack dfs_state))) -\<^sub>G (seen dfs_state) = (\<emptyset>\<^sub>N)\<rbrakk> \<Longrightarrow> P\<rbrakk> \<Longrightarrow> 
    P"
   by(auto simp: DFS_call_2_conds_def split: list.splits option.splits if_splits)
@@ -129,7 +129,7 @@ definition "DFS_upd2 dfs_state =
 
 definition "DFS_ret_1_conds dfs_state =
    (case stack dfs_state of (v # stack_tl) \<Rightarrow>
-       (if P_T v then 
+       (if v = t then 
           False
         else (
                 (if ((\<N>\<^sub>G v) -\<^sub>G (seen dfs_state)) \<noteq> \<emptyset>\<^sub>N then
@@ -154,7 +154,7 @@ definition "DFS_ret1 dfs_state = (dfs_state \<lparr>return := NotReachable\<rpar
 
 definition "DFS_ret_2_conds dfs_state =
    (case stack dfs_state of (v # stack_tl) \<Rightarrow>
-       (if P_T  v then 
+       (if v = t then 
           True
         else (
                 (if (\<N>\<^sub>G v -\<^sub>G (seen dfs_state)) \<noteq> \<emptyset>\<^sub>N then
@@ -169,12 +169,12 @@ definition "DFS_ret_2_conds dfs_state =
 lemma DFS_ret_2_conds[call_cond_elims]:
   "DFS_ret_2_conds dfs_state \<Longrightarrow> 
    \<lbrakk>\<And>v stack_tl. \<lbrakk>stack dfs_state = v # stack_tl;
-    P_T (hd (stack dfs_state))\<rbrakk> \<Longrightarrow> P\<rbrakk> \<Longrightarrow> 
+    (hd (stack dfs_state)) = t\<rbrakk> \<Longrightarrow> P\<rbrakk> \<Longrightarrow> 
    P"
   by(auto simp: DFS_ret_2_conds_def split: list.splits option.splits if_splits)
 
 lemma DFS_ret_2_condsI[call_cond_intros]:
-  "\<And>v stack_tl. \<lbrakk>stack dfs_state = v # stack_tl; P_T (hd (stack dfs_state))\<rbrakk> \<Longrightarrow> DFS_ret_2_conds dfs_state"
+  "\<And>v stack_tl. \<lbrakk>stack dfs_state = v # stack_tl; (hd (stack dfs_state)) = t\<rbrakk> \<Longrightarrow> DFS_ret_2_conds dfs_state"
   by(auto simp: DFS_ret_2_conds_def split: list.splits option.splits if_splits)
 
 definition "DFS_ret2 dfs_state = (dfs_state \<lparr>return := Reachable\<rparr>)"
@@ -237,21 +237,19 @@ qed
 
 definition "invar_1 dfs_state = vset_inv (seen dfs_state)"
 
-definition "invar_2 dfs_state = (Vwalk.vwalk (Graph.digraph_abs G) (rev (stack dfs_state))
-                                \<or> stack dfs_state = [s])"
+definition "invar_2 dfs_state = (Vwalk.vwalk (Graph.digraph_abs G) (rev (stack dfs_state)))"
 
 definition "invar_seen_stack dfs_state \<longleftrightarrow> 
     distinct (stack dfs_state)
     \<and> set (stack dfs_state) \<subseteq> t_set (seen dfs_state)
-    \<and> t_set (seen dfs_state) \<subseteq> Set.insert s (dVs (Graph.digraph_abs G))"
+    \<and> t_set (seen dfs_state) \<subseteq> dVs (Graph.digraph_abs G)"
 
 definition "invar_s_in_stack dfs_state \<longleftrightarrow> 
   (stack (dfs_state) \<noteq> [] \<longrightarrow> last (stack dfs_state) = s)"
 
 definition "invar_visited_through_seen dfs_state = 
     (\<forall>v \<in> t_set (seen dfs_state).
-       (\<forall>p tt. Vwalk.vwalk_bet (Graph.digraph_abs G) v p tt \<and> P_T tt \<and> distinct p 
-\<longrightarrow> (set p \<inter> set (stack dfs_state) \<noteq> {})))"
+       (\<forall>p. Vwalk.vwalk_bet (Graph.digraph_abs G) v p t \<and> distinct p \<longrightarrow> (set p \<inter> set (stack dfs_state) \<noteq> {})))"
 
 definition "call_1_measure dfs_state = card (dVs (Graph.digraph_abs G) -  t_set (seen dfs_state))"
 
@@ -279,7 +277,7 @@ lemma graph_inv[simp,intro]:
   using DFS_axioms
   by (auto simp: DFS_axioms_def)
 
-lemma s_in_G[simp,intro]: "s \<in> Set.insert s (dVs (Graph.digraph_abs G))"
+lemma s_in_G[simp,intro]: "s \<in> dVs (Graph.digraph_abs G)"
   using DFS_axioms
   by (auto simp: DFS_axioms_def)
 
@@ -327,36 +325,29 @@ qed
 
 lemma invar_2_props[invar_props_elims]: 
   "invar_2 dfs_state \<Longrightarrow>
-     ((Vwalk.vwalk (Graph.digraph_abs G) (rev (stack dfs_state))) \<Longrightarrow> P) \<Longrightarrow>
-      ( (stack dfs_state) = [s] \<Longrightarrow> P)\<Longrightarrow> P"
+     ((Vwalk.vwalk (Graph.digraph_abs G) (rev (stack dfs_state))) \<Longrightarrow> P) \<Longrightarrow> P"
   by (auto simp: invar_2_def)
 
-lemma invar_2_intro[invar_props_intros]: 
-"Vwalk.vwalk (Graph.digraph_abs G) (rev (stack dfs_state)) \<Longrightarrow> invar_2 dfs_state"
+lemma invar_2_intro[invar_props_intros]: "Vwalk.vwalk (Graph.digraph_abs G) (rev (stack dfs_state)) \<Longrightarrow> invar_2 dfs_state"
   by (auto simp: invar_2_def)
 
-lemma invar_2_inter_alternative: 
-"(stack dfs_state) = [s] \<Longrightarrow> invar_2 dfs_state"
-  by (auto simp: invar_2_def)
 
 lemma invar_2_holds_1[invar_holds_intros]:
   assumes "DFS_call_1_conds dfs_state" "invar_1 dfs_state" "invar_2 dfs_state"
   shows "invar_2 (DFS_upd1 dfs_state)"
     using assms graph_inv 
-    by (fastforce simp: Let_def DFS_upd1_def elim!: call_cond_elims elim!: invar_props_elims
+    by (force simp: Let_def DFS_upd1_def elim!: call_cond_elims elim!: invar_props_elims
                 intro!: Vwalk.vwalk_append2 neighbourhoodI invar_props_intros)
+
 
 lemma invar_2_holds_2[invar_holds_intros]: "\<lbrakk>DFS_call_2_conds dfs_state; invar_2 dfs_state\<rbrakk> \<Longrightarrow> invar_2 (DFS_upd2 dfs_state)"
   by (auto simp: DFS_upd2_def dest!: append_vwalk_pref elim!: invar_props_elims intro!: invar_props_intros elim: call_cond_elims)
 
-lemma invar_2_holds_4[invar_holds_intros]: "\<lbrakk>DFS_ret_1_conds dfs_state; invar_2 dfs_state\<rbrakk> 
-\<Longrightarrow> invar_2 (DFS_ret1 dfs_state)"
-  by(auto elim!: invar_props_elims intro: invar_props_intros derivative_intros
-invar_2_inter_alternative simp: DFS_ret1_def)
+lemma invar_2_holds_4[invar_holds_intros]: "\<lbrakk>DFS_ret_1_conds dfs_state; invar_2 dfs_state\<rbrakk> \<Longrightarrow> invar_2 (DFS_ret1 dfs_state)"
+  by (auto elim!: invar_props_elims intro: invar_props_intros derivative_intros simp: DFS_ret1_def)
 
 lemma invar_2_holds_5[invar_holds_intros]: "\<lbrakk>DFS_ret_2_conds dfs_state; invar_2 dfs_state\<rbrakk> \<Longrightarrow> invar_2 (DFS_ret2 dfs_state)"
-  by (auto elim!: invar_props_elims intro: invar_props_intros 
-invar_2_inter_alternative simp: DFS_ret2_def)
+  by (auto elim!: invar_props_elims intro: invar_props_intros simp: DFS_ret2_def)
 
 lemma invar_2_holds[invar_holds_intros]:
    assumes "DFS_dom dfs_state" "invar_1 dfs_state" "invar_2 dfs_state"
@@ -372,19 +363,17 @@ qed
 lemma invar_seen_stack_props[invar_props_elims]:
    "invar_seen_stack dfs_state \<Longrightarrow> 
      (\<lbrakk>distinct (stack dfs_state); set (stack dfs_state) \<subseteq> t_set (seen dfs_state);
-       t_set (seen dfs_state) \<subseteq> Set.insert s ( dVs (Graph.digraph_abs G))\<rbrakk> \<Longrightarrow> P) \<Longrightarrow> P "
+       t_set (seen dfs_state) \<subseteq> dVs (Graph.digraph_abs G)\<rbrakk> \<Longrightarrow> P) \<Longrightarrow> P "
   by (auto simp: invar_seen_stack_def)
 
 lemma invar_seen_stack_intro[invar_props_intros]:
-  "\<lbrakk>distinct (stack dfs_state); set (stack dfs_state) \<subseteq> t_set (seen dfs_state);
- t_set (seen dfs_state) \<subseteq> Set.insert s (dVs (Graph.digraph_abs G))\<rbrakk> \<Longrightarrow> invar_seen_stack dfs_state"
+  "\<lbrakk>distinct (stack dfs_state); set (stack dfs_state) \<subseteq> t_set (seen dfs_state); t_set (seen dfs_state) \<subseteq> dVs (Graph.digraph_abs G)\<rbrakk> \<Longrightarrow> invar_seen_stack dfs_state"
   by (auto simp: invar_seen_stack_def)
 
 lemma invar_seen_stack_holds_1[invar_holds_intros]:
-  "\<lbrakk>DFS_call_1_conds dfs_state; invar_1 dfs_state; invar_seen_stack dfs_state\<rbrakk>
- \<Longrightarrow> invar_seen_stack (DFS_upd1 dfs_state)"
-  by (auto simp: Let_def DFS_upd1_def dest!: append_vwalk_pref elim!: call_cond_elims
-            elim!: invar_props_elims intro!: invar_props_intros | force)+
+  "\<lbrakk>DFS_call_1_conds dfs_state; invar_1 dfs_state; invar_seen_stack dfs_state\<rbrakk> \<Longrightarrow> invar_seen_stack (DFS_upd1 dfs_state)"
+  by (force simp: Let_def DFS_upd1_def dest!: append_vwalk_pref elim!: call_cond_elims
+            elim!: invar_props_elims intro!: invar_props_intros)
 
 lemma invar_seen_stack_holds_2[invar_holds_intros]: 
   "\<lbrakk>DFS_call_2_conds dfs_state; invar_1 dfs_state; invar_seen_stack dfs_state\<rbrakk> \<Longrightarrow>
@@ -454,15 +443,15 @@ qed
 
 lemma invar_visited_through_seen_props[elim!]:
    "invar_visited_through_seen dfs_state \<Longrightarrow> 
-     (\<lbrakk>\<And>v p tt. \<lbrakk>v \<in> t_set (seen dfs_state);
-              (Vwalk.vwalk_bet (Graph.digraph_abs G) v p tt);  P_T tt; distinct p \<rbrakk> \<Longrightarrow>
+     (\<lbrakk>\<And>v p. \<lbrakk>v \<in> t_set (seen dfs_state);
+              (Vwalk.vwalk_bet (Graph.digraph_abs G) v p t); distinct p \<rbrakk> \<Longrightarrow>
               set p \<inter> set (stack dfs_state) \<noteq> {}\<rbrakk> \<Longrightarrow> P) \<Longrightarrow> P "
   by (auto simp: invar_visited_through_seen_def)
 
 
 lemma invar_visited_through_seen_intro[invar_props_intros]:
-  "\<lbrakk>\<And>v p tt. \<lbrakk>v \<in> t_set (seen dfs_state);
-           (Vwalk.vwalk_bet (Graph.digraph_abs G) v p tt);  P_T tt; distinct p\<rbrakk> \<Longrightarrow>
+  "\<lbrakk>\<And>v p. \<lbrakk>v \<in> t_set (seen dfs_state);
+           (Vwalk.vwalk_bet (Graph.digraph_abs G) v p t); distinct p\<rbrakk> \<Longrightarrow>
            set p \<inter> set (stack dfs_state) \<noteq> {}\<rbrakk> \<Longrightarrow> invar_visited_through_seen dfs_state"
   by (auto simp: invar_visited_through_seen_def)
 
@@ -479,7 +468,7 @@ lemma invar_visited_through_seen_holds_2[invar_holds_intros]:
   "\<lbrakk>DFS_call_2_conds dfs_state; invar_1 dfs_state; invar_seen_stack dfs_state;
     invar_visited_through_seen dfs_state\<rbrakk> \<Longrightarrow> invar_visited_through_seen (DFS_upd2 dfs_state)"
 proof(rule invar_props_intros, elim invar_visited_through_seen_props call_cond_elims exE,  goal_cases)
-  case (1 v1 p tt v2 stack_tl)
+  case (1 v1 p v2 stack_tl)
   text \<open>We know one thing: a path starting at @{term v1} and ending at @{term t} intersects with the
         old stack @{term "v2 # stack_tl"}.
         We have two cases:\<close>
@@ -516,6 +505,7 @@ proof(rule invar_props_intros, elim invar_visited_through_seen_props call_cond_e
     text \<open>
                 Since the invariant holds for the old state, then @{term "[v2] @ p2"}
                 intersects the old stack @{term "v2 # stack_tl"}.\<close>
+
     show ?thesis
     proof(cases "p2 = []")
       case True
@@ -525,8 +515,8 @@ proof(rule invar_props_intros, elim invar_visited_through_seen_props call_cond_e
                 Case a: @{term "p2 = []"} This cannot be the case, since it would imply that @{term "v2 = t"}, which 
                         violates the assumption of us being in this execution branch.\<close>
       thus ?thesis
-        using 1 using \<open>p = p1 @ [v2] @ p2\<close>  vwalk_bet_snoc 
-        by fastforce
+        using 1
+          by (auto simp: vwalk_bet_snoc)
     next
       case False
       text \<open>
@@ -537,14 +527,11 @@ proof(rule invar_props_intros, elim invar_visited_through_seen_props call_cond_e
                         cannot contain @{term v2}. This means that it intersects @{term stack_tl},
                         which implies that @{term p} with @{term stack_tl}. This finishes our proof.\<close>
       hence "hd p2 \<in> t_set (\<N>\<^sub>G v2)"
-        using \<open>vwalk_bet (Graph.digraph_abs G) v1 p tt\<close> 
+        using \<open>vwalk_bet (Graph.digraph_abs G) v1 p t\<close> 
         by (auto dest!: split_vwalk simp:  neq_Nil_conv)
       hence "hd p2 \<in> t_set (seen dfs_state)"
-        using 1(1-6,8-) 1(7)[OF _ 1(4,5,6)] invar_1_props[OF 1(1)]
-               Graph.neighbourhood_invars'[OF graph_inv(1)]
-               Graph.vset.set.set_empty  graph_inv(1)  set_ops.set_diff[of "\<N>\<^sub>G v2" "seen dfs_state"]
-        by auto
-        (*by (fas tforce elim!: invar_props_elims simp del: \<open>p = p1 @ [v2] @ p2\<close>)*)
+        using 1
+        by (fastforce elim!: invar_props_elims simp del: \<open>p = p1 @ [v2] @ p2\<close>)
       hence "set p2 \<inter> set (stack dfs_state) \<noteq> {}" 
         using 1 False 
         by (fastforce simp: DFS_upd2_def neq_Nil_conv dest!: split_vwalk)
@@ -640,7 +627,7 @@ qed
 
 lemma DFS_correct_ret_1:
   "\<lbrakk>invar_visited_through_seen dfs_state; DFS_ret_1_conds dfs_state; u \<in> t_set (seen dfs_state)\<rbrakk>
-         \<Longrightarrow> \<nexists>p t. distinct p \<and> vwalk_bet (Graph.digraph_abs G) u p t \<and> P_T t"
+         \<Longrightarrow> \<nexists>p. distinct p \<and> vwalk_bet (Graph.digraph_abs G) u p t"
   by (auto elim!: call_cond_elims invar_props_elims)
 
 lemma DFS_ret_2[ret_holds_intros]: "DFS_ret_2_conds (dfs_state) \<Longrightarrow> DFS_ret_2_conds (DFS_ret2 dfs_state)"
@@ -660,10 +647,8 @@ qed
 
 lemma DFS_correct_ret_2:
   "\<lbrakk>invar_2 dfs_state; DFS_ret_2_conds dfs_state\<rbrakk>
-         \<Longrightarrow> \<exists> t. (vwalk_bet (Graph.digraph_abs G) (last (stack dfs_state)) (rev (stack dfs_state)) t
-                  \<or> (stack dfs_state = [s] \<and> t= s)) \<and> P_T t"
-  by (auto elim!: call_cond_elims invar_props_elims simp: hd_rev vwalk_bet_def
-       intro: invar_2_inter_alternative)
+         \<Longrightarrow> vwalk_bet (Graph.digraph_abs G) (last (stack dfs_state)) (rev (stack dfs_state)) t"
+  by (auto elim!: call_cond_elims invar_props_elims simp: hd_rev vwalk_bet_def)
 
 subsection \<open>Termination\<close>
 
@@ -732,14 +717,14 @@ lemma initial_state_props[invar_holds_intros, termination_intros]:
   "invar_1 (initial_state)" "invar_2 (initial_state)" "invar_seen_stack (initial_state)"
   "invar_visited_through_seen (initial_state)" "invar_s_in_stack initial_state" 
   "DFS_dom initial_state"
-by (auto simp: initial_state_def
+  by (auto simp: initial_state_def
                  hd_of_vwalk_bet''
            elim: vwalk_betE
-           intro!: termination_intros invar_props_intros invar_2_inter_alternative)
+           intro!: termination_intros invar_props_intros)
 
 lemma DFS_correct_1:
   assumes "return (DFS initial_state) = NotReachable"
-  shows   "\<nexists>p t. distinct p \<and> (vwalk_bet (Graph.digraph_abs G) s p t ) \<and> P_T t"
+  shows   "\<nexists>p. distinct p \<and> vwalk_bet (Graph.digraph_abs G) s p t"
 proof-
   have "s \<in> t_set (seen (DFS initial_state))"
     by(auto intro!: invar_holds_intros ret_holds_intros state_rel_holds_intros
@@ -751,44 +736,23 @@ proof-
       (auto intro!: invar_holds_intros ret_holds_intros state_rel_holds_intros)
 qed
 
-lemma DFS_correct_1_s_is_t:
-  assumes "return (DFS initial_state) = NotReachable"
-  shows   "\<not> P_T s" 
-  apply(rule ccontr, simp)
-  using assms
-  apply(subst (asm) DFS_simps(4)[OF initial_state_props(6)])
-  by(auto simp add: DFS_ret_2_conds_def initial_state_def DFS_ret2_def)
-
 lemma DFS_correct_2:
   assumes  "return (DFS initial_state) = Reachable"
-  shows "\<exists> t. ((vwalk_bet (Graph.digraph_abs G) s (rev (stack (DFS initial_state))) t
-        \<or> (stack (DFS initial_state) = [s] \<and> s= t)) \<and> P_T t)"
+  shows "vwalk_bet (Graph.digraph_abs G) s (rev (stack (DFS initial_state))) t"
 proof-
-  have "\<exists> t. (vwalk_bet
+  have "vwalk_bet
               (Graph.digraph_abs G)
               (last (stack (DFS initial_state)))
-              (rev (stack (DFS initial_state))) t 
-       \<or> (stack (DFS initial_state) = [s] \<and> s = t)) \<and> P_T t"
-    using assms DFS_correct_ret_2 initial_state_props(1) initial_state_props(2) 
-          initial_state_props(6) invar_2_holds  ret2_holds 
-    by (cases "P_T s")fastforce+
-   (* apply(aut o intro!: invar_holds_intros ret_holds_intros state_rel_holds_intros
-                     invar_2_inter_alternative
-                       DFS_correct_ret_2[where dfs_state = "DFS initial_state"])*)
+              (rev (stack (DFS initial_state))) t"
+    using assms
+    by(auto intro!: invar_holds_intros ret_holds_intros state_rel_holds_intros
+                       DFS_correct_ret_2[where dfs_state = "DFS initial_state"])
   moreover hence "(last (stack (DFS initial_state))) = s"
     by(fastforce intro!: invar_holds_intros
                  intro: invar_s_in_stack_props[where dfs_state = "DFS initial_state"])+
   ultimately show ?thesis
     by auto
 qed
-
-lemma DFS_correct_2_s_is_t:
-  assumes  "P_T s"
-  shows "return (DFS initial_state) = Reachable"
-  and  "stack (DFS initial_state) = [s]"
-  using DFS_correct_1_s_is_t assms return.exhaust  DFS.psimps assms initial_state_def 
-        initial_state_props(6) by force+
-
 end
 end
 
@@ -798,7 +762,7 @@ begin
 partial_function (tailrec) DFS_impl::"('v, 'vset) DFS_state \<Rightarrow> ('v, 'vset) DFS_state" where
   "DFS_impl dfs_state = 
      (case (stack dfs_state) of (v # stack_tl) \<Rightarrow>
-       (if P_T v then 
+       (if v = t then 
           (dfs_state \<lparr>return := Reachable\<rparr>)
         else ((if (\<N>\<^sub>G v -\<^sub>G (seen dfs_state)) \<noteq> \<emptyset>\<^sub>N then
                   let u = (sel ((\<N>\<^sub>G v) -\<^sub>G (seen dfs_state)));
