Spanning_Trees/Kruskal_Greedy.thy
@@ -1,155 +1,19 @@
 theory Kruskal_Greedy
-  imports Matroids_Greedy.Best_In_Greedy Spanning_Trees Graph_Algorithms.DFS_Cycles_Aux
-    Graph_Algorithms.DFS_Cycles Insertion_Sort_Desc Graphs_Matroids_Encoding
-    "HOL-Data_Structures.Set2_Join_RBT" "HOL-Data_Structures.RBT_Map" "HOL-Library.Product_Lexorder"
+  imports Matroids_Greedy.Best_In_Greedy Spanning_Trees Encoding
+         Graph_Algorithms.DFS_Example Insertion_Sort_Desc "HOL-Library.Product_Lexorder"
 begin
 
-
-subsection \<open>Instantiations for Kruskal's algorithm\<close>
-
-abbreviation "rbt_inv == ( \<lambda>t. (invc t \<and> invh t) \<and> Tree2.bst t)"
-
-fun rbt_sel where
-  "rbt_sel Leaf = undefined"
-| "rbt_sel (Node _ (a,_) _) = a"
-
-lemma rbt_sel_correct:
-  "t \<noteq> empty \<Longrightarrow> rbt_sel t \<in> (set o inorder) t"
-  by (induction t) (auto simp: empty_def)
-
-interpretation Set_Choose_RBT: Set_Choose
-  where empty = "\<langle>\<rangle>" and insert = insert_rbt and delete = delete_rbt and
-    isin = isin and t_set = "Tree2.set_tree" and invar = "rbt_inv::(('v::linorder) rbt \<Rightarrow> bool)" and
-    sel = rbt_sel
-  apply(simp add: Set_Choose_def)
-  apply(intro conjI)
-  subgoal
-    using RBT.Set_axioms[unfolded] by(auto simp add: S.set_def S.invar_def)
-  subgoal apply unfold_locales subgoal for s by (cases s) (auto dest!: rbt_sel_correct)
-  done
-  done
-
-
-interpretation Pair_Graph_U_RBT: Pair_Graph_U_Specs
-  where empty = RBT_Set.empty and update = update and delete = RBT_Map.delete and
+hide_const RBT_Set.insert
+global_interpretation Pair_Graph_U_RBT: Pair_Graph_U_Specs
+  where empty = empty and update = update and delete = delete and
     lookup = lookup and adjmap_inv = "M.invar" and vset_empty = "\<langle>\<rangle>" and
-    insert = insert_rbt and vset_delete = delete_rbt and vset_inv = "rbt_inv::(('v::linorder) rbt \<Rightarrow> bool)" and
-    isin = isin and t_set = "Tree2.set_tree" and sel = rbt_sel
-  apply(simp add: Pair_Graph_U_Specs_def Pair_Graph_Specs_def)
-  using M.Map_axioms Set_Choose_RBT.Set_Choose_axioms by simp
+    insert = vset_insert and vset_delete = vset_delete and vset_inv = "vset_inv::(('v::linorder) rbt \<Rightarrow> bool)" and
+    isin = isin and t_set = "Tree2.set_tree" and sel = sel
+  defines add_edge =Pair_Graph_U_RBT.add_edge
+    and  delete_edge =Pair_Graph_U_RBT.delete_edge
+  by(simp add: Pair_Graph_U_Specs_def Pair_Graph_Specs_def M.Map_axioms S_C.Set_Choose_axioms)
 
-interpretation DFS_Aux_Interp: DFS_Aux
-  where empty = RBT_Set.empty and update = update and delete = RBT_Map.delete and
-    lookup = lookup and adjmap_inv = "M.invar" and vset_empty = "\<langle>\<rangle>" and
-    insert = insert_rbt and vset_delete = delete_rbt and vset_inv = "rbt_inv::(('v::linorder) rbt \<Rightarrow> bool)" and
-    isin = isin and t_set = "Tree2.set_tree" and union = "RBT.union" and inter = "RBT.inter" and 
-    diff = "RBT.diff" and sel = rbt_sel for G and s
-  apply(simp add: DFS_Aux_def)
-  using Pair_Graph_U_RBT.Pair_Graph_Specs_axioms RBT.Set2_axioms by auto
-
-abbreviation "DFS_Aux' G s \<equiv> DFS_Aux_Interp.DFS_Aux G (DFS_Aux_Interp.initial_state s)"
-
-interpretation DFS_Cycles_Interp: DFS_Cycles
-  where empty = RBT_Set.empty and update = update and delete = RBT_Map.delete and
-    lookup = lookup and adjmap_inv = "M.invar" and vset_empty = "\<langle>\<rangle>" and
-    insert = insert_rbt and vset_delete = delete_rbt and vset_inv = "rbt_inv::(('v::linorder) rbt \<Rightarrow> bool)" and
-    isin = isin and t_set = "Tree2.set_tree" and union = "RBT.union" and inter = "RBT.inter" and 
-    diff = "RBT.diff" and sel = rbt_sel and seen_aux = "DFS_Aux_state.seen" and cycle_aux = "DFS_Aux_state.cycle" and
-    dfs_aux = "DFS_Aux' G" for G and V
-  apply(simp add: DFS_Cycles_def)
-  using Pair_Graph_U_RBT.Pair_Graph_Specs_axioms RBT.Set2_axioms by auto
-
-lemma DFS_Aux_correct_1_inst:
-  assumes "DFS_Cycles.DFS_Cycles_axioms isin Tree2.set_tree M.invar \<langle>\<rangle> rbt_inv lookup G V"
-    "s \<in> dVs (Pair_Graph_U_RBT.digraph_abs G)"
-  shows "DFS_Aux_state.cycle (DFS_Aux' G s) \<Longrightarrow> \<exists>c. cycle' (Pair_Graph_U_RBT.digraph_abs G) c"
-  using assms[simplified DFS_Cycles_Interp.DFS_Cycles_axioms_def[of "G" "V"]]
-    DFS_Aux_Interp.DFS_Aux_correct_1[unfolded DFS_Aux_Interp.DFS_Aux_axioms_def]
-  by blast
-
-lemma DFS_Aux_correct_2_inst:
-  assumes "DFS_Cycles.DFS_Cycles_axioms isin Tree2.set_tree M.invar \<langle>\<rangle> rbt_inv lookup G V"
-    "s \<in> dVs (Pair_Graph_U_RBT.digraph_abs G)"
-  shows "\<not>DFS_Aux_state.cycle (DFS_Aux' G s) \<Longrightarrow>
-    \<nexists>c. cycle' (Pair_Graph_U_RBT.digraph_abs G \<downharpoonright> Tree2.set_tree (DFS_Aux_state.seen (DFS_Aux' G s))) c"
-  using assms[simplified DFS_Cycles_Interp.DFS_Cycles_axioms_def[of "G" "V"]]
-    DFS_Aux_Interp.DFS_Aux_correct_2[unfolded DFS_Aux_Interp.DFS_Aux_axioms_def]
-  by blast
-
-lemma DFS_Aux_correct_3_inst:
-  assumes "DFS_Cycles.DFS_Cycles_axioms isin Tree2.set_tree M.invar \<langle>\<rangle> rbt_inv lookup G V"
-    "s \<in> dVs (Pair_Graph_U_RBT.digraph_abs G)"
-  shows "\<not>DFS_Aux_state.cycle (DFS_Aux' G s) \<Longrightarrow> v \<in> Tree2.set_tree (DFS_Aux_state.seen (DFS_Aux' G s)) \<Longrightarrow>
-    w \<in> dVs (Pair_Graph_U_RBT.digraph_abs G) - Tree2.set_tree (DFS_Aux_state.seen (DFS_Aux' G s)) \<Longrightarrow>
-    \<nexists>p. awalk (Pair_Graph_U_RBT.digraph_abs G) v p w"
-  using assms[simplified DFS_Cycles_Interp.DFS_Cycles_axioms_def[of "G" "V"]]
-    DFS_Aux_Interp.DFS_Aux_correct_3[unfolded DFS_Aux_Interp.DFS_Aux_axioms_def]
-  by blast
-
-lemma DFS_Aux_correct_4_inst:
-  assumes "DFS_Cycles.DFS_Cycles_axioms isin Tree2.set_tree M.invar \<langle>\<rangle> rbt_inv lookup G V"
-    "s \<in> dVs (Pair_Graph_U_RBT.digraph_abs G)"
-  shows "rbt_inv (DFS_Aux_state.seen (DFS_Aux' G s))"
-  using assms[simplified DFS_Cycles_Interp.DFS_Cycles_axioms_def[of "G" "V"]]
-    DFS_Aux_Interp.DFS_Aux_correct_4[unfolded DFS_Aux_Interp.DFS_Aux_axioms_def]
-  by blast
-
-lemma DFS_Aux_correct_5_inst:
-  assumes "DFS_Cycles.DFS_Cycles_axioms isin Tree2.set_tree M.invar \<langle>\<rangle> rbt_inv lookup G V"
-    "s \<in> dVs (Pair_Graph_U_RBT.digraph_abs G)"
-  shows "v \<in> Tree2.set_tree (DFS_Aux_state.seen (DFS_Aux' G s)) \<Longrightarrow>
-    \<exists>p. awalk (Pair_Graph_U_RBT.digraph_abs G) s p v"
-  using assms[simplified DFS_Cycles_Interp.DFS_Cycles_axioms_def[of "G" "V"]]
-    DFS_Aux_Interp.DFS_Aux_correct_5[unfolded DFS_Aux_Interp.DFS_Aux_axioms_def]
-  by blast
-
-lemma DFS_Aux_correct_6_inst:
-  assumes "DFS_Cycles.DFS_Cycles_axioms isin Tree2.set_tree M.invar \<langle>\<rangle> rbt_inv lookup G V"
-    "s \<in> dVs (Pair_Graph_U_RBT.digraph_abs G)"
-  shows "s \<in> Tree2.set_tree (DFS_Aux_state.seen (DFS_Aux' G s))"
-  using assms[simplified DFS_Cycles_Interp.DFS_Cycles_axioms_def[of "G" "V"]]
-    DFS_Aux_Interp.DFS_Aux_correct_6[unfolded DFS_Aux_Interp.DFS_Aux_axioms_def]
-  by blast
-
-
-lemma DFS_Cycles_imp_dfs_aux_axioms:
-  assumes "DFS_Cycles.DFS_Cycles_axioms isin Tree2.set_tree M.invar \<langle>\<rangle> rbt_inv lookup G V"
-  shows "DFS_Cycles.dfs_aux_axioms isin Tree2.set_tree \<langle>\<rangle> rbt_inv lookup G (DFS_Aux' G) DFS_Aux_state.seen DFS_Aux_state.cycle"
-  unfolding DFS_Cycles_Interp.dfs_aux_axioms_def
-  using DFS_Aux_correct_1_inst[OF assms] DFS_Aux_correct_2_inst[OF assms] DFS_Aux_correct_3_inst[OF assms]
-    DFS_Aux_correct_4_inst[OF assms] DFS_Aux_correct_5_inst[OF assms] DFS_Aux_correct_6_inst[OF assms]
-  by meson
-
-
-thm DFS_Cycles_Interp.DFS_Cycles_correct_1
-
-(* If Pair_Graph_U_invar holds + relationship between G and V, we have cycle iff cycle in ugraph_abs *)
-
-abbreviation "DFS_Cycles' G V \<equiv> DFS_Cycles_Interp.DFS_Cycles V G DFS_Cycles_Interp.initial_state"
-
-thm Pair_Graph_U_RBT.pair_graph_u_invar_def
-thm DFS_Cycles.DFS_Cycles_axioms_def
-
-lemma DFS_Cycles_correct_final:
-  assumes "Pair_Graph_U_RBT.pair_graph_u_invar G" "rbt_inv V"
-    "Tree2.set_tree (V::(('a::linorder) rbt)) = dVs (Pair_Graph_U_RBT.digraph_abs G)"
-  shows "DFS_Cycles_state.cycle (DFS_Cycles' G V) = (\<exists>u c. decycle (Pair_Graph_U_RBT.ugraph_abs G) u c)"
-proof-
-  have "DFS_Cycles.DFS_Cycles_axioms isin Tree2.set_tree M.invar \<langle>\<rangle> rbt_inv lookup G V"
-    unfolding DFS_Cycles_Interp.DFS_Cycles_axioms_def 
-    using assms[simplified Pair_Graph_U_RBT.pair_graph_u_invar_def[of "G"]]
-      Pair_Graph_U_RBT.digraph_abs_irreflexive[OF assms(1)]
-      Pair_Graph_U_RBT.digraph_abs_symmetric[OF assms(1)] by fastforce
-
-  from DFS_Cycles_Interp.DFS_Cycles_correct_1[OF this DFS_Cycles_imp_dfs_aux_axioms[OF this]]
-    DFS_Cycles_Interp.DFS_Cycles_correct_2[OF this DFS_Cycles_imp_dfs_aux_axioms[OF this]]
-    have "DFS_Cycles_state.cycle (DFS_Cycles' G V) = (\<exists>c. cycle' (Pair_Graph_U_RBT.digraph_abs G) c)"
-    by blast
-  with Pair_Graph_U_RBT.cycle_equivalence[OF assms(1)]
-  show "DFS_Cycles_state.cycle (DFS_Cycles' G V) = (\<exists>u c. decycle (Pair_Graph_U_RBT.ugraph_abs G) u c)"
-    by blast
-qed
-
+find_theorems add_edge
 
 text \<open>Instantiations for Greedy\<close>
 
@@ -161,19 +25,19 @@ fun rbt_subseteq :: "('a::linorder) rbt \<Rightarrow> 'a rbt \<Rightarrow> bool"
   "rbt_subseteq t1 t2 = (case (RBT.diff t1 t2) of Leaf \<Rightarrow> True | _ \<Rightarrow> False)"
 
 lemma rbt_subseteq_correct:
-  "rbt_inv t1 \<Longrightarrow> rbt_inv t2 \<Longrightarrow> (rbt_subseteq t1 t2) = (Tree2.set_tree t1 \<subseteq> Tree2.set_tree t2)"
+  "vset_inv t1 \<Longrightarrow> vset_inv t2 \<Longrightarrow> (rbt_subseteq t1 t2) = (Tree2.set_tree t1 \<subseteq> Tree2.set_tree t2)"
 proof(unfold rbt_subseteq.simps tree.split[of "\<lambda> x. x= (_ \<subseteq> _)" True "\<lambda> _ _ _. False" "RBT.diff t1 t2" ],
       goal_cases)
   case 1
   have is_empty_iff:"RBT.diff t1 t2 = \<langle>\<rangle> \<longleftrightarrow> Tree2.set_tree t1 - Tree2.set_tree t2 = {}"
-    using 1  Tree2.eq_set_tree_empty 
-    by (subst RBT.set_tree_diff[of t1 t2, symmetric])fast+
+    using 1  Tree2.eq_set_tree_empty  RBT.set_tree_diff[of t1 t2, symmetric]
+    by (simp add: vset_inv_def)
   show ?case 
     using is_empty_iff by (subst Diff_eq_empty_iff[symmetric])fastforce
 qed
 
 lemma rbt_size_correct:
-  "rbt_inv X \<Longrightarrow> size X = card (Tree2.set_tree X)"
+  "vset_inv X \<Longrightarrow> size X = card (Tree2.set_tree X)"
   unfolding set_inorder[symmetric]
 proof(induction X rule: inorder.induct)
   case 1
@@ -182,26 +46,28 @@ next
   case (2 l a uu r)
   have inter_empty:"set (Tree2.inorder l) \<inter> Set.insert a (set (Tree2.inorder r)) = {}"
     using 2(3) bst.simps(2)[simplified Tree2.set_inorder[symmetric]]
-    by (metis Int_emptyI insert_iff not_less_iff_gr_or_eq)
-  have rbt_inv_l: "rbt_inv l" 
-    by (metis "2.prems" RBT.inv_Node bst.simps(2))
-  have rbt_inv_r: "rbt_inv r" 
-    by (metis "2.prems" RBT.inv_Node bst.simps(2))
+    by (metis (no_types, lifting) Int_emptyI insert_iff not_less_iff_gr_or_eq vset_inv_def)
+  have vset_inv_l: "vset_inv l" 
+    by (metis "2.prems" RBT.inv_Node bst.simps(2) vset_inv_def)
+  have vset_inv_r: "vset_inv r" 
+    by (metis "2.prems" RBT.inv_Node bst.simps(2) vset_inv_def)
   have a_not_down: "a \<notin> set (Tree2.inorder r)" 
-    using 2(3) bst.simps(2)[simplified Tree2.set_inorder[symmetric]] by fast
+    using 2(3) bst.simps(2)[simplified Tree2.set_inorder[symmetric]] 
+    by (metis not_less_iff_gr_or_eq vset_inv_def)
   show ?case 
    using a_not_down inter_empty 
-   by(auto  simp add: card_Un_disjoint card_insert_if  2(1)[OF rbt_inv_l] 2(2)[OF rbt_inv_r])
+   by(auto  simp add: card_Un_disjoint card_insert_if  2(1)[OF vset_inv_l] 2(2)[OF vset_inv_r])
 qed
 
 interpretation Custom_Set_RBT: Custom_Set
-  where empty = "\<langle>\<rangle>" and insert = insert_rbt and delete = delete_rbt and invar = "rbt_inv::(('e::linorder) rbt \<Rightarrow> bool)" and
+  where empty = "\<langle>\<rangle>" and insert = insert_rbt and delete = delete_rbt and invar = "vset_inv::(('e::linorder) rbt \<Rightarrow> bool)" and
     isin = isin and set = "Tree2.set_tree" and union = "RBT.union" and inter = "RBT.inter" and diff = "RBT.diff" and
     subseteq = rbt_subseteq and cardinality = size
   apply (subst Custom_Set_def)
   apply(intro conjI)
   subgoal
-    using RBT.Set2_axioms by blast
+    using RBT.Set2_axioms
+    by (metis RBT_Set.empty_def dfs.set_ops.Set2_axioms)
   subgoal
     apply (subst Custom_Set_axioms_def)
     using rbt_subseteq_correct rbt_size_correct by blast
@@ -210,17 +76,17 @@ interpretation Custom_Set_RBT: Custom_Set
 
 definition "set_of_sets_isin f a = f a"
 
+lemma set_of_sets_isin_def': "set_of_sets_isin = id"
+  using set_of_sets_isin_def by fastforce
+
 interpretation Matroid_Specs_Inst: Matroid_Specs
-  where set_empty = "\<langle>\<rangle>" and set_insert = insert_rbt and set_delete = delete_rbt and set_inv = "rbt_inv::(('e::linorder) rbt \<Rightarrow> bool)" and
+  where set_empty = "\<langle>\<rangle>" and set_insert = insert_rbt and set_delete = delete_rbt and set_inv = "vset_inv::(('e::linorder) rbt \<Rightarrow> bool)" and
     set_isin = isin and to_set = "Tree2.set_tree" and union = "RBT.union" and inter = "RBT.inter" and diff = "RBT.diff" and
     subseteq = rbt_subseteq and cardinality = size and
     set_of_sets_isin = "set_of_sets_isin :: ('e rbt \<Rightarrow> bool) \<Rightarrow> 'e rbt \<Rightarrow> bool"
   apply (subst Matroid_Specs_def)
   apply (subst Indep_System_Specs_def)
   using Custom_Set_RBT.Custom_Set_axioms by blast
-
-term "DFS_Cycles'"
-
 
 fun rbt_set_fold :: "'a rbt \<Rightarrow> ('a \<Rightarrow> 'b \<Rightarrow> 'b) \<Rightarrow> 'b \<Rightarrow> 'b" where
   "rbt_set_fold Leaf f acc = acc"
@@ -236,27 +102,24 @@ fun rbt_map_fold :: "('a \<times> 'd) rbt \<Rightarrow> ('a \<Rightarrow> 'd \<R
 lemma rbt_map_fold_revinorder: "rbt_map_fold T f acc = foldr (\<lambda> (x, y) acc. f x y acc) (rev (inorder T)) acc"
  by(induction T f acc rule: rbt_map_fold.induct) auto
 
-global_interpretation Kruskal_Graphs_Matroids: Graphs_Matroids_Encoding
+global_interpretation Kruskal_Graphs_Matroids: Encoding
   where empty = RBT_Set.empty and update = update and delete = RBT_Map.delete and
     lookup = lookup and adjmap_inv = "M.invar" and vset_empty = "\<langle>\<rangle>" and
-    insert = insert_rbt and vset_delete = delete_rbt and vset_inv = "rbt_inv::(('v::linorder) rbt \<Rightarrow> bool)" and
-    isin = isin and t_set = "Tree2.set_tree" and sel = rbt_sel and
+    insert = insert_rbt and vset_delete = delete_rbt and vset_inv = "vset_inv::(('v::linorder) rbt \<Rightarrow> bool)" and
+    isin = isin and t_set = "Tree2.set_tree" and sel = sel and
 
-    set_empty = "\<langle>\<rangle>" and set_insert = insert_rbt and set_delete = delete_rbt and set_inv = "rbt_inv::(('e::linorder) rbt \<Rightarrow> bool)" and
+    set_empty = "\<langle>\<rangle>" and set_insert = insert_rbt and set_delete = delete_rbt and set_inv = "vset_inv::(('e::linorder) rbt \<Rightarrow> bool)" and
     set_isin = isin and to_set = "Tree2.set_tree" and union = "RBT.union" and inter = "RBT.inter" and diff = "RBT.diff" and
-    subseteq = rbt_subseteq and cardinality = size and 
-    set_of_sets_isin = "set_of_sets_isin :: ('e rbt \<Rightarrow> bool) \<Rightarrow> 'e rbt \<Rightarrow> bool" and
-
     adjmap_fold = "rbt_map_fold" and vset_fold = "rbt_set_fold" and set_fold_adjmap = "rbt_set_fold" and
     set_fold_vset = "rbt_set_fold"
-    for v1_of :: "('e::linorder) \<Rightarrow> ('v::linorder)" and v2_of :: "('e::linorder) \<Rightarrow> ('v::linorder)" and 
-        edge_of :: "('v::linorder) \<Rightarrow> 'v \<Rightarrow> ('e::linorder)" and c :: "('v set) \<Rightarrow> rat" and c' :: "'e \<Rightarrow> rat"
-      defines graph_to_edges = Kruskal_Graphs_Matroids.graph_to_edges
-and edges_to_graph = Kruskal_Graphs_Matroids.edges_to_graph
+    for v1_of :: "('e::linorder) \<Rightarrow> ('v::linorder)" and v2_of :: "('e::linorder) \<Rightarrow> ('v::linorder)" (*and 
+        edge_of :: "('v::linorder) \<Rightarrow> 'v \<Rightarrow> ('e::linorder)"*) and c :: "('v set) \<Rightarrow> rat" and c' :: "'e \<Rightarrow> rat"
+      defines (*graph_to_edges = Kruskal_Graphs_Matroids.graph_to_edges
+and*) edges_to_graph = Kruskal_Graphs_Matroids.edges_to_graph
 and edges_to_vertices = Kruskal_Graphs_Matroids.edges_to_vertices
-  apply (subst Graphs_Matroids_Encoding_def)
-  using Pair_Graph_U_RBT.Pair_Graph_U_Specs_axioms Matroid_Specs_Inst.Matroid_Specs_axioms
-  by blast
+  by (auto intro: Encoding.intro simp add: Custom_Set_RBT.Set2_axioms Pair_Graph_U_RBT.Pair_Graph_U_Specs_axioms)
+
+
 
 lemma map_of_dom_is:"set (map fst list) = {a. AList_Upd_Del.map_of list a \<noteq> None}"
 proof(induction list)
@@ -345,20 +208,16 @@ qed
 lemma bst_distinct_inorder:"bst T \<Longrightarrow> distinct (inorder T)"
   by(induction T rule: inorder.induct) fastforce+
 
-lemma rbt_set_fold_correct: "rbt_inv S \<Longrightarrow> \<exists>xs. distinct xs \<and> set xs = Tree2.set_tree S \<and> rbt_set_fold S f G = foldr f xs G"
+lemma rbt_set_fold_correct: "vset_inv S \<Longrightarrow> \<exists>xs. distinct xs \<and> set xs = Tree2.set_tree S \<and> rbt_set_fold S f G = foldr f xs G"
   apply(subst rbt_set_fold_revinorder)
   apply(rule exI[of _ "rev (Tree2.inorder S)"])
   using  bst_distinct_inorder[of S]
-  by (unfold set_inorder[symmetric] set_rev distinct_rev ) fastforce
+  by(unfold set_inorder[symmetric] set_rev distinct_rev)(simp add: vset_inv_def )
 
-locale Transforms =
+locale Oracle =
 fixes v1_of::"('e::linorder \<Rightarrow> 'v::linorder)" and v2_of::"'e \<Rightarrow> 'v" 
-and edge_of::"'v \<Rightarrow> 'v \<Rightarrow> 'e"
-and input_G :: "('v * ('v rbt)) rbt" 
+and input_G :: "'e rbt"
 begin
-
-abbreviation Kruskal_G_to_E :: "(('v::linorder) \<times> ('v rbt)) rbt \<Rightarrow> 'e rbt" where
-  "Kruskal_G_to_E \<equiv> graph_to_edges edge_of"
 
 definition Kruskal_E_to_G :: "('e::linorder) rbt \<Rightarrow> ('v \<times> ('v rbt)) rbt" where
   "Kruskal_E_to_G = edges_to_graph v1_of v2_of"
@@ -366,569 +225,811 @@ definition Kruskal_E_to_G :: "('e::linorder) rbt \<Rightarrow> ('v \<times> ('v 
 definition Kruskal_E_to_V :: "('e::linorder) rbt \<Rightarrow> ('v rbt)" where
   "Kruskal_E_to_V = edges_to_vertices v1_of v2_of"
 
-definition carrier_graph_matroid :: "('e::linorder) rbt" where
-  "carrier_graph_matroid = graph_to_edges edge_of input_G"
+definition indep_graph_matroid :: "('e::linorder) rbt \<Rightarrow> bool" where
+  "indep_graph_matroid = (\<lambda> E. undirected_multigraph_spec.has_no_cycle_multi (\<lambda> e. {v1_of e, v2_of e})
+                              (Tree2.set_tree input_G) (Tree2.set_tree E))"
 
-fun indep_graph_matroid :: "('e::linorder) rbt \<Rightarrow> bool" where
-  "indep_graph_matroid E = 
-    (let
-      G = (Kruskal_E_to_G E);
-      V = (Kruskal_E_to_V E)
-    in
-      (if rbt_subseteq E carrier_graph_matroid then \<not>DFS_Cycles_state.cycle (DFS_Cycles' G V)
-      else False))"
+definition "local_indep_oracle e X = 
+((rbt_subseteq (vset_insert e X) input_G) \<and>
+                   (lookup (Kruskal_E_to_G X) (v2_of e) \<noteq> None \<and> lookup (Kruskal_E_to_G X) (v1_of e) \<noteq> None\<longrightarrow>
+                   return (dfs_impl (Kruskal_E_to_G X) (\<lambda> w. w = v2_of e) (dfs_initial_state (v1_of e))) 
+                    = NotReachable))"
+
 end
 
-global_interpretation transforms: Transforms
-  where v1_of = v1_of and v2_of = v2_of and edge_of = edge_of and input_G = input_G
+global_interpretation orcl: Oracle
+  where v1_of = v1_of and v2_of = v2_of  and input_G = input_G
   for v1_of::"'e::linorder \<Rightarrow> 'a::linorder" and v2_of edge_of input_G
-  defines Kruskal_G_to_E = transforms.Kruskal_G_to_E
-   and Kruskal_E_to_G=transforms.Kruskal_E_to_G
-   and Kruskal_E_to_V=transforms.Kruskal_E_to_V
-   and carrier_graph_matroid=transforms.carrier_graph_matroid
-   and indep_graph_matroid=transforms.indep_graph_matroid
+  defines Kruskal_E_to_G=orcl.Kruskal_E_to_G
+   and Kruskal_E_to_V=orcl.Kruskal_E_to_V
+   and indep_graph_matroid=orcl.indep_graph_matroid
+   and local_indep_oracle= orcl.local_indep_oracle
   done
 
-
-
-global_interpretation Kruskal_Greedy: Best_In_Greedy
+global_interpretation Kruskal_Greedy: Best_In_Greedy'
   where set_empty = "\<langle>\<rangle>" and set_insert = insert_rbt and set_delete = delete_rbt 
-     and set_inv = "rbt_inv::(('e::linorder) rbt \<Rightarrow> bool)" and
+     and set_inv = "vset_inv::(('e::linorder) rbt \<Rightarrow> bool)" and
     set_isin = isin and to_set = "Tree2.set_tree" and union = "RBT.union" and inter = "RBT.inter" and diff = "RBT.diff" and
     subseteq = rbt_subseteq and cardinality = size and
     set_of_sets_isin = "set_of_sets_isin :: (('e::linorder) rbt \<Rightarrow> bool) \<Rightarrow> 'e rbt \<Rightarrow> bool" and 
-    carrier = "carrier_graph_matroid edge_of input_G" 
-and indep_set = "indep_graph_matroid v1_of v2_of edge_of input_G" and
-    sort_desc = insort_key_desc
-  for v1_of::"'e::linorder \<Rightarrow>'a::linorder" and v2_of edge_of input_G
-  (* TODO should we instantiate remaining parameters here or just outside? \<Rightarrow> probably should instantiate carrier and indep_set
-  here since they are specified in the locale, but cannot yet instantiate c and order *)
-  apply (subst Best_In_Greedy_def)
-  using Matroid_Specs_Inst.Matroid_Specs_axioms by blast
-
-abbreviation "indep'  == Kruskal_Greedy.indep' (TYPE ('a::linorder))"
+    carrier = input_G and 
+    indep_set = "indep_graph_matroid v1_of v2_of input_G" and
+    sort_desc = insort_key_desc and 
+    local_indep_oracle = "local_indep_oracle v1_of v2_of input_G"
+    and wrapper_insert = insert_rbt
+and wrapper_invar = "vset_inv::(('e::linorder) rbt \<Rightarrow> bool)"
+and remove_wrapper = id
+and wrapper_empty = Leaf
+  for v1_of::"'e::linorder \<Rightarrow>'a::linorder" and v2_of input_G
+  defines kruskal' = Kruskal_Greedy.BestInGreedy'
+    and  kruskal = Kruskal_Greedy.BestInGreedy
+    and   kruskal_init = Kruskal_Greedy.initial_state
+    and   kruskal_init' = Kruskal_Greedy.initial_state'
+    and indep' = "Kruskal_Greedy.indep'"
+    and to_ordinary = Kruskal_Greedy.to_ordinary
+  apply (subst Best_In_Greedy'_def, subst Best_In_Greedy_def)
+ by(auto intro!: Best_In_Greedy'_axioms.intro 
+simp add: Matroid_Specs_Inst.Matroid_Specs_axioms Pair_Graph_RBT.set.Set_axioms
+ dfs.Graph.vset.set.invar_insert set.invar_empty)
 
 locale Kruskal_Proof_Matroid_Edges =
-Transforms +
-  assumes v1_never_v2:"\<And> e. v1_of (e::'e::linorder) \<noteq> v2_of e"
-and v1_of_edge_of: "x \<noteq> y \<Longrightarrow> v1_of (edge_of x y) = x \<or> v1_of (edge_of x y) = y"
-and v2_of_edge_of: "x \<noteq> y \<Longrightarrow> v2_of (edge_of x y) = x \<or> v2_of (edge_of x y) = y"
+Oracle where v1_of = "v1_of::'e::linorder \<Rightarrow> 'v::linorder" for v1_of+
+assumes v1_never_v2:"\<And> e. v1_of e \<noteq> v2_of e"
 begin
 
-interpretation Kruskal_Graphs_Matroids_Proofs: Graphs_Matroids_Encoding_Proofs
-  where empty = RBT_Set.empty and update = update and delete = RBT_Map.delete and
-    lookup = lookup and adjmap_inv = "M.invar" and vset_empty = "\<langle>\<rangle>" and
-    insert = insert_rbt and vset_delete = delete_rbt and vset_inv = "rbt_inv::(('a::linorder) rbt \<Rightarrow> bool)" and
-    isin = isin and t_set = "Tree2.set_tree" and sel = rbt_sel and
-
-    set_empty = "\<langle>\<rangle>" and set_insert = insert_rbt and set_delete = delete_rbt and set_inv = "rbt_inv::(('e::linorder) rbt \<Rightarrow> bool)" and
-    set_isin = isin and to_set = "Tree2.set_tree" and union = "RBT.union" and inter = "RBT.inter" and diff = "RBT.diff" and
-    subseteq = rbt_subseteq and cardinality = size and 
-    set_of_sets_isin = "set_of_sets_isin :: ('e rbt \<Rightarrow> bool) \<Rightarrow> 'e rbt \<Rightarrow> bool" and
-
-    adjmap_fold = "rbt_map_fold" and vset_fold = "rbt_set_fold" and set_fold_adjmap = "rbt_set_fold" and
-    set_fold_vset = "rbt_set_fold"
-  for c :: "('a set) \<Rightarrow> rat" and c' :: "'e \<Rightarrow> rat"
- proof(rule Graphs_Matroids_Encoding_Proofs.intro, 
-     rule Kruskal_Graphs_Matroids.Graphs_Matroids_Encoding_axioms, 
-     rule Graphs_Matroids_Encoding_Proofs_axioms.intro, goal_cases)
+context 
+  assumes  G_good: "vset_inv input_G"
+begin
+lemma Encoding_Proofs_axioms:
+ " Encoding_Proofs_axioms t_set M.invar vset_inv lookup vset_inv t_set rbt_map_fold
+     rbt_set_fold rbt_set_fold rbt_set_fold v1_of v2_of"(* edge_of"*)
+proof(rule Encoding_Proofs_axioms.intro, goal_cases)
   case (1 G S f)
-  then show ?case by(auto intro:  rbt_map_fold_correct)
+  then show ?case 
+    by (simp add: rbt_map_fold_correct)
 next
   case (2 G S f)
-  show ?case 
-  by(insert 2, rule rbt_set_fold_correct[of S f G]) fast
+  then show ?case 
+    by (simp add: rbt_set_fold_correct)
 next
   case (3 V f S)
-  show ?case by(insert 3, rule rbt_set_fold_correct) fast
-next
-  case 5
-  then show ?case  by(auto intro: finite_set_tree simp add: Pair_Graph_Specs.finite_vsets_def[OF Pair_Graph_U_RBT.Pair_Graph_Specs_axioms])
+  then show ?case 
+    by (simp add: rbt_set_fold_correct)
 next
   case (4 V f S)
-  show ?case  by(insert 4, rule rbt_set_fold_correct) fast
+  then show ?case 
+    by (simp add: rbt_set_fold_correct)
+next
+  case 5
+  then show ?case 
+    by (simp add: dfs.Graph.finite_vsetsI)
 next
   case (6 e)
-  thus ?case 
+  then show ?case 
     by (simp add: v1_never_v2)
+qed
+(*
 next
   case (7 x y)
-  thus ?case 
-    using v1_of_edge_of by blast
+  then show ?case
+    by (simp add: v1_of_edge_of)
 next
   case (8 x y)
-  thus ?case
-    using v2_of_edge_of by presburger
+  then show ?case
+    by (simp add: v2_of_edge_of)
+qed
+*)
+interpretation Kruskal_Graphs_Matroids_proofs: Encoding_Proofs
+  where empty = RBT_Set.empty and update = update and delete = RBT_Map.delete and
+    lookup = lookup and adjmap_inv = "M.invar" and vset_empty = "\<langle>\<rangle>" and
+    insert = insert_rbt and vset_delete = delete_rbt and vset_inv = "vset_inv::(('v::linorder) rbt \<Rightarrow> bool)" and
+    isin = isin and t_set = "Tree2.set_tree" and sel = sel and
+
+    set_empty = "\<langle>\<rangle>" and set_insert = insert_rbt and set_delete = delete_rbt and set_inv = "vset_inv::(('e::linorder) rbt \<Rightarrow> bool)" and
+    set_isin = isin and to_set = "Tree2.set_tree" and union = "RBT.union" and inter = "RBT.inter" and diff = "RBT.diff" and
+    adjmap_fold = "rbt_map_fold" and vset_fold = "rbt_set_fold" and set_fold_adjmap = "rbt_set_fold" and
+    set_fold_vset = "rbt_set_fold"
+  for c :: "('v set) \<Rightarrow> rat" and c' :: "'e \<Rightarrow> rat"
+  by(auto intro!: Encoding_Proofs.intro  Encoding_Proofs_axioms 
+           simp add: Encoding_def 
+            Pair_Graph_U_RBT.Pair_Graph_U_Specs_axioms Custom_Set_RBT.Set2_axioms)
+
+lemma pair_graph_u_invar:
+"vset_inv S \<Longrightarrow> Pair_Graph_U_RBT.pair_graph_u_invar (Kruskal_E_to_G S)"
+  by (simp add: Kruskal_Graphs_Matroids_proofs.edges_invar_imp_graph_invar edges_to_graph_def local.Kruskal_E_to_G_def)
+
+lemma same_dgraphabs:"dfs.Graph.digraph_abs = G.digraph_abs"
+  by (simp add: RBT_Set.empty_def)
+
+abbreviation "to_dbltn == (\<lambda>x. {v1_of x, v2_of x})"
+
+lemma to_dbltn_sym: "{v2_of x, v1_of x} = to_dbltn x" by auto
+
+interpretation undirected_multigraph: undirected_multigraph to_dbltn "Tree2.set_tree G"
+  using v1_never_v2 by (auto intro!:  undirected_multigraph.intro)
+
+lemma local_indep_oracle_correct:
+  assumes "vset_inv S"
+        "indep' v1_of v2_of input_G (id S)"
+        "rbt_subseteq (id S) input_G"
+        "e \<notin> t_set (id S)"
+ shows "local_indep_oracle e S = indep' v1_of v2_of input_G (vset_insert e (id S))"
+  apply(insert assms)
+  unfolding indep'_def Matroid_Specs_Inst.indep_def indep_graph_matroid_def
+            indep_graph_matroid_def set_of_sets_isin_def 
+proof(goal_cases)
+  case 1
+  note case_assms = this
+  have first_eq:"rbt_subseteq (vset_insert e S) input_G = (t_set (vset_insert e (id S)) \<subseteq> t_set input_G)" 
+    using G_good assms(1) dfs.Graph.vset.set.invar_insert rbt_subseteq_correct by auto
+  have second_eq:"(((lookup (local.Kruskal_E_to_G S) (v2_of e) \<noteq> None \<and> lookup (Kruskal_E_to_G S) (v1_of e) \<noteq> None) \<longrightarrow>
+                 (return (dfs_impl (local.Kruskal_E_to_G S) (\<lambda> w. w = v2_of e) 
+                 (dfs_initial_state (v1_of e))) = NotReachable))) =
+                (\<nexists>u. Ex (undirected_multigraph_spec.decycle_multi (\<lambda>e. {v1_of e, v2_of e}) (t_set (vset_insert e (id S)))u))"
+    if additional_assm: "insert e (t_set  S) \<subseteq> t_set input_G"
+  proof-
+    have digraph_abs_is:"G.digraph_abs (Kruskal_E_to_G S) =
+     (\<lambda>e. (v1_of e, v2_of e)) ` t_set S \<union> (\<lambda>e. (v2_of e, v1_of e)) ` t_set S"
+     by(auto intro!: Kruskal_Graphs_Matroids_proofs.digraph_abs_of_edges_of_to_graph_general
+            simp add: assms(1) Kruskal_E_to_G_def edges_to_graph_def )
+   have ugraph_abs_is: "Pair_Graph_U_RBT.ugraph_abs (Kruskal_E_to_G S) = to_dbltn ` (t_set  S)"
+    by(auto intro!: Kruskal_Graphs_Matroids_proofs.dbltn_set_and_ugraph_abs[symmetric]
+            simp add: assms(1) Kruskal_E_to_G_def edges_to_graph_def )
+   have pair_graph_u_invar:"Pair_Graph_U_RBT.pair_graph_u_invar (edges_to_graph  v1_of  v2_of S)" 
+     using assms(1) local.Kruskal_E_to_G_def pair_graph_u_invar by auto
+   have double_ex_I: "rest x y \<Longrightarrow> \<exists>v1 v2.
+       {x, y} = {v1, v2} \<and> rest v1 v2" for x y rest by auto
+   have lookup_in_dVs:"lookup (local.Kruskal_E_to_G S) x = Some y\<Longrightarrow> 
+          x \<in> dVs (dfs.Graph.digraph_abs (local.Kruskal_E_to_G S))" for x y
+     using Kruskal_Graphs_Matroids_proofs.edges_invar_imp_graph_invar(2)[OF assms(1)]
+            S_C.choose  
+     by(unfold  dfs.Graph.digraph_abs_def DFS_Example.neighbourhood_def)
+       (auto simp add: Kruskal_E_to_G_def edges_to_graph_def
+                      neighbourhood_def[symmetric] dfs.Graph.neighbourhood_def dVs_def
+               intro!: exI[of _ "{x, sel y}"]  double_ex_I)
+   have "lookup (local.Kruskal_E_to_G S) (v1_of e) = Some y \<Longrightarrow>
+         DFS.DFS_axioms isin t_set adj_inv vset_empty vset_inv lookup
+          (local.Kruskal_E_to_G S) (v1_of e)" for y
+     unfolding DFS.DFS_axioms_def[OF dfs.DFS_axioms]
+     using   lookup_in_dVs pair_graph_u_invar
+     by(unfold Pair_Graph_U_RBT.pair_graph_u_invar_def Kruskal_E_to_G_def adj_inv_def)
+     simp
+   hence DFS_thms: "lookup (local.Kruskal_E_to_G S) (v1_of e) \<noteq> None \<Longrightarrow>
+        DFS_thms map_empty RBT_Map.delete vset_insert isin t_set sel update adj_inv vset_empty vset_delete vset_inv
+     vset_union vset_inter vset_diff lookup (Kruskal_E_to_G S) (v1_of e)"
+     by(auto intro!: DFS_thms.intro dfs.DFS_axioms DFS_thms_axioms.intro )
+   have graph_abs_with_e: "graph_abs (to_dbltn ` insert e (t_set S))"
+     using v1_never_v2 by (auto simp add: graph_abs_def dblton_graph_def Vs_def)
+   have graph_abs_without_e: "graph_abs (to_dbltn `(t_set S))"
+     using graph_abs_mono graph_abs_with_e by auto
+   have graph_abs_vset_insert:"graph_abs (to_dbltn ` t_set (vset_insert e S))"
+     using RBT.set_tree_insert[of S] case_assms(1) graph_abs_with_e 
+     by(simp add:vset_inv_def)
+   show ?thesis 
+     unfolding dfs_impl_def dfs_initial_state_def
+   proof(cases "lookup (local.Kruskal_E_to_G S) (v1_of e) \<noteq> None 
+         \<and> lookup (local.Kruskal_E_to_G S) (v2_of e) \<noteq> None", goal_cases)
+     case 1
+     hence 1: "lookup (local.Kruskal_E_to_G S) (v1_of e) \<noteq> None" 
+              "lookup (local.Kruskal_E_to_G S) (v2_of e) \<noteq> None" by auto
+     note one = this
+     show ?case
+     proof(subst DFS_thms.DFS_to_DFS_impl[OF DFS_thms, symmetric, OF 1(1)], rule, all \<open>rule ccontr\<close>, goal_cases)
+       case 1
+       then obtain u C where uC_prop:"undirected_multigraph_spec.decycle_multi to_dbltn
+                 (t_set (vset_insert e S)) u C" by auto
+       moreover have  not_cycle_old:"\<not> undirected_multigraph_spec.decycle_multi to_dbltn
+                 (t_set S) u C" 
+         using case_assms(2) 
+         by(simp add: id_def undirected_multigraph_spec.has_no_cycle_multi_def
+                    Kruskal_Greedy.indep_graph_matroid_def local.indep_graph_matroid_def
+                )
+       ultimately have e_and_C:"e \<in> set C" "set C \<subseteq> (t_set (vset_insert e S))"
+         unfolding undirected_multigraph_spec.decycle_multi_def     
+        using epath_subset_other_set[of "insert {v1_of e, v2_of e} (to_dbltn ` t_set S)"
+                                    u "map _ C" u , simplified list.set_map,OF _ image_mono] 
+        by (auto simp add: Pair_Graph_RBT.set.set_insert[OF case_assms(1)])
+      then obtain C1 C2 where C_split:"C = C1@[e]@C2"
+        by (metis append_Cons append_self_conv2 split_list_last)
+      obtain q where q_prop:"walk_betw (to_dbltn ` (insert e (t_set S))) u q u" "map to_dbltn C = edges_of_path q"
+        using graph_abs.epath_imp_walk_betw[of _ u "map to_dbltn C" u, OF graph_abs_with_e] 
+              uC_prop 
+         by(auto simp add: undirected_multigraph_spec.decycle_multi_def  Pair_Graph_RBT.set.set_insert[OF case_assms(1)])
+      
+       hence e_in_p: "to_dbltn e \<in> set (edges_of_path q)"
+        by (metis (mono_tags, lifting) \<open>e \<in> set C\<close> image_set rev_image_eqI)
+      have lengthq: "length q \<ge> 2" 
+        using \<open>to_dbltn e \<in> set (edges_of_path q)\<close> edges_of_path_nempty by fastforce
+      have v1v2: "v1_of e \<noteq> v2_of e" 
+        by (simp add: v1_never_v2)
+    show ?case proof(cases "lookup (local.Kruskal_E_to_G S) (v2_of e)")
+      case None
+       thus ?thesis 
+        by (simp add: one(2))
+    next
+      case (Some neighb)
+      have "\<exists>q. walk_betw (to_dbltn ` t_set (vset_insert e S)) u q u \<and> map to_dbltn C = edges_of_path q"
+        using graph_abs_vset_insert  uC_prop 
+        by(auto intro:graph_abs.epath_imp_walk_betw simp add: undirected_multigraph.decycle_multi_def)
+      have no_distinct_path:"\<nexists>p. distinct p \<and>
+              vwalk_bet (dfs.Graph.digraph_abs (local.Kruskal_E_to_G S)) (v1_of e) p (v2_of e)"
+        using DFS_thms.DFS_correct_1[OF DFS_thms] Some  one 1 by blast
+      have no_other_e:"(to_dbltn e) \<notin> (to_dbltn ` t_set S)"
+      proof(rule, rule ccontr, goal_cases)
+        case 1
+        then obtain d where d_prop:"to_dbltn d = to_dbltn e" "d \<in> t_set S" by auto
+        hence "{(v1_of d, v2_of d), (v2_of d, v1_of d)} \<subseteq> (dfs.Graph.digraph_abs (local.Kruskal_E_to_G S))"
+          by (simp add: RBT_Set.empty_def digraph_abs_is)
+        moreover have "(v1_of e, v2_of e) = (v1_of d, v2_of d)\<or>(v1_of e, v2_of e) = (v2_of d, v1_of d)"
+          using d_prop by(unfold doubleton_eq_iff) presburger
+        ultimately have "vwalk_bet (dfs.Graph.digraph_abs (Kruskal_E_to_G S)) 
+                         (v1_of e) [v1_of e, v2_of e] (v2_of e)" 
+          by fastforce
+        moreover have "distinct [v1_of e, v2_of e]"
+          using v1v2 by auto
+        ultimately show ?case 
+          using   no_distinct_path by blast
+      qed 
+      moreover have dbltn_inj:"inj_on to_dbltn (t_set S) "
+        using case_assms(2) undirected_multigraph.has_no_cycle_multi_to_dbltn_inj 
+        by(auto simp add: Kruskal_Greedy.indep_graph_matroid_def
+                          local.indep_graph_matroid_def)
+      ultimately have dbltn_inj_big:"inj_on to_dbltn (insert e (t_set S))" by auto
+      moreover have C_subset:"set C \<subseteq> (insert e (t_set S))"
+        using case_assms(1) dfs.Graph.vset.set.set_insert e_and_C(2) by auto
+      ultimately have inj_C:"inj_on to_dbltn (set C)" 
+        by (meson inj_on_subset)
+      have distinct_edges_q:"distinct (edges_of_path q)"
+        using q_prop(2) distinct_map[of to_dbltn C] uC_prop e_and_C inj_C
+        by(auto simp add: undirected_multigraph.decycle_multi_def) 
+      have e_vs_in_new_v_set:"{v1_of e, v2_of e} \<subseteq> Vs (to_dbltn ` insert e (t_set S))"
+        by (simp add: vs_member)
+      then obtain q1 q2 where q1_q2_prop: "q = q1@[v1_of e, v2_of e]@ q2 \<or> q = q1@[v2_of e, v1_of e]@ q2"
+        using undirected_multigraph.edges_to_path_split_by_edge[of _ _ "v1_of e" "v2_of e"] e_in_p by fast
+       obtain q' where  path_without_e:"walk_betw (to_dbltn `  (t_set S)) (v1_of e) q' (v2_of e)"
+       proof(cases rule: disjE[OF q1_q2_prop], all "cases q1", all \<open>cases q2\<close>, goal_cases)
+         case 1
+         then show ?case 
+           using q_prop(1) v1v2 walk_between_nonempty_pathD(3) walk_between_nonempty_pathD(4) by fastforce
+       next
+         case (2 a list)
+         hence a1:"walk_betw (to_dbltn ` insert e (t_set S)) u (q1 @ [v1_of e]) (v1_of e)"
+           using q_prop(1) by (intro walk_pref[of _ u q1 "v1_of e" "v2_of e # q2" u]) force
+         moreover have a2:"walk_betw (to_dbltn ` insert e (t_set S)) (v2_of e) (v2_of e # q2) u"
+           using q_prop(1) 2(2)  by(intro walk_suff[of _ u "q1@[v1_of e]" "v2_of e" q2 u]) force 
+         ultimately have a3:"walk_betw (to_dbltn ` insert e (t_set S)) (v2_of e) ([v2_of e] @ q2) (v1_of e)"
+           by (simp add: "2"(3) walk_betw_def)
+         have a4:"set (edges_of_path ([v2_of e] @ q2)) \<subseteq> set (edges_of_path q)"
+           using "2"(2) "2"(3) by auto
+         moreover have a5:"to_dbltn e \<notin> set (edges_of_path ([v2_of e] @ q2))" 
+           using "2"(2) "2"(3) distinct_edges_q by auto
+         ultimately have a6:"set (edges_of_path ([v2_of e] @ q2)) \<subseteq> (to_dbltn `(t_set S))" 
+           using a3 graph_abs.path_ball_edges' graph_abs_with_e walk_between_nonempty_pathD(1) by fastforce
+         have "walk_betw (to_dbltn `(t_set S)) (v2_of e) ([v2_of e] @ q2) (v1_of e)"  
+           using walk_betw_strengthen[OF a3 _ a6] 2(4) by simp
+         hence "walk_betw (to_dbltn `(t_set S)) (v1_of e) (rev ([v2_of e] @ q2)) (v2_of e)" 
+           by (meson walk_symmetric)
+         thus ?case
+           using 2(1) by simp         
+       next
+         case (3 a list)
+         hence a1:"walk_betw (to_dbltn ` insert e (t_set S)) u (q1 @ [v1_of e]) (v1_of e)"
+           using q_prop(1) by (intro walk_pref[of _ u q1 "v1_of e" "v2_of e # q2" u]) force
+         moreover have a2:"walk_betw (to_dbltn ` insert e (t_set S)) (v2_of e) (v2_of e # q2) u"
+           using q_prop(1) 3(2)  by(intro walk_suff[of _ u "q1@[v1_of e]" "v2_of e" q2 u]) force 
+         ultimately have a3:"walk_betw (to_dbltn ` insert e (t_set S)) (v2_of e) (q1@ [v1_of e] ) (v1_of e)"
+           by (simp add: "3"(4) walk_betw_def)
+         have a4:"set (edges_of_path (q1@ [v1_of e])) \<subseteq> set (edges_of_path q)" 
+           using 3(2-) edges_of_path_append_subset_2 by fastforce
+         moreover have a5:"to_dbltn e \<notin> set (edges_of_path (q1@ [v1_of e]))" 
+           using  distinct_edges_q by(unfold 3(2) edges_of_path_symmetric_split) simp
+         ultimately have a6:"set (edges_of_path (q1@ [v1_of e])) \<subseteq> (to_dbltn `(t_set S))" 
+           using a3 graph_abs.path_ball_edges' graph_abs_with_e walk_between_nonempty_pathD(1) by fastforce
+         have "walk_betw (to_dbltn `(t_set S)) (v2_of e) (q1@ [v1_of e]) (v1_of e)"  
+           using walk_betw_strengthen[OF a3 _ a6] 3(3) by simp
+         hence "walk_betw (to_dbltn `(t_set S)) (v1_of e) (rev (q1@ [v1_of e])) (v2_of e)" 
+           by (meson walk_symmetric)
+         thus ?case
+           using 3(1) by simp 
+       next
+         case (4 a list aa lista)
+         hence a1:"walk_betw (to_dbltn ` insert e (t_set S)) u (q1 @ [v1_of e]) (v1_of e)"
+           using q_prop(1) by (intro walk_pref[of _ u q1 "v1_of e" "v2_of e # q2" u]) force
+         moreover have a2:"walk_betw (to_dbltn ` insert e (t_set S)) (v2_of e) (v2_of e # q2) u"
+           using q_prop(1) 4(2)  by(intro walk_suff[of _ u "q1@[v1_of e]" "v2_of e" q2 u]) force     
+         have a4:"set (edges_of_path (q1@ [v1_of e])) \<subseteq> set (edges_of_path q)" 
+           using 4(2-) edges_of_path_append_subset_2 by fastforce
+         moreover have a5:"to_dbltn e \<notin> set (edges_of_path (q1@ [v1_of e]))" 
+           using  distinct_edges_q by(unfold 4(2) edges_of_path_symmetric_split) simp
+         ultimately have a6:"set (edges_of_path (q1@ [v1_of e])) \<subseteq> (to_dbltn `(t_set S))" 
+           using graph_abs.path_ball_edges' graph_abs_with_e walk_between_nonempty_pathD(1) by fastforce
+         have a4:"set (edges_of_path ([v2_of e] @ q2)) \<subseteq> set (edges_of_path q)"
+           using "4"(2) edges_of_path_append_subset by fastforce
+         moreover have a5:"to_dbltn e \<notin> set (edges_of_path ([v2_of e] @ q2))" 
+           using  "4"(4) distinct_edges_q by(unfold 4(2) edges_of_path_symmetric_split) simp 
+         moreover have a3:"walk_betw (to_dbltn ` insert e (t_set S)) (v2_of e) ([v2_of e] @ q2) u"
+           using a2 a1 by simp 
+         ultimately have a7:"set (edges_of_path ([v2_of e] @ q2)) \<subseteq> (to_dbltn `(t_set S))"
+           using  a1 a2 graph_abs.path_ball_edges' graph_abs_with_e walk_between_nonempty_pathD(1) by fast 
+         have "walk_betw (to_dbltn `(t_set S)) u (q1@ [v1_of e]) (v1_of e)"  
+           using walk_betw_strengthen 4(3) a1 a6 by fastforce
+         moreover have "walk_betw (to_dbltn `(t_set S)) (v2_of e) ( [v2_of e]@q2)u"  
+           using walk_betw_strengthen 4(3)  "4"(4) a3 a7 by fastforce
+         ultimately have  "walk_betw (to_dbltn `(t_set S)) (v2_of e) ( ([v2_of e]@q2@(tl q1)@[v1_of e])) (v1_of e)" 
+           using "4"(3) walk_transitive_2 by fastforce
+         then show ?case 
+           using 4(1)[of "rev ([v2_of e]@q2@(tl q1)@[v1_of e])"]
+           by (meson walk_symmetric)
+       next
+         case 5
+         then show ?case 
+           using q_prop(1) v1v2 walk_between_nonempty_pathD(3) walk_between_nonempty_pathD(4) by fastforce
+       next
+         case (6 a list)
+         hence a1:"walk_betw (to_dbltn ` insert e (t_set S)) u (q1 @ [v2_of e]) (v2_of e)"
+           using q_prop(1) by (intro walk_pref[of _ u q1 "v2_of e" "v1_of e # q2" u]) force
+         moreover have a2:"walk_betw (to_dbltn ` insert e (t_set S)) (v1_of e) (v1_of e # q2) u"
+           using q_prop(1) 6(2)  by(intro walk_suff[of _ u "q1@[v2_of e]" "v1_of e" q2 u]) force 
+         ultimately have a3:"walk_betw (to_dbltn ` insert e (t_set S)) (v1_of e) ([v1_of e] @ q2) (v2_of e)"
+           by (simp add: "6"(3) walk_betw_def)
+         have a4:"set (edges_of_path ([v1_of e] @ q2)) \<subseteq> set (edges_of_path q)"
+           using "6"(2) "6"(3) by auto
+         moreover have a5:"to_dbltn e \<notin> set (edges_of_path ([v1_of e] @ q2))" 
+           using "6"(2) "6"(3) distinct_edges_q 
+           by (simp add: insert_commute)
+         ultimately have a6:"set (edges_of_path ([v1_of e] @ q2)) \<subseteq> (to_dbltn `(t_set S))" 
+           using a3 graph_abs.path_ball_edges' graph_abs_with_e walk_between_nonempty_pathD(1) by fastforce
+         have "walk_betw (to_dbltn `(t_set S)) (v1_of e) ([v1_of e] @ q2) (v2_of e)"  
+           using walk_betw_strengthen[OF a3 _ a6] 6(4) by simp
+         thus ?case
+           using 6(1) by simp         
+       next
+         case (7 a list)
+         hence a1:"walk_betw (to_dbltn ` insert e (t_set S)) u (q1 @ [v2_of e]) (v2_of e)"
+           using q_prop(1) by (intro walk_pref[of _ u q1 "v2_of e" "v1_of e # q2" u]) force
+         moreover have a2:"walk_betw (to_dbltn ` insert e (t_set S)) (v1_of e) (v1_of e # q2) u"
+           using q_prop(1) 7(2)  by(intro walk_suff[of _ u "q1@[v2_of e]" "v1_of e" q2 u]) force 
+         ultimately have a3:"walk_betw (to_dbltn ` insert e (t_set S)) (v1_of e) (q1@ [v2_of e] ) (v2_of e)"
+           by (simp add: "7"(4) walk_betw_def)
+         have a4:"set (edges_of_path (q1@ [v2_of e])) \<subseteq> set (edges_of_path q)" 
+           using 7(2-) edges_of_path_append_subset_2 by fastforce
+         moreover have a5:"to_dbltn e \<notin> set (edges_of_path (q1@ [v2_of e]))" 
+           using  distinct_edges_q by(unfold 7(2) edges_of_path_symmetric_split to_dbltn_sym) auto
+         ultimately have a6:"set (edges_of_path (q1@ [v2_of e])) \<subseteq> (to_dbltn `(t_set S))" 
+           using a3 graph_abs.path_ball_edges' graph_abs_with_e walk_between_nonempty_pathD(1) by fastforce
+         have "walk_betw (to_dbltn `(t_set S)) (v1_of e) (q1@ [v2_of e]) (v2_of e)"  
+           using walk_betw_strengthen[OF a3 _ a6] 7(3) by simp
+         thus ?case
+           using 7(1) by simp 
+       next
+         case (8 a list aa lista)
+         hence a1:"walk_betw (to_dbltn ` insert e (t_set S)) u (q1 @ [v2_of e]) (v2_of e)"
+           using q_prop(1) by (intro walk_pref[of _ u q1 "v2_of e" "v1_of e # q2" u]) force
+         moreover have a2:"walk_betw (to_dbltn ` insert e (t_set S)) (v1_of e) (v1_of e # q2) u"
+           using q_prop(1) 8(2)  by(intro walk_suff[of _ u "q1@[v2_of e]" "v1_of e" q2 u]) force     
+         have a4:"set (edges_of_path (q1@ [v2_of e])) \<subseteq> set (edges_of_path q)" 
+           using 8(2-) edges_of_path_append_subset_2 by fastforce
+         moreover have a5:"to_dbltn e \<notin> set (edges_of_path (q1@ [v2_of e]))" 
+           using  distinct_edges_q by(unfold 8(2) edges_of_path_symmetric_split to_dbltn_sym) simp
+         ultimately have a6:"set (edges_of_path (q1@ [v2_of e])) \<subseteq> (to_dbltn `(t_set S))" 
+           using graph_abs.path_ball_edges' graph_abs_with_e walk_between_nonempty_pathD(1) by fastforce
+         have a4:"set (edges_of_path ([v1_of e] @ q2)) \<subseteq> set (edges_of_path q)"
+           using 8(2) edges_of_path_append_subset by fastforce
+         moreover have a5:"to_dbltn e \<notin> set (edges_of_path ([v1_of e] @ q2))" 
+           using 8(4) distinct_edges_q by(unfold 8(2) edges_of_path_symmetric_split to_dbltn_sym) simp 
+         moreover have a3:"walk_betw (to_dbltn ` insert e (t_set S)) (v1_of e) ([v1_of e] @ q2) u"
+           using a2 a1 by simp 
+         ultimately have a7:"set (edges_of_path ([v1_of e] @ q2)) \<subseteq> (to_dbltn `(t_set S))"
+           using  a1 a2 graph_abs.path_ball_edges' graph_abs_with_e walk_between_nonempty_pathD(1) by fast 
+         have "walk_betw (to_dbltn `(t_set S)) u (q1@ [v2_of e]) (v2_of e)"  
+           using walk_betw_strengthen 8(3) a1 a6 by fastforce
+         moreover have "walk_betw (to_dbltn `(t_set S)) (v1_of e) ( [v1_of e]@q2)u"  
+           using walk_betw_strengthen 8(3)  8(4) a3 a7 by fastforce
+         ultimately have  "walk_betw (to_dbltn `(t_set S)) (v1_of e) ( ([v1_of e]@q2@(tl q1)@[v2_of e])) (v2_of e)" 
+           using 8(3) walk_transitive_2 by fastforce
+         then show ?case using 8(1) by auto
+       qed
+       have  dfs_vwalk:"vwalk_bet (dfs.Graph.digraph_abs (local.Kruskal_E_to_G S)) (v1_of e) q' (v2_of e)"
+         apply(subst same_dgraphabs, subst Pair_Graph_U_RBT.ugraph_abs_digraph_abs[symmetric])
+         using local.Kruskal_E_to_G_def pair_graph_u_invar apply simp
+         using  graph_abs.walk_betw_iff_vwalk_bet[OF graph_abs_without_e]  path_without_e 
+         by (simp  add: ugraph_abs_is )
+       obtain q'' where "vwalk_bet (dfs.Graph.digraph_abs (local.Kruskal_E_to_G S)) (v1_of e) q'' (v2_of e)"
+                             "distinct q''" 
+         using  vwalk_bet_to_distinct_is_distinct_vwalk_bet[OF dfs_vwalk]
+         by(auto simp add: distinct_vwalk_bet_def)
+       thus False 
+         using no_distinct_path by blast
+     qed
+   next
+     case 2
+     note two = this
+     show ?case 
+     proof(cases "lookup (local.Kruskal_E_to_G S) (v2_of e)")
+       case None 
+       hence "lookup (local.Kruskal_E_to_G S) (v1_of e) = None" 
+         using two(2) by blast
+       thus False 
+         by (simp add: one)
+     next
+       case (Some neighbs)
+       hence dfs_reachable:"return
+         (dfs.DFS (local.Kruskal_E_to_G S) (\<lambda> w. w= v2_of e) (DFS.initial_state vset_insert vset_empty (v1_of e))) =
+             Reachable" 
+         using two(2) return.exhaust by auto
+       then obtain p where p_vwalk:"vwalk_bet (dfs.Graph.digraph_abs (local.Kruskal_E_to_G S)) (v1_of e)
+                                      p (v2_of e) \<or>
+         stack (dfs.DFS (local.Kruskal_E_to_G S) (\<lambda> w. w = v2_of e) (DFS.initial_state vset_insert vset_empty (v1_of e))) =
+             [v1_of e] \<and> v1_of e = (v2_of e)"
+         using DFS_thms.DFS_correct_2[OF DFS_thms[OF one(1)]] dfs_reachable by auto
+       have walk_betw_around_e:"walk_betw (to_dbltn ` t_set S) (v1_of e) p (v2_of e)"
+         apply(subst  ugraph_abs_is[symmetric], subst graph_abs.walk_betw_iff_vwalk_bet, simp add: graph_abs_without_e ugraph_abs_is)
+         using  pair_graph_u_invar  p_vwalk v1_never_v2
+         by(auto simp add: Pair_Graph_U_RBT.ugraph_abs_digraph_abs same_dgraphabs Kruskal_E_to_G_def)
+       have "epath (to_dbltn ` t_set S) (v1_of e) (edges_of_path p) (v2_of e)" 
+         by(auto intro!: graph_abs.walk_betw_imp_epath simp add: walk_betw_around_e graph_abs_without_e)
+       moreover then obtain p' where p'_prop:"map to_dbltn p' = edges_of_path p" "set p' \<subseteq>  (t_set S)"
+         using undirected_multigraph.edges_of_path_to_multigraph_path[OF epath_edges_subset]
+         by blast 
+       ultimately have epath_first_path:"epath (to_dbltn `  (t_set S)) (v1_of e) (map to_dbltn p') (v2_of e)"  
+         by simp
+       then obtain p'' where p''_prop:"epath (to_dbltn ` t_set S) (v1_of e) p'' (v2_of e)" 
+                       "set p'' \<subseteq> set (map to_dbltn p')" "distinct p''"
+         using  epath_distinct_epath by fast
+       obtain p_mul where p_mul: "map to_dbltn p_mul = p''" "set p_mul \<subseteq> set p'"
+         using p''_prop(2) map_eq_Cons_conv by(induction p'')  fastforce+
+       hence epath_p_mul:"epath (to_dbltn ` t_set S) (v1_of e) (map to_dbltn p_mul) (v2_of e)"
+         using p''_prop(1) by blast
+       hence epath_first_path:"epath (to_dbltn ` (insert e (t_set S))) (v1_of e) (map to_dbltn p_mul) (v2_of e)"  
+         by (auto intro: epath_subset image_mono subset_insertI)
+       moreover have "epath (to_dbltn ` (insert e (t_set S))) (v2_of e) [to_dbltn e] (v1_of e)" 
+         using v1_never_v2[of e] by(auto intro!: epath_single)
+       ultimately have epath3:"epath (to_dbltn ` (insert e (t_set S))) (v1_of e) 
+                              (map to_dbltn (p_mul@[e])) (v1_of e)" 
+         by (auto intro: epath_append)
+       moreover have "set (p_mul@[e]) \<subseteq> insert e (t_set S)" 
+         using p'_prop(2) p_mul(2) by auto
+       moreover have "2 \<le> length (p_mul@[e])" 
+         using epath_non_empty[OF epath_p_mul, simplified length_map] 
+         by (simp add: v1_never_v2)
+       moreover have "distinct (p_mul@[e])" 
+       proof-
+         have "distinct p_mul"
+           using p_mul(1)  p''_prop(3) by (auto simp add: distinct_map)
+         moreover have "set p_mul \<subseteq> t_set S" 
+           using p'_prop(2) p_mul(2) by order
+         ultimately show ?thesis using assms(4) by auto
+       qed
+       ultimately have "undirected_multigraph.decycle_multi (t_set (vset_insert e (id S))) (v1_of e) (p_mul@[e])" 
+          by (simp add: undirected_multigraph.decycle_multi_def  case_assms(1) dfs.Graph.vset.set.set_insert)
+        thus ?thesis 
+         using 2(1) by simp
+     qed
+   qed
+ next
+   case 2
+   have "(\<nexists>u. Ex (undirected_multigraph.decycle_multi (t_set (vset_insert e (id S))) u))"
+   proof(rule ccontr,goal_cases)
+     case 1
+     then obtain u C where uC:"undirected_multigraph.decycle_multi (insert e (t_set S)) u C"
+       using case_assms(1) dfs.Graph.vset.set.set_insert by fastforce
+     hence C_prop: "epath (to_dbltn ` insert e (t_set S)) u (map to_dbltn C) u"
+                    "set C \<subseteq> insert e (t_set S)" " 2 \<le> length C" "distinct C"
+       using uC[simplified undirected_multigraph.decycle_multi_def] by auto
+     have e_in_C:"e \<in> set C"
+     proof(rule ccontr, goal_cases)
+       case 1
+       hence "undirected_multigraph.decycle_multi (t_set S) u C"
+         using uC epath_subset_other_set[of "(to_dbltn ` insert e (t_set S))" 
+                    u "map to_dbltn C" u "to_dbltn ` (t_set S)"] 
+         by (simp add: image_mono subset_insert undirected_multigraph.decycle_multi_def)
+       then show ?case 
+         using assms(2)  case_assms(2)
+         by(auto simp add:  Kruskal_Greedy.indep_graph_matroid_def 
+                            local.indep_graph_matroid_def undirected_multigraph.has_no_cycle_multi_def)
+     qed
+     obtain C1 C2 where C1C2:"C = C1@[e]@C2"
+       by (metis append_Cons append_Nil e_in_C in_set_conv_decomp_first)
+     hence epath_extended:"epath  (to_dbltn ` insert e (t_set S)) u (map to_dbltn (C1@[e]@C2@C1@[e]@C2@C1@[e]@C2)) u"
+       using epath_append C_prop(1)[simplified C1C2] by fastforce
+     have middle_three_rewrite:"xs@[x,y,z]@ys = (xs@[x])@[y]@(z#ys)" for x y z xs ys by auto
+     have e_path_very_verbose: "epath (to_dbltn ` insert e (t_set S)) u
+ (butlast (map to_dbltn (C1 @ [e] @ C2 @ C1)) @
+  [last (map to_dbltn (C1 @ [e] @ C2 @ C1)), to_dbltn e, hd (map to_dbltn (C2 @ C1 @ [e] @ C2))] @
+  tl (map to_dbltn (C2 @ C1 @ [e] @ C2))) u"
+       using epath_extended
+       apply(rule back_subst[of "\<lambda> p. epath _ _ p _ "])
+       apply(subst middle_three_rewrite) 
+       apply(subst append_butlast_last_id, simp)
+       apply(subst hd_Cons_tl,simp)
+       by auto
+     have "\<exists>x y. to_dbltn e = {x, y} \<and>
+      x \<noteq> y \<and>
+      epath (to_dbltn ` insert e (t_set S)) u
+       (butlast (map to_dbltn (C1 @ [e] @ C2 @ C1)) @ [last (map to_dbltn (C1 @ [e] @ C2 @ C1))]) x \<and>
+      epath (to_dbltn ` insert e (t_set S)) y
+       ([hd (map to_dbltn (C2 @ C1 @ [e] @ C2))] @ tl (map to_dbltn (C2 @ C1 @ [e] @ C2))) u \<and>
+      x \<in> last (map to_dbltn (C1 @ [e] @ C2 @ C1)) \<inter> to_dbltn e \<and>
+      y \<in> to_dbltn e \<inter> hd (map to_dbltn (C2 @ C1 @ [e] @ C2))"
+       using epath_find_splitter_advanced[OF e_path_very_verbose] by simp
+     then obtain x y where xy_prop:"to_dbltn e = {x, y}"
+      "x \<noteq> y"
+      "epath (to_dbltn ` insert e (t_set S)) u (map to_dbltn (C1 @ [e] @ C2 @ C1)) x"
+      "epath (to_dbltn ` insert e (t_set S)) y (map to_dbltn (C2 @ C1 @ [e] @ C2)) u"
+      "x \<in> last (map to_dbltn (C1 @ [e] @ C2 @ C1)) \<inter> to_dbltn e"
+      "y \<in> to_dbltn e \<inter> hd (map to_dbltn (C2 @ C1 @ [e] @ C2))" 
+       by(subst (asm) append_butlast_last_id, simp) force
+     have C1C2_empt:"C2@C1 \<noteq> []" 
+       using C1C2 C_prop(3) by force
+     define d1 where "d1 = last (C1 @ [e] @ C2 @ C1)"
+     have d1_def': "d1 = last (C2@C1)"
+       using C1C2_empt d1_def by auto
+     define d2 where "d2 = hd  (C2 @ C1 @ [e] @ C2)"
+     have d2_def': "d2 = hd (C2@C1)" 
+       using C1C2_empt  by(auto simp add: d2_def hd_append)
+     have xy_prop':"x \<in> to_dbltn d1 \<inter> to_dbltn e"
+                   "y \<in> to_dbltn e \<inter> to_dbltn d2" 
+       using xy_prop(5,6)
+       by(all \<open>subst (asm) last_map, simp\<close>, all \<open>subst (asm) hd_map, simp\<close>)
+          (auto simp add: d2_def d1_def)
+     have last_in:"d1 \<in> set C"
+       using C1C2   by(subst d1_def, intro set_rev_mp[OF last_in_set,of _  "set C"]) auto
+     have hd_in:"d2 \<in> set C"
+       using C1C2   by(subst d2_def, intro set_rev_mp[OF hd_in_set,of _  "set C"]) auto
+     have  d1_prop:"d1 \<in> set C" "to_dbltn e \<inter> to_dbltn d1 \<noteq> {}" 
+       using last_in xy_prop(1,5) by(all \<open>subst (asm) last_map, simp\<close>)(auto simp add: d1_def)
+     have  d2_prop:"d2 \<in> set C" "to_dbltn e \<inter> to_dbltn d2 \<noteq> {}" 
+       using hd_in xy_prop(1,6) by(all \<open>subst (asm) hd_map, simp\<close>)(auto simp add: d2_def)
+     have "d1 \<in> insert e (t_set S)" 
+       using C_prop(2) last_in by blast
+     moreover  have d1_not_e:"d1 \<noteq> e"
+     proof(rule ccontr, goal_cases)
+       case 1
+       hence "e \<in> set (C2@C1)"
+         using C1C2_empt d1_def' last_in_set by blast
+       hence "\<not> distinct C"
+         using C1C2 by fastforce
+       then show ?case
+         by (simp add: C_prop(4))
+     qed
+     ultimately have d1_in_S:"d1 \<in>  (t_set S)" 
+       by simp
+     have  "d2 \<in> insert e (t_set S)" 
+       using C_prop(2) hd_in by blast
+     moreover have d2_not_e:"d2 \<noteq> e"
+     proof(rule ccontr, goal_cases)
+       case 1
+       hence "e \<in> set (C2@C1)"
+         using C1C2_empt d2_def' hd_in_set by blast
+       hence "\<not> distinct C"
+         using C1C2 by fastforce
+       then show ?case
+         by (simp add: C_prop(4))
+     qed
+     ultimately have d2_in_S: "d2 \<in> (t_set S)" by simp
+
+     have dir_ds_in:"(v1_of d1, v2_of d1) \<in> G.digraph_abs (local.Kruskal_E_to_G S)"
+          "(v2_of d1, v1_of d1) \<in> G.digraph_abs (local.Kruskal_E_to_G S)"
+          "(v1_of d2, v2_of d2) \<in> G.digraph_abs (local.Kruskal_E_to_G S)"
+          "(v2_of d2, v1_of d2) \<in> G.digraph_abs (local.Kruskal_E_to_G S)"
+       by (simp add: d1_in_S d2_in_S digraph_abs_is)+
+     have graph_inv:"G.graph_inv (local.Kruskal_E_to_G S)" 
+       using local.Kruskal_E_to_G_def pair_graph_u_invar by force
+     have "lookup (local.Kruskal_E_to_G S) (v1_of e) \<noteq> None" 
+       using dir_ds_in  d1_prop(2) d2_prop(2) 2 d1_not_e d2_not_e  C1C2_empt  isin.simps(1)  xy_prop(1) xy_prop' 
+       apply(cases "lookup (local.Kruskal_E_to_G S) (v1_of d1)")
+       apply(all \<open>cases "lookup (local.Kruskal_E_to_G S) (v2_of d1)"\<close>)
+       apply(all \<open>cases "lookup (local.Kruskal_E_to_G S) (v1_of d2)"\<close>)
+       apply(all \<open>cases "lookup (local.Kruskal_E_to_G S) (v2_of d2)"\<close>)
+       apply(simp add: doubleton_eq_iff  G.neighbourhood_def Pair_Graph_RBT.G.are_connected_abs[OF graph_inv, symmetric])+
+       by metis
+     moreover have "lookup (local.Kruskal_E_to_G S) (v2_of e) \<noteq> None"
+       using dir_ds_in  d1_prop(2) d2_prop(2) 2 d1_not_e d2_not_e  C1C2_empt  isin.simps(1)  xy_prop(1) xy_prop' 
+       apply(cases "lookup (local.Kruskal_E_to_G S) (v1_of d1)")
+       apply(all \<open>cases "lookup (local.Kruskal_E_to_G S) (v2_of d1)"\<close>)
+       apply(all \<open>cases "lookup (local.Kruskal_E_to_G S) (v1_of d2)"\<close>)
+       apply(all \<open>cases "lookup (local.Kruskal_E_to_G S) (v2_of d2)"\<close>)
+       apply(simp add: doubleton_eq_iff  G.neighbourhood_def Pair_Graph_RBT.G.are_connected_abs[OF graph_inv, symmetric])+
+       by metis+
+     ultimately show ?case
+       using "2" by auto
+   qed
+   thus ?case 
+     using "2" by blast
+ qed
+qed
+  show ?case 
+    using second_eq dfs.Graph.vset.set.set_insert[OF assms(1)]
+    by (cases "rbt_subseteq (vset_insert e S) input_G ", 
+       unfold local_indep_oracle_def undirected_multigraph_spec.has_no_cycle_multi_def first_eq ) 
+       (auto simp add: Kruskal_Greedy.indep_graph_matroid_def local.indep_graph_matroid_def
+                        undirected_multigraph.has_no_cycle_multi_def)
 qed
 
-term Kruskal_Graphs_Matroids.graph_to_edges
-
-definition "cost_nonnegative (c::(('v set) \<Rightarrow> rat)) = ( \<forall>e. c e \<ge> 0)"
-
-term Kruskal_Graphs_Matroids.graph_to_edges
-term Kruskal_Graphs_Matroids.edges_to_graph
-
-
-context
-    fixes c :: "('a set) \<Rightarrow> rat" and c' :: "'e \<Rightarrow> rat"
+context fixes c::"'e \<Rightarrow> rat" and  order::"'e list"
+  assumes non_negative_c:"\<And> e. e \<in> t_set input_G \<Longrightarrow> c e \<ge> 0"
+and order_is_G: "t_set input_G = set order"
+and order_length_is_G_card: "distinct order"
 begin
 
+lemma best_in_greedy_axioms:"Best_In_Greedy.BestInGreedy_axioms vset_inv t_set set_of_sets_isin input_G
+     (Kruskal_Greedy.indep_graph_matroid v1_of v2_of input_G)"
+    by(auto simp add:  Matroid_Specs_Inst.invar_def local.indep_graph_matroid_def set_of_sets_isin_def
+      Best_In_Greedy.BestInGreedy_axioms_def[OF Kruskal_Greedy.Kruskal_Greedy.Best_In_Greedy_axioms] 
+      G_good Kruskal_Greedy.indep_graph_matroid_def Matroid_Specs_Inst.indep_def
+      Matroid_Specs_Inst.finite_setsI)
 
-lemma (* TODO instantiate assms directly using thms from encoding locale, maybe take the statement "further"*)
-  indep_graph_matroid_expr_1:
-  assumes "Pair_Graph_U_RBT.pair_graph_u_invar (Kruskal_E_to_G  (E::('e::linorder) rbt))" 
-          "rbt_inv (Kruskal_E_to_V   E)"
-    "Tree2.set_tree (Kruskal_E_to_V   E) =
-            dVs (Pair_Graph_U_RBT.digraph_abs (Kruskal_E_to_G   E))"
-  shows "indep_graph_matroid  E =
-    (rbt_subseteq E (carrier_graph_matroid ) \<and>
- \<not>(\<exists>u c. decycle (Pair_Graph_U_RBT.ugraph_abs (Kruskal_E_to_G  E)) u c))"
-  apply (subst indep_graph_matroid.simps)
-  apply (subst Let_def)+
-  apply (subst DFS_Cycles_correct_final[OF assms]) by presburger
+lemma sort_desc_axioms: "Best_In_Greedy.sort_desc_axioms Kruskal_Greedy.carrier_sorted"
+  by (simp add: Kruskal_Greedy.sort_desc_axioms_def insort_key_desc_stable
+ length_insort_key_desc set_insort_key_desc sorted_desc_f_insort_key_desc)
 
-lemma
-  indep_graph_matroid_expr_2:
-  assumes "rbt_inv (E::('e::linorder) rbt)"
-  shows "indep_graph_matroid  E =
-    (rbt_subseteq E (carrier_graph_matroid ) \<and> 
-\<not>(\<exists>u c. decycle (Pair_Graph_U_RBT.ugraph_abs (Kruskal_E_to_G E)) u c))"
-  using indep_graph_matroid_expr_1[of "E", unfolded Kruskal_E_to_G_def Kruskal_E_to_V_def]
-    Kruskal_Graphs_Matroids_Proofs.edges_invar_imp_graph_invar[OF assms]
-    Kruskal_Graphs_Matroids_Proofs.edges_invar_imp_vertices_props[OF assms]
-  by(unfold Kruskal_E_to_G_def  edges_to_graph_def edges_to_vertices_def) blast
-  
-
-term Kruskal_Greedy.valid_solution 
-term Kruskal_Greedy.nonnegative 
-term Kruskal_Greedy.valid_order
-
-thm Kruskal_Greedy.BestInGreedy_correct_1
-thm Kruskal_Greedy.BestInGreedy_correct_3
-thm Kruskal_Greedy.BestInGreedy_matroid_iff_opt
-
-
-
-term Matroid_Specs_Inst.indep
-term indep_graph_matroid
-
-lemma carrier_graph_matroid_inv:
-  assumes "Pair_Graph_U_RBT.pair_graph_u_invar input_G"
-  shows "rbt_inv  (carrier_graph_matroid)"
-  using Kruskal_Graphs_Matroids_Proofs.graph_invar_imp_edges_invar[OF assms] 
-  by(unfold carrier_graph_matroid_def graph_to_edges_def)
-
-lemma Kruskal_Greedy_indep':
-  "Kruskal_Greedy.indep'  v1_of v2_of edge_of input_G (X::('e \<times> color) tree) =
- indep_graph_matroid X"
-  using Matroid_Specs_Inst.indep_def set_of_sets_isin_def
-  by (metis indep_graph_matroid_def)
-
-lemma indep_graph_matroid_abs_equal:
-  assumes "Pair_Graph_U_RBT.pair_graph_u_invar input_G" "rbt_inv X" "rbt_inv Y" "Tree2.set_tree X = Tree2.set_tree Y"
-  shows "indep_graph_matroid  X
-           = indep_graph_matroid  Y"
-proof-
-  have "rbt_subseteq X (carrier_graph_matroid) =
-        rbt_subseteq Y (carrier_graph_matroid )"
-    using rbt_subseteq_correct[OF \<open>rbt_inv X\<close> carrier_graph_matroid_inv[OF assms(1)]]
-    rbt_subseteq_correct[OF \<open>rbt_inv Y\<close> carrier_graph_matroid_inv[OF assms(1)]] assms(4)
-    by blast
-  with Kruskal_Graphs_Matroids_Proofs.to_set_equal_imp_ugraph_abs_equal[OF assms(2-4)]
-  show "indep_graph_matroid  X =
-        indep_graph_matroid  Y"
-    apply (subst indep_graph_matroid_expr_2[OF \<open>rbt_inv X\<close>])
-    apply (subst indep_graph_matroid_expr_2[OF \<open>rbt_inv Y\<close>])
-    unfolding Kruskal_E_to_G_def edges_to_graph_def using arg_cong2 .
-qed
-lemma Kruskal_BestInGreedy_axioms:
-  assumes "Pair_Graph_U_RBT.pair_graph_u_invar input_G"
-  shows "Best_In_Greedy.BestInGreedy_axioms rbt_inv Tree2.set_tree set_of_sets_isin 
-  (carrier_graph_matroid) (indep_graph_matroid )"
-  unfolding Kruskal_Greedy.BestInGreedy_axioms_def Matroid_Specs_Inst.invar_def
-    Matroid_Specs_Inst.finite_sets_def
-proof-
-  from carrier_graph_matroid_def Kruskal_Graphs_Matroids_Proofs.graph_invar_imp_edges_invar[OF assms]
-    have "rbt_inv  (carrier_graph_matroid )" 
-      using assms carrier_graph_matroid_inv by blast
-  with indep_graph_matroid_abs_equal[OF assms] Kruskal_Greedy_indep' finite_set_tree
-  have "(rbt_inv  (carrier_graph_matroid ) \<and>
-    (\<forall>X Y. rbt_inv X \<longrightarrow> rbt_inv Y \<longrightarrow> Tree2.set_tree X = Tree2.set_tree Y \<longrightarrow>
-      indep'  v1_of v2_of edge_of input_G X =
-      indep'  v1_of v2_of edge_of input_G Y)) \<and>
-    (\<forall>X. finite (Tree2.set_tree X))" by blast
-  thus ?thesis 
-    by (metis (mono_tags, lifting) Best_In_Greedy.BestInGreedy_axioms_def Kruskal_Greedy.Best_In_Greedy_axioms Matroid_Specs_Inst.finite_sets_def Matroid_Specs_Inst.invar_def indep_graph_matroid_def)
+lemma indep_system_axioms:"Matroid_Specs_Inst.indep_system_axioms input_G
+             (Kruskal_Greedy.indep_graph_matroid v1_of v2_of input_G)"
+  unfolding  Matroid_Specs_Inst.indep_system_axioms_def
+proof(rule conjI[OF _ conjI], goal_cases)
+  case 1
+  then show ?case 
+  by(simp add: rbt_subseteq_correct[OF _ G_good, symmetric]
+           Matroid_Specs_Inst.indep_def Kruskal_Greedy.indep_graph_matroid_def
+             indep_graph_matroid_def undirected_multigraph.has_no_cycle_multi_def
+             set_of_sets_isin_def) 
+next
+  case 2
+  show ?case
+    using undirected_multigraph.empty_has_no_cycle_multi_indep 
+    by(auto intro!: exI[of _ Leaf] 
+         simp add: Kruskal_Greedy.wrapper_axioms(5) Matroid_Specs_Inst.indep_def 
+                   Kruskal_Greedy.indep_graph_matroid_def indep_graph_matroid_def set_of_sets_isin_def
+                    local.undirected_multigraph.empty_has_no_cycle_multi_indep)
+next
+  case 3
+  show ?case
+    unfolding Matroid_Specs_Inst.indep_def Kruskal_Greedy.indep_graph_matroid_def indep_graph_matroid_def
+              set_of_sets_isin_def
+  proof(rule+, goal_cases)
+    case (1 X Y)
+    show ?case 
+      using 1(1,2,4) Custom_Set_RBT.set_subseteq 
+      by (auto intro:  undirected_multigraph.has_no_cycle_multi_indep_subset[OF 1(3)])
+  qed
 qed
 
+lemma nonnegative:" Kruskal_Greedy.nonnegative input_G c"
+  by(auto simp add: Kruskal_Greedy.nonnegative_def Pair_Graph_RBT.set.set_isin G_good  non_negative_c )
 
-lemma Kruskal_sort_desc_axioms:
-  "Best_In_Greedy.sort_desc_axioms Kruskal_Greedy.carrier_sorted"
-  unfolding Kruskal_Greedy.sort_desc_axioms_def
-  using set_insort_key_desc length_insort_key_desc sorted_desc_f_insort_key_desc insort_key_desc_stable
-  by metis
+lemma size_G_length_order:"size input_G = length order"
+  by(simp add:  G_good  Kruskal_Greedy.rbt_size_correct distinct_card order_is_G order_length_is_G_card)
 
+lemma valid_order: "Kruskal_Greedy.valid_order input_G order"
+  by(simp add: Kruskal_Greedy.valid_order_def Pair_Graph_RBT.set.set_isin G_good  non_negative_c 
+                  size_G_length_order order_is_G)
 
-context
-  assumes pair_graph_u: "Pair_Graph_U_RBT.pair_graph_u_invar input_G"
-begin
-
-lemmas carrier_inv = carrier_graph_matroid_inv[OF pair_graph_u]
-
-(*
-interpretation input_G_graph_abs: graph_abs
-  where G = "Pair_Graph_U_RBT.ugraph_abs input_G"
-  using Pair_Graph_U_RBT.graph_abs_ugraph[OF pair_graph_u] by simp
-
-interpretation (Pair_Graph_U_RBT.ugraph_abs (Kruskal_E_to_G carrier_graph_matroid))
-*)
-(*
-lemma carrier_converted_back:
-  "Kruskal_E_to_G carrier_graph_matroid = input_G"
-  unfolding Kruskal_E_to_G_def carrier_graph_matroid_def 
-  using Kruskal_Graphs_Matroids_Proofs.graph_to_edges_inverse[OF pair_graph_u] by simp
-*)
-
-lemma carrier_converted_graph_abs:
-  "graph_abs (Pair_Graph_U_RBT.ugraph_abs 
-(Kruskal_E_to_G  ( carrier_graph_matroid )))"
-  using (*carrier_converted_back*) Pair_Graph_U_RBT.graph_abs_ugraph[OF pair_graph_u]
-  sorry
-(* Put this into interpretation or not? *)
-
-lemma indep_graph_matroid_expr_3:
-  assumes "rbt_inv (E::('e::linorder) rbt)"
-  shows "indep_graph_matroid  E = 
-    graph_abs.has_no_cycle (Pair_Graph_U_RBT.ugraph_abs 
-(Kruskal_E_to_G  (carrier_graph_matroid)))
-    (Pair_Graph_U_RBT.ugraph_abs (Kruskal_E_to_G  E))"
-  unfolding graph_abs.has_no_cycle_def[OF carrier_converted_graph_abs]
-  (* (rbt_subseteq E carrier_graph_matroid \<and> \<not>(\<exists>u c. decycle (Pair_Graph_U_RBT.ugraph_abs (Kruskal_E_to_G E)) u c)) *)
-proof-
-  from indep_graph_matroid_expr_2[OF assms]
-  have "indep_graph_matroid  E =
-    (rbt_subseteq E (carrier_graph_matroid ) \<and>
-    (\<nexists>u c. decycle (Pair_Graph_U_RBT.ugraph_abs (Kruskal_E_to_G  E)) u c))" by blast
-  also have "... = 
-    (Pair_Graph_U_RBT.ugraph_abs (Kruskal_E_to_G  E) \<subseteq>
- Pair_Graph_U_RBT.ugraph_abs (Kruskal_E_to_G  (carrier_graph_matroid )) \<and>
-    (\<nexists>u c. decycle (Pair_Graph_U_RBT.ugraph_abs (Kruskal_E_to_G  E)) u c))"
-    unfolding Kruskal_E_to_G_def
-    using Kruskal_Graphs_Matroids_Proofs.subset_iff_graph_to_edges_subset[OF assms carrier_inv]
-    sorry
-  finally show "indep_graph_matroid  E =
-    (Pair_Graph_U_RBT.ugraph_abs (Kruskal_E_to_G  E) \<subseteq>
- Pair_Graph_U_RBT.ugraph_abs (Kruskal_E_to_G (carrier_graph_matroid )) \<and>
-     (\<nexists>u c. decycle (Pair_Graph_U_RBT.ugraph_abs (Kruskal_E_to_G  E)) u c))" .
+lemma kruskal_impl_corespondence: 
+  "to_ordinary (kruskal' v1_of v2_of input_G (kruskal_init' c order)) =
+  kruskal v1_of v2_of input_G (kruskal_init c order)"
+proof(rule Kruskal_Greedy.BestInGreedy'_corresp, goal_cases)
+  case (1 S x)
+  then show ?case 
+    by(unfold Kruskal_Greedy.local_indep_oracle_def, intro local_indep_oracle_correct) auto
+next
+  case 2
+  then show ?case 
+    by (simp add: G_good)
+next
+  case 3
+  then show ?case
+    by (simp add: best_in_greedy_axioms) 
+next
+  case 4
+  then show ?case 
+    by (simp add: sort_desc_axioms)
+next
+  case 5
+  then show ?case
+    by (simp add: indep_system_axioms)
+next
+  case 6
+  then show ?case
+    by (simp add: nonnegative)
+next
+  case 7
+  then show ?case
+    by (simp add: valid_order)
 qed
 
+lemma indep_finite: "undirected_multigraph_spec.has_no_cycle_multi to_dbltn (t_set input_G) X \<Longrightarrow> finite X"
+  using Spanning_Trees.undirected_multigraph.graph_indep_system_multi indep_system.indep_finite
+ undirected_multigraph.undirected_multigraph_axioms by fast
 
-(* TODO maybe generalise some parts of these theorems? *)
-term indep'
-lemma Kruskal_indep'_eq_has_no_cycle:
-  assumes "rbt_inv (X::('e::linorder) rbt)"
-  shows "indep' v1_of v2_of edge_of input_G X = graph_abs.has_no_cycle 
-(Pair_Graph_U_RBT.ugraph_abs (Kruskal_E_to_G  (carrier_graph_matroid )))
-    (Pair_Graph_U_RBT.ugraph_abs (Kruskal_E_to_G  X))"
-  using Kruskal_Greedy_indep' indep_graph_matroid_expr_3[OF assms] by blast
+lemma idnep_in_G:"undirected_multigraph_spec.has_no_cycle_multi to_dbltn (t_set input_G) X \<Longrightarrow>
+           x \<in> X \<Longrightarrow> x \<in> t_set input_G"
+  using local.undirected_multigraph.has_no_cycle_multi_indep_subset_carrier by auto
 
-lemma Kruskal_indep_subset_carrier:
-  assumes "rbt_inv (X::('e::linorder) rbt)" "indep' v1_of v2_of edge_of input_G X"
-  shows "rbt_subseteq X (carrier_graph_matroid )"
-proof-
-  from assms(2) Kruskal_Greedy_indep' indep_graph_matroid_expr_3[OF assms(1)]
-  have "graph_abs.has_no_cycle (Pair_Graph_U_RBT.ugraph_abs 
-(Kruskal_E_to_G (carrier_graph_matroid )))
-    (Pair_Graph_U_RBT.ugraph_abs (Kruskal_E_to_G  X))" by blast
-  then have "Pair_Graph_U_RBT.ugraph_abs (Kruskal_E_to_G  X) \<subseteq>
-    Pair_Graph_U_RBT.ugraph_abs (Kruskal_E_to_G  (carrier_graph_matroid ))"
-    using graph_abs.has_no_cycle_indep_subset_carrier[OF carrier_converted_graph_abs] by blast
-  then have "Tree2.set_tree X \<subseteq> Tree2.set_tree ((carrier_graph_matroid ))"
-    unfolding Kruskal_E_to_G_def
-    using Kruskal_Graphs_Matroids_Proofs.edges_to_graph_subset_imp_subset[OF \<open>rbt_inv X\<close> carrier_inv]
-    sorry
-  with Custom_Set_RBT.set_subseteq[OF \<open>rbt_inv X\<close> carrier_inv]
-    show "rbt_subseteq X (carrier_graph_matroid )" by blast
-qed
+lemma indep_system_order:"indep_system (set order) (undirected_multigraph_spec.has_no_cycle_multi to_dbltn (set order))"
+  using local.undirected_multigraph.graph_indep_system_multi[of input_G] order_is_G by auto
 
-lemma Kruskal_indep_ex:
-  "(\<exists>X. rbt_inv (X::('e::linorder) rbt) \<and> indep' v1_of v2_of edge_of input_G X)"
-proof-
-  from graph_abs.has_no_cycle_indep_ex[OF carrier_converted_graph_abs]
-  obtain G where "graph_abs.has_no_cycle (Pair_Graph_U_RBT.ugraph_abs 
-(Kruskal_E_to_G  (carrier_graph_matroid ))) G"
-    by blast
-  from graph_abs.has_no_cycle_indep_subset_carrier[OF carrier_converted_graph_abs this]
-    have "G \<subseteq> (Pair_Graph_U_RBT.ugraph_abs (Kruskal_E_to_G  (carrier_graph_matroid )))"
-      sorry
-  from graph_abs_mono[OF carrier_converted_graph_abs this]
-    have "graph_abs G" by blast
-    obtain G_impl where G_impl_invar: "Pair_Graph_U_RBT.pair_graph_u_invar G_impl" and
-      G_impl_abs: "Pair_Graph_U_RBT.ugraph_abs G_impl = G"
-      sorry
+interpretation use_greedy_thms_kruskal:
+Use_Greedy_Thms Leaf vset_insert vset_delete isin t_set vset_inv vset_union
+                               vset_inter vset_diff rbt_subseteq  size set_of_sets_isin 
+"undirected_multigraph_spec.has_no_cycle_multi (\<lambda> e. {v1_of e, v2_of e})(Tree2.set_tree input_G)"
+input_G c order Kruskal_Greedy.carrier_sorted
+  by(intro Use_Greedy_Thms.intro 
+                      undirected_multigraph.graph_indep_system_multi indep_finite idnep_in_G)
+    (auto intro!: Use_Greedy_Thms_axioms.intro
+       simp add: Matroid_Specs_Inst.Matroid_Specs_axioms[simplified Matroid_Specs_def]
+                       set_of_sets_isin_def' G_good non_negative_c order_is_G
+                      indep_system_order indep_finite undirected_multigraph_spec.has_no_cycle_multi_def
+                      order_length_is_G_card sort_desc_axioms)
 
-  (* If G satisfies ugraph_abs, there exists an impl graph satisfying pair_graph_u such that ugraph_abs (G_impl) = *)
+lemma kruskal_returns_basis: "indep_system.basis (t_set input_G) 
+(undirected_multigraph_spec.has_no_cycle_multi to_dbltn (t_set input_G))
+ (t_set (result (kruskal v1_of v2_of input_G (kruskal_init c order))))"
+  by(simp add:  kruskal_def Kruskal_Greedy.indep_graph_matroid_def local.indep_graph_matroid_def 
+                kruskal_init_def use_greedy_thms_kruskal.algo_gives_basis )
 
-  from Kruskal_Graphs_Matroids_Proofs.graph_invar_imp_edges_invar[OF \<open>Pair_Graph_U_RBT.pair_graph_u_invar G_impl\<close>]
-    have "rbt_inv (Kruskal_Graphs_Matroids.graph_to_edges edge_of G_impl)" sorry
+corollary kruskal_returns_spanning_forest: 
+"undirected_multigraph_spec.is_spanning_forest_multi to_dbltn (t_set input_G)
+ (t_set (result (kruskal v1_of v2_of input_G (kruskal_init c order))))"
+  apply(subst undirected_multigraph.spanning_forest_iff_basis_multi)
+  by(rule kruskal_returns_basis)
 
+lemma rank_quotient_one: "indep_system.rank_quotient (t_set input_G)
+    (undirected_multigraph_spec.has_no_cycle_multi to_dbltn (t_set input_G)) = 1"
+  apply(subst Matroids_Theory.indep_system.matroid_iff_rq_eq_1[symmetric])
+  by (auto simp add: use_greedy_thms_kruskal.indep_system 
+                undirected_multigraph.graph_matroid_multi)
 
-  from \<open>graph_abs.has_no_cycle (Pair_Graph_U_RBT.ugraph_abs (Kruskal_E_to_G (carrier_graph_matroid ))) G\<close> G_impl_abs
-    have "graph_abs.has_no_cycle (Pair_Graph_U_RBT.ugraph_abs (Kruskal_E_to_G (carrier_graph_matroid )))
-      (Pair_Graph_U_RBT.ugraph_abs (Kruskal_E_to_G (Kruskal_Graphs_Matroids.graph_to_edges edge_of G_impl)))"
-    unfolding Kruskal_E_to_G_def sorry
-   (* apply (subst Kruskal_Graphs_Matroids_Proofs.graph_to_edges_inverse[OF G_impl_invar])
-    by (metis Kruskal_E_to_G_def carrier_converted_back)*)
+theorem kruskal_is_max:
+"undirected_multigraph_spec.has_no_cycle_multi to_dbltn (t_set input_G) X \<Longrightarrow>
+sum c X \<le> sum c (t_set (result (kruskal v1_of v2_of input_G (kruskal_init c order))))"
+  unfolding kruskal_def kruskal_init_def Kruskal_Greedy.indep_graph_matroid_def
+            local.indep_graph_matroid_def
+  apply(rule order.trans[rotated])
+  apply(rule use_greedy_thms_kruskal.indep_predicate_greedy_correct[of X])
+  by(simp add:  rank_quotient_one)+
 
-  with Kruskal_Greedy_indep' indep_graph_matroid_expr_3[OF \<open>rbt_inv (Kruskal_Graphs_Matroids.graph_to_edges edge_of G_impl)\<close>]
-    (* \<open>graph_abs.has_no_cycle (Pair_Graph_U_RBT.ugraph_abs (Kruskal_E_to_G carrier_graph_matroid)) G\<close>
-    \<open>Pair_Graph_U_RBT.ugraph_abs G_impl = G\<close>
-    Kruskal_Graphs_Matroids.graph_to_edges_inverse[OF G_impl_invar] *)
-    have "Kruskal_Greedy.indep' v1_of v2_of edge_of input_G (Kruskal_Graphs_Matroids.graph_to_edges edge_of G_impl)" by blast
-  with \<open>rbt_inv (Kruskal_Graphs_Matroids.graph_to_edges edge_of G_impl)\<close>
-    show ?thesis by blast
-qed
+definition "max_forest X =
+ (undirected_multigraph_spec.is_spanning_forest_multi to_dbltn (t_set input_G) X
+\<and> (\<forall> Y. undirected_multigraph_spec.is_spanning_forest_multi to_dbltn (t_set input_G) Y \<longrightarrow>
+     sum c Y \<le> sum c X))"
 
-
-lemma Kruskal_indep_subset:
-  assumes "rbt_inv X" "rbt_inv Y" "indep' v1_of v2_of edge_of input_G X" "rbt_subseteq Y X"
-  shows "indep' v1_of v2_of edge_of input_G Y"
-proof-
-  from Kruskal_indep'_eq_has_no_cycle[OF assms(1)] assms(3)
-  have no_cycle: "graph_abs.has_no_cycle
- (Pair_Graph_U_RBT.ugraph_abs (Kruskal_E_to_G (carrier_graph_matroid)))
-      (Pair_Graph_U_RBT.ugraph_abs (Kruskal_E_to_G X))" by blast
-  have X_subset_Y: "Pair_Graph_U_RBT.ugraph_abs (Kruskal_E_to_G Y) \<subseteq>
-    Pair_Graph_U_RBT.ugraph_abs (Kruskal_E_to_G X)"
-   (* using Kruskal_Graphs_Matroids_Proofs.subset_iff_graph_to_edges_subset[OF assms(2,1), of v1_of v2_of]
-    assms(4) by(force simp add: Kruskal_E_to_G_def) *) sorry
-  from graph_abs.has_no_cycle_indep_subset[OF carrier_converted_graph_abs no_cycle X_subset_Y]
-  have "graph_abs.has_no_cycle (Pair_Graph_U_RBT.ugraph_abs
- (Kruskal_E_to_G  (carrier_graph_matroid)))
-      (Pair_Graph_U_RBT.ugraph_abs (Kruskal_E_to_G Y))" by blast
-  with Kruskal_indep'_eq_has_no_cycle[OF \<open>rbt_inv Y\<close>]
-    show ?thesis by blast
-qed
-
-lemma Kruskal_augment:
-  assumes "rbt_inv X" "rbt_inv Y" "indep' v1_of v2_of edge_of input_G X" 
-"indep' v1_of v2_of edge_of input_G Y" "size X = Suc (size Y)"
-shows "(\<exists>x. Pair_Graph_U_RBT.isin' x (RBT.diff X Y) \<and>
- indep' v1_of v2_of edge_of input_G (insert_rbt x Y))"
-proof-
-  from Kruskal_indep'_eq_has_no_cycle[OF assms(1)] assms(3)
-  have no_cycle_X: "graph_abs.has_no_cycle (Pair_Graph_U_RBT.ugraph_abs
- (Kruskal_E_to_G  (carrier_graph_matroid )))
-      (Pair_Graph_U_RBT.ugraph_abs (Kruskal_E_to_G X))" by blast
-  from Kruskal_indep'_eq_has_no_cycle[OF assms(2)] assms(4)
-  have no_cycle_Y: "graph_abs.has_no_cycle (Pair_Graph_U_RBT.ugraph_abs
- (Kruskal_E_to_G  (carrier_graph_matroid )))
-      (Pair_Graph_U_RBT.ugraph_abs (Kruskal_E_to_G  Y))" by blast
-
-  from Kruskal_Graphs_Matroids_Proofs.card_graph_to_edges[OF \<open>rbt_inv X\<close>]
-     Kruskal_Graphs_Matroids_Proofs.card_graph_to_edges[OF \<open>rbt_inv Y\<close>] assms(5)
-
-  have card_rel: "card (Pair_Graph_U_RBT.ugraph_abs (Kruskal_E_to_G  X)) 
-= Suc (card (Pair_Graph_U_RBT.ugraph_abs (Kruskal_E_to_G  Y))) "
-    unfolding Kruskal_E_to_G_def sorry
-
-  from graph_abs.has_no_cycle_augment[OF carrier_converted_graph_abs no_cycle_X no_cycle_Y card_rel]
-  obtain x where "x \<in> Pair_Graph_U_RBT.ugraph_abs (Kruskal_E_to_G X) 
-- Pair_Graph_U_RBT.ugraph_abs (Kruskal_E_to_G  Y)"
-      "graph_abs.has_no_cycle (Pair_Graph_U_RBT.ugraph_abs (Kruskal_E_to_G  
-(carrier_graph_matroid )))
-       (Set.insert x (Pair_Graph_U_RBT.ugraph_abs (Kruskal_E_to_G  Y)))" by blast
-find_theorems Pair_Graph_U_RBT.ugraph_abs Kruskal_E_to_G
-   (* TODO HERE !! *)
-  show ?thesis
-    apply(subst Kruskal_indep'_eq_has_no_cycle) sorry
-qed
-
-
-lemma Kruskal_indep_system_axioms:
-  "Matroid_Specs_Inst.indep_system_axioms (carrier_graph_matroid ) 
-(indep_graph_matroid)"
-  apply (subst Matroid_Specs_Inst.indep_system_axioms_def)
-  using Kruskal_indep_subset_carrier Kruskal_indep_ex Kruskal_indep_subset
-  by (smt (verit) indep_graph_matroid_def)
-
-lemma Kruskal_matroid_axioms:
-  "Matroid_Specs_Inst.matroid_axioms (carrier_graph_matroid )
- (indep_graph_matroid )"
-  apply (subst Matroid_Specs_Inst.matroid_axioms_def)
-  using Kruskal_indep_system_axioms Kruskal_augment
-  by (metis (no_types, lifting) indep_graph_matroid_def)
-
+corollary kruskal_computes_max_spanning_forest:
+"max_forest(t_set (result (kruskal v1_of v2_of input_G (kruskal_init c order))))"
+  using kruskal_is_max kruskal_returns_spanning_forest 
+  by(auto simp add: max_forest_def undirected_multigraph.is_spanning_forest_multi_def)
+end
+end
 end
 
 
-(* thm Kruskal_Greedy.BestInGreedy_correct_1[OF Kruskal_BestInGreedy_axioms] *)
-(*thm Kruskal_Greedy.BestInGreedy_correct_1[OF Kruskal_BestInGreedy_axioms Kruskal_sort_desc_axioms Kruskal_indep_system_axioms]
-*)
-(* TODO NOW INSTANTIATE INDEP SYSTEM AXIOMS, CONNECT FINAL THEOREM 
-\<Rightarrow> assumptions on c and order can be left as-is for now *)
+definition "v1_of (e::(nat\<times>nat)) = min (fst e) (snd e)"
+definition "v2_of e = (if fst e = snd e then fst e + 1 else  max (fst e) (snd e))"
 
-
-
-(* !! TODO here assumption !! *)
-(*
-interpretation G_edges_abs: graph_abs
-  where G = "Pair_Graph_U_RBT.ugraph_abs input_G"
-  using Pair_Graph_U_RBT.graph_abs_ugraph[OF pair_graph_u] by simp
-*)
-
-term Kruskal_Greedy.initial_state 
-
-(* TODO define Kruskal_MST, maybe should parametrise with graph and define outside of context? \<Rightarrow> or parametrise
-with c and order? \<Longrightarrow> Don't need to put this function in context, only use use context when pair graph property
-is actually necessary
-\<Rightarrow> maybe parametrise with c and order? *)
-(*
-fun Kruskal_MST :: "(('v::linorder) * ('v rbt)) rbt" where
-  "Kruskal_MST = Kruskal_E_to_G (best_in_greedy_state.result (Kruskal_Greedy.BestInGreedy (Kruskal_Greedy.initial_state c order)))"
-*)
-find_theorems "_::_ itself"
-
-abbreviation "BestInGreedy == Kruskal_Greedy.BestInGreedy "
-
-fun Kruskal_MST :: "('e::linorder list) \<Rightarrow> (('a::linorder) * ('a rbt)) rbt" where
-  "Kruskal_MST order =
-    Kruskal_E_to_G  (
-best_in_greedy_state.result
- (Kruskal_Greedy.BestInGreedy (TYPE ('a)) v1_of v2_of edge_of input_G  
-(Kruskal_Greedy.initial_state c' order)))"
-
-context
-  assumes pair_graph_u: "Pair_Graph_U_RBT.pair_graph_u_invar input_G"
-begin
-
-interpretation G_edges_abs: graph_abs
-  where G = "Pair_Graph_U_RBT.ugraph_abs input_G"
-  using Pair_Graph_U_RBT.graph_abs_ugraph[OF pair_graph_u] by simp
-
-(* thm spanning_tree_def *)
-thm G_edges_abs.is_spanning_forest_def
-(*
-thm Kruskal_Greedy.BestInGreedy_correct_3[OF Kruskal_BestInGreedy_axioms[OF pair_graph_u]
-    Kruskal_sort_desc_axioms Kruskal_indep_system_axioms[OF pair_graph_u]]
-*)
-lemma Kruskal_Greedy_valid_inst:
-  assumes "Kruskal_Greedy.nonnegative (TYPE ('a)) edge_of inut_G c'" 
-"Kruskal_Greedy.valid_order (TYPE ('a)) edge_of input_G order"
-shows "Kruskal_Greedy.valid_solution (TYPE ('a)) edge_of input_G v1_of v2_of
- (result (Kruskal_Greedy.BestInGreedy (TYPE ('a)) v1_of v2_of edge_of input_G
- (Kruskal_Greedy.initial_state c' order)))"
-(*proof-
-  from Kruskal_Greedy.BestInGreedy_correct_1[OF Kruskal_BestInGreedy_axioms[OF pair_graph_u]
-    Kruskal_sort_desc_axioms Kruskal_indep_system_axioms[OF pair_graph_u], OF assms]
-  show ?thesis by metis
-qed*) sorry
-
-lemma Kruskal_Greedy_opt_inst:
-  assumes "Kruskal_Greedy.nonnegative (TYPE ('a)) edge_of input_G c'" 
-"Kruskal_Greedy.valid_order (TYPE ('a)) edge_of input_G order"
- "Kruskal_Greedy.valid_solution (TYPE ('a)) edge_of input_G v1_of v2_of X"
-  shows "sum c' (Tree2.set_tree X) \<le> sum c'
-           (Tree2.set_tree (result (Kruskal_Greedy.BestInGreedy (TYPE ('a))
-           v1_of v2_of edge_of input_G (Kruskal_Greedy.initial_state c' order))))"
-proof-
- (* from Kruskal_Greedy.BestInGreedy_matroid_iff_opt[OF Kruskal_BestInGreedy_axioms[OF pair_graph_u]
-    Kruskal_sort_desc_axioms Kruskal_indep_system_axioms[OF pair_graph_u]]
-    Kruskal_matroid_axioms[OF pair_graph_u]
-    assms Kruskal_Greedy.c_set_def*)
-  have "Kruskal_Greedy.c_set c' (Tree2.set_tree X) \<le>
-    Kruskal_Greedy.c_set c' (Tree2.set_tree (result
- (Kruskal_Greedy.BestInGreedy  (TYPE ('a))
-           v1_of v2_of edge_of input_G (Kruskal_Greedy.initial_state c' order))))"
-    sorry
-  with Kruskal_Greedy.c_set_def show ?thesis by metis
+interpretation kruskal_proof_maitroid_edges: Kruskal_Proof_Matroid_Edges v2_of G v1_of for G
+proof(rule  Kruskal_Proof_Matroid_Edges.intro, unfold v1_of_def v2_of_def, goal_cases)
+  case (1 e)
+  then show ?case 
+    by(cases "fst e = snd e") auto
 qed
 
+definition "edges = [(0::nat, 1::nat), (0, 2), (2, 3), (2,4), (2,1), (1,5), (5,8), (8,7), (7,1),
+                     (7,2), (7,4), (4,3), (3,4), (3,3), (9, 8), (8, 1), (4,5), (5,10), (10,5), (10,1)]"
 
+definition "G = foldr (\<lambda> x tree. vset_insert x  tree) edges empty"
 
-lemma nonneg_conv:
-  "cost_nonnegative c \<Longrightarrow> Kruskal_Greedy.nonnegative (TYPE ('a)) edge_of input_G c'"
-  sorry
+definition "c_list = [((0::nat, 1::nat), 1::rat), ((0, 2), 0.5), ((2, 3), 5/8), ((2,4), 3), ((2,1), -1/3),
+                      ((1,5), 4), ((5,8), 2), ((8,7), 0.1), ((7,1), 1.3),
+                     ((7,2), 3), ((7,4), 3), ((4,3), 2), ((3,4), 1), ((3,3), 0), ((9, 8),2.5),
+                      ((8, 1), 0), ((4,5), 2), ((5,10), 3), ((10,5), 30), ((10,1), 1000)]"
 
+definition "c_impl = foldr (\<lambda> xy tree. update (prod.fst xy) (prod.snd xy) tree) c_list Leaf"
+value "c_impl"
 
-lemma Kruskal_correct_final_1:
-  assumes "cost_nonnegative c" "Kruskal_Greedy.valid_order (TYPE ('a)) 
-edge_of input_G order" (* WRONG ASSUMPTIONS !! *)
-  shows "G_edges_abs.is_spanning_forest (Pair_Graph_U_RBT.ugraph_abs (Kruskal_MST order))"
-  sorry
- 
+definition "costs  e =  (case (lookup c_impl e) of Some c \<Rightarrow> c | None \<Rightarrow> 0)"
 
-thm Kruskal_matroid_axioms[OF pair_graph_u]
-(*thm Kruskal_Greedy.BestInGreedy_matroid_iff_opt[OF Kruskal_BestInGreedy_axioms[OF pair_graph_u]
-    Kruskal_sort_desc_axioms Kruskal_indep_system_axioms[OF pair_graph_u]]
-*)
-term "(Pair_Graph_U_RBT.ugraph_abs (Kruskal_MST order))"
-lemma Kruskal_correct_final_2:
-  assumes "cost_nonnegative c" "Kruskal_Greedy.valid_order (TYPE ('a)) edge_of input_G order" (* WRONG ASSUMPTIONS !! *)
-    (* introduce new nonnegative predicate, maybe find some way to get order based on existing stuff or assume 
-    function*)
-    "Pair_Graph_U_RBT.pair_graph_u_invar G'"
-    "Pair_Graph_U_RBT.ugraph_abs G' \<subseteq> Pair_Graph_U_RBT.ugraph_abs input_G"
-    "G_edges_abs.is_spanning_forest (Pair_Graph_U_RBT.ugraph_abs G')"
-  (* shows "sum c (Pair_Graph_U_RBT.ugraph_abs (Kruskal_MST c order)) \<le> sum c (Pair_Graph_U_RBT.ugraph_abs G')"  *)
-  shows "sum c (Pair_Graph_U_RBT.ugraph_abs (Kruskal_MST order)) \<le>
- sum c (Pair_Graph_U_RBT.ugraph_abs G')"
-proof-
-  from \<open>G_edges_abs.is_spanning_forest (Pair_Graph_U_RBT.ugraph_abs G')\<close>
-    have "graph_abs.has_no_cycle (Pair_Graph_U_RBT.ugraph_abs input_G) (Pair_Graph_U_RBT.ugraph_abs G')"
-    unfolding G_edges_abs.is_spanning_forest_def by blast
+value "kruskal_init' costs edges"
+value  "kruskal' v1_of v2_of G (kruskal_init' costs edges)"
+value "inorder (result (kruskal' v1_of v2_of G (kruskal_init' costs edges)))"
 
-  thm indep_graph_matroid_expr_3[OF pair_graph_u]
-
- (* thm Kruskal_Greedy.BestInGreedy_matroid_iff_opt[OF Kruskal_BestInGreedy_axioms Kruskal_sort_desc_axioms
-      Kruskal_indep_system_axioms] pair_graph_u
-*)
-  have valid_soln: "Kruskal_Greedy.valid_solution (TYPE ('a)) edge_of input_G v1_of v2_of 
-          (Kruskal_G_to_E G')" sorry
-  from Kruskal_Greedy_opt_inst[OF nonneg_conv[OF assms(1)] assms(2) valid_soln]
-  have "sum c' (Tree2.set_tree (Kruskal_G_to_E G'))
-    \<le> sum c' (Tree2.set_tree (result (Kruskal_Greedy.BestInGreedy (TYPE ('a)) v1_of v2_of edge_of input_G 
-(Kruskal_Greedy.initial_state c' order))))"
-    by blast
-  then have
-      "sum c (Pair_Graph_U_RBT.ugraph_abs (Kruskal_E_to_G  (Kruskal_G_to_E G')))
-    \<ge> sum c (Pair_Graph_U_RBT.ugraph_abs (Kruskal_E_to_G 
- (result (Kruskal_Greedy.BestInGreedy (TYPE ('a)) v1_of v2_of edge_of input_G (Kruskal_Greedy.initial_state c' order)))))"
-   (*   using Kruskal_Graphs_Matroids_Proofs.costs_transformation[where E' ="(Kruskal_G_to_E G')" and
-          E'' = "(result (Kruskal_Greedy.BestInGreedy (Kruskal_Greedy.initial_state c' order)))"]
-    by blast*) sorry
-  then
-    show "sum c (Pair_Graph_U_RBT.ugraph_abs (Kruskal_MST order)) \<le> sum c (Pair_Graph_U_RBT.ugraph_abs G')"
-    using Kruskal_Graphs_Matroids_Proofs.graph_to_edges_inverse[OF \<open>Pair_Graph_U_RBT.pair_graph_u_invar G'\<close>]
-    using Kruskal_E_to_G_def sorry
-qed
-  
-
-
-end
-
-end
-end
-(* Example: Edge is implemented as pair of vertices where first element is always less than or equal
-to second element *)
-definition edge_of :: "('v::linorder) \<Rightarrow> 'v \<Rightarrow> ('v \<times> 'v)" where
-  "edge_of u v = (if u \<le> v then (u, v) else (v, u))"
-
-definition v1_of :: "('v \<times> 'v) \<Rightarrow> ('v::linorder)" where
-  "v1_of e = fst e"
-
-definition v2_of :: "('v \<times> 'v) \<Rightarrow> ('v::linorder)" where
-  "v2_of e = snd e"
-(*
-definition "Kruskal_MST' input_G c' order = Kruskal_MST input_G v1_of v2_of edge_of c' order"
-*)
-(*
-definition c where "c e = 0"
-
-definition order where "order = []"
-
-value "Kruskal_MST' (Leaf::((nat \<times> nat rbt) rbt)) c order"
-*)
-
-
+thm kruskal_proof_maitroid_edges.kruskal_computes_max_spanning_forest
 end
