Spanning_Trees/Kruskal_Greedy_old.thy
@@ -1,0 +1,934 @@
+theory Kruskal_Greedy
+  imports Matroids_Greedy.Best_In_Greedy Spanning_Trees Graph_Algorithms.DFS_Cycles_Aux
+    Graph_Algorithms.DFS_Cycles Insertion_Sort_Desc Graphs_Matroids_Encoding
+    "HOL-Data_Structures.Set2_Join_RBT" "HOL-Data_Structures.RBT_Map" "HOL-Library.Product_Lexorder"
+begin
+
+
+subsection \<open>Instantiations for Kruskal's algorithm\<close>
+
+abbreviation "rbt_inv == ( \<lambda>t. (invc t \<and> invh t) \<and> Tree2.bst t)"
+
+fun rbt_sel where
+  "rbt_sel Leaf = undefined"
+| "rbt_sel (Node _ (a,_) _) = a"
+
+lemma rbt_sel_correct:
+  "t \<noteq> empty \<Longrightarrow> rbt_sel t \<in> (set o inorder) t"
+  by (induction t) (auto simp: empty_def)
+
+interpretation Set_Choose_RBT: Set_Choose
+  where empty = "\<langle>\<rangle>" and insert = insert_rbt and delete = delete_rbt and
+    isin = isin and t_set = "Tree2.set_tree" and invar = "rbt_inv::(('v::linorder) rbt \<Rightarrow> bool)" and
+    sel = rbt_sel
+  apply(simp add: Set_Choose_def)
+  apply(intro conjI)
+  subgoal
+    using RBT.Set_axioms[unfolded] by(auto simp add: S.set_def S.invar_def)
+  subgoal apply unfold_locales subgoal for s by (cases s) (auto dest!: rbt_sel_correct)
+  done
+  done
+
+
+interpretation Pair_Graph_U_RBT: Pair_Graph_U_Specs
+  where empty = RBT_Set.empty and update = update and delete = RBT_Map.delete and
+    lookup = lookup and adjmap_inv = "M.invar" and vset_empty = "\<langle>\<rangle>" and
+    insert = insert_rbt and vset_delete = delete_rbt and vset_inv = "rbt_inv::(('v::linorder) rbt \<Rightarrow> bool)" and
+    isin = isin and t_set = "Tree2.set_tree" and sel = rbt_sel
+  apply(simp add: Pair_Graph_U_Specs_def Pair_Graph_Specs_def)
+  using M.Map_axioms Set_Choose_RBT.Set_Choose_axioms by simp
+
+interpretation DFS_Aux_Interp: DFS_Aux
+  where empty = RBT_Set.empty and update = update and delete = RBT_Map.delete and
+    lookup = lookup and adjmap_inv = "M.invar" and vset_empty = "\<langle>\<rangle>" and
+    insert = insert_rbt and vset_delete = delete_rbt and vset_inv = "rbt_inv::(('v::linorder) rbt \<Rightarrow> bool)" and
+    isin = isin and t_set = "Tree2.set_tree" and union = "RBT.union" and inter = "RBT.inter" and 
+    diff = "RBT.diff" and sel = rbt_sel for G and s
+  apply(simp add: DFS_Aux_def)
+  using Pair_Graph_U_RBT.Pair_Graph_Specs_axioms RBT.Set2_axioms by auto
+
+abbreviation "DFS_Aux' G s \<equiv> DFS_Aux_Interp.DFS_Aux G (DFS_Aux_Interp.initial_state s)"
+
+interpretation DFS_Cycles_Interp: DFS_Cycles
+  where empty = RBT_Set.empty and update = update and delete = RBT_Map.delete and
+    lookup = lookup and adjmap_inv = "M.invar" and vset_empty = "\<langle>\<rangle>" and
+    insert = insert_rbt and vset_delete = delete_rbt and vset_inv = "rbt_inv::(('v::linorder) rbt \<Rightarrow> bool)" and
+    isin = isin and t_set = "Tree2.set_tree" and union = "RBT.union" and inter = "RBT.inter" and 
+    diff = "RBT.diff" and sel = rbt_sel and seen_aux = "DFS_Aux_state.seen" and cycle_aux = "DFS_Aux_state.cycle" and
+    dfs_aux = "DFS_Aux' G" for G and V
+  apply(simp add: DFS_Cycles_def)
+  using Pair_Graph_U_RBT.Pair_Graph_Specs_axioms RBT.Set2_axioms by auto
+
+lemma DFS_Aux_correct_1_inst:
+  assumes "DFS_Cycles.DFS_Cycles_axioms isin Tree2.set_tree M.invar \<langle>\<rangle> rbt_inv lookup G V"
+    "s \<in> dVs (Pair_Graph_U_RBT.digraph_abs G)"
+  shows "DFS_Aux_state.cycle (DFS_Aux' G s) \<Longrightarrow> \<exists>c. cycle' (Pair_Graph_U_RBT.digraph_abs G) c"
+  using assms[simplified DFS_Cycles_Interp.DFS_Cycles_axioms_def[of "G" "V"]]
+    DFS_Aux_Interp.DFS_Aux_correct_1[unfolded DFS_Aux_Interp.DFS_Aux_axioms_def]
+  by blast
+
+lemma DFS_Aux_correct_2_inst:
+  assumes "DFS_Cycles.DFS_Cycles_axioms isin Tree2.set_tree M.invar \<langle>\<rangle> rbt_inv lookup G V"
+    "s \<in> dVs (Pair_Graph_U_RBT.digraph_abs G)"
+  shows "\<not>DFS_Aux_state.cycle (DFS_Aux' G s) \<Longrightarrow>
+    \<nexists>c. cycle' (Pair_Graph_U_RBT.digraph_abs G \<downharpoonright> Tree2.set_tree (DFS_Aux_state.seen (DFS_Aux' G s))) c"
+  using assms[simplified DFS_Cycles_Interp.DFS_Cycles_axioms_def[of "G" "V"]]
+    DFS_Aux_Interp.DFS_Aux_correct_2[unfolded DFS_Aux_Interp.DFS_Aux_axioms_def]
+  by blast
+
+lemma DFS_Aux_correct_3_inst:
+  assumes "DFS_Cycles.DFS_Cycles_axioms isin Tree2.set_tree M.invar \<langle>\<rangle> rbt_inv lookup G V"
+    "s \<in> dVs (Pair_Graph_U_RBT.digraph_abs G)"
+  shows "\<not>DFS_Aux_state.cycle (DFS_Aux' G s) \<Longrightarrow> v \<in> Tree2.set_tree (DFS_Aux_state.seen (DFS_Aux' G s)) \<Longrightarrow>
+    w \<in> dVs (Pair_Graph_U_RBT.digraph_abs G) - Tree2.set_tree (DFS_Aux_state.seen (DFS_Aux' G s)) \<Longrightarrow>
+    \<nexists>p. awalk (Pair_Graph_U_RBT.digraph_abs G) v p w"
+  using assms[simplified DFS_Cycles_Interp.DFS_Cycles_axioms_def[of "G" "V"]]
+    DFS_Aux_Interp.DFS_Aux_correct_3[unfolded DFS_Aux_Interp.DFS_Aux_axioms_def]
+  by blast
+
+lemma DFS_Aux_correct_4_inst:
+  assumes "DFS_Cycles.DFS_Cycles_axioms isin Tree2.set_tree M.invar \<langle>\<rangle> rbt_inv lookup G V"
+    "s \<in> dVs (Pair_Graph_U_RBT.digraph_abs G)"
+  shows "rbt_inv (DFS_Aux_state.seen (DFS_Aux' G s))"
+  using assms[simplified DFS_Cycles_Interp.DFS_Cycles_axioms_def[of "G" "V"]]
+    DFS_Aux_Interp.DFS_Aux_correct_4[unfolded DFS_Aux_Interp.DFS_Aux_axioms_def]
+  by blast
+
+lemma DFS_Aux_correct_5_inst:
+  assumes "DFS_Cycles.DFS_Cycles_axioms isin Tree2.set_tree M.invar \<langle>\<rangle> rbt_inv lookup G V"
+    "s \<in> dVs (Pair_Graph_U_RBT.digraph_abs G)"
+  shows "v \<in> Tree2.set_tree (DFS_Aux_state.seen (DFS_Aux' G s)) \<Longrightarrow>
+    \<exists>p. awalk (Pair_Graph_U_RBT.digraph_abs G) s p v"
+  using assms[simplified DFS_Cycles_Interp.DFS_Cycles_axioms_def[of "G" "V"]]
+    DFS_Aux_Interp.DFS_Aux_correct_5[unfolded DFS_Aux_Interp.DFS_Aux_axioms_def]
+  by blast
+
+lemma DFS_Aux_correct_6_inst:
+  assumes "DFS_Cycles.DFS_Cycles_axioms isin Tree2.set_tree M.invar \<langle>\<rangle> rbt_inv lookup G V"
+    "s \<in> dVs (Pair_Graph_U_RBT.digraph_abs G)"
+  shows "s \<in> Tree2.set_tree (DFS_Aux_state.seen (DFS_Aux' G s))"
+  using assms[simplified DFS_Cycles_Interp.DFS_Cycles_axioms_def[of "G" "V"]]
+    DFS_Aux_Interp.DFS_Aux_correct_6[unfolded DFS_Aux_Interp.DFS_Aux_axioms_def]
+  by blast
+
+
+lemma DFS_Cycles_imp_dfs_aux_axioms:
+  assumes "DFS_Cycles.DFS_Cycles_axioms isin Tree2.set_tree M.invar \<langle>\<rangle> rbt_inv lookup G V"
+  shows "DFS_Cycles.dfs_aux_axioms isin Tree2.set_tree \<langle>\<rangle> rbt_inv lookup G (DFS_Aux' G) DFS_Aux_state.seen DFS_Aux_state.cycle"
+  unfolding DFS_Cycles_Interp.dfs_aux_axioms_def
+  using DFS_Aux_correct_1_inst[OF assms] DFS_Aux_correct_2_inst[OF assms] DFS_Aux_correct_3_inst[OF assms]
+    DFS_Aux_correct_4_inst[OF assms] DFS_Aux_correct_5_inst[OF assms] DFS_Aux_correct_6_inst[OF assms]
+  by meson
+
+
+thm DFS_Cycles_Interp.DFS_Cycles_correct_1
+
+(* If Pair_Graph_U_invar holds + relationship between G and V, we have cycle iff cycle in ugraph_abs *)
+
+abbreviation "DFS_Cycles' G V \<equiv> DFS_Cycles_Interp.DFS_Cycles V G DFS_Cycles_Interp.initial_state"
+
+thm Pair_Graph_U_RBT.pair_graph_u_invar_def
+thm DFS_Cycles.DFS_Cycles_axioms_def
+
+lemma DFS_Cycles_correct_final:
+  assumes "Pair_Graph_U_RBT.pair_graph_u_invar G" "rbt_inv V"
+    "Tree2.set_tree (V::(('a::linorder) rbt)) = dVs (Pair_Graph_U_RBT.digraph_abs G)"
+  shows "DFS_Cycles_state.cycle (DFS_Cycles' G V) = (\<exists>u c. decycle (Pair_Graph_U_RBT.ugraph_abs G) u c)"
+proof-
+  have "DFS_Cycles.DFS_Cycles_axioms isin Tree2.set_tree M.invar \<langle>\<rangle> rbt_inv lookup G V"
+    unfolding DFS_Cycles_Interp.DFS_Cycles_axioms_def 
+    using assms[simplified Pair_Graph_U_RBT.pair_graph_u_invar_def[of "G"]]
+      Pair_Graph_U_RBT.digraph_abs_irreflexive[OF assms(1)]
+      Pair_Graph_U_RBT.digraph_abs_symmetric[OF assms(1)] by fastforce
+
+  from DFS_Cycles_Interp.DFS_Cycles_correct_1[OF this DFS_Cycles_imp_dfs_aux_axioms[OF this]]
+    DFS_Cycles_Interp.DFS_Cycles_correct_2[OF this DFS_Cycles_imp_dfs_aux_axioms[OF this]]
+    have "DFS_Cycles_state.cycle (DFS_Cycles' G V) = (\<exists>c. cycle' (Pair_Graph_U_RBT.digraph_abs G) c)"
+    by blast
+  with Pair_Graph_U_RBT.cycle_equivalence[OF assms(1)]
+  show "DFS_Cycles_state.cycle (DFS_Cycles' G V) = (\<exists>u c. decycle (Pair_Graph_U_RBT.ugraph_abs G) u c)"
+    by blast
+qed
+
+
+text \<open>Instantiations for Greedy\<close>
+
+lemma tree_split_case:
+  "(case t of Leaf \<Rightarrow> True | _ \<Rightarrow> False) = (t = Leaf)"
+  by (fastforce split: tree.splits) 
+
+fun rbt_subseteq :: "('a::linorder) rbt \<Rightarrow> 'a rbt \<Rightarrow> bool" where
+  "rbt_subseteq t1 t2 = (case (RBT.diff t1 t2) of Leaf \<Rightarrow> True | _ \<Rightarrow> False)"
+
+lemma rbt_subseteq_correct:
+  "rbt_inv t1 \<Longrightarrow> rbt_inv t2 \<Longrightarrow> (rbt_subseteq t1 t2) = (Tree2.set_tree t1 \<subseteq> Tree2.set_tree t2)"
+proof(unfold rbt_subseteq.simps tree.split[of "\<lambda> x. x= (_ \<subseteq> _)" True "\<lambda> _ _ _. False" "RBT.diff t1 t2" ],
+      goal_cases)
+  case 1
+  have is_empty_iff:"RBT.diff t1 t2 = \<langle>\<rangle> \<longleftrightarrow> Tree2.set_tree t1 - Tree2.set_tree t2 = {}"
+    using 1  Tree2.eq_set_tree_empty 
+    by (subst RBT.set_tree_diff[of t1 t2, symmetric])fast+
+  show ?case 
+    using is_empty_iff by (subst Diff_eq_empty_iff[symmetric])fastforce
+qed
+
+lemma rbt_size_correct:
+  "rbt_inv X \<Longrightarrow> size X = card (Tree2.set_tree X)"
+  unfolding set_inorder[symmetric]
+proof(induction X rule: inorder.induct)
+  case 1
+  then show ?case by simp
+next
+  case (2 l a uu r)
+  have inter_empty:"set (Tree2.inorder l) \<inter> Set.insert a (set (Tree2.inorder r)) = {}"
+    using 2(3) bst.simps(2)[simplified Tree2.set_inorder[symmetric]]
+    by (metis Int_emptyI insert_iff not_less_iff_gr_or_eq)
+  have rbt_inv_l: "rbt_inv l" 
+    by (metis "2.prems" RBT.inv_Node bst.simps(2))
+  have rbt_inv_r: "rbt_inv r" 
+    by (metis "2.prems" RBT.inv_Node bst.simps(2))
+  have a_not_down: "a \<notin> set (Tree2.inorder r)" 
+    using 2(3) bst.simps(2)[simplified Tree2.set_inorder[symmetric]] by fast
+  show ?case 
+   using a_not_down inter_empty 
+   by(auto  simp add: card_Un_disjoint card_insert_if  2(1)[OF rbt_inv_l] 2(2)[OF rbt_inv_r])
+qed
+
+interpretation Custom_Set_RBT: Custom_Set
+  where empty = "\<langle>\<rangle>" and insert = insert_rbt and delete = delete_rbt and invar = "rbt_inv::(('e::linorder) rbt \<Rightarrow> bool)" and
+    isin = isin and set = "Tree2.set_tree" and union = "RBT.union" and inter = "RBT.inter" and diff = "RBT.diff" and
+    subseteq = rbt_subseteq and cardinality = size
+  apply (subst Custom_Set_def)
+  apply(intro conjI)
+  subgoal
+    using RBT.Set2_axioms by blast
+  subgoal
+    apply (subst Custom_Set_axioms_def)
+    using rbt_subseteq_correct rbt_size_correct by blast
+  done
+
+
+definition "set_of_sets_isin f a = f a"
+
+interpretation Matroid_Specs_Inst: Matroid_Specs
+  where set_empty = "\<langle>\<rangle>" and set_insert = insert_rbt and set_delete = delete_rbt and set_inv = "rbt_inv::(('e::linorder) rbt \<Rightarrow> bool)" and
+    set_isin = isin and to_set = "Tree2.set_tree" and union = "RBT.union" and inter = "RBT.inter" and diff = "RBT.diff" and
+    subseteq = rbt_subseteq and cardinality = size and
+    set_of_sets_isin = "set_of_sets_isin :: ('e rbt \<Rightarrow> bool) \<Rightarrow> 'e rbt \<Rightarrow> bool"
+  apply (subst Matroid_Specs_def)
+  apply (subst Indep_System_Specs_def)
+  using Custom_Set_RBT.Custom_Set_axioms by blast
+
+term "DFS_Cycles'"
+
+
+fun rbt_set_fold :: "'a rbt \<Rightarrow> ('a \<Rightarrow> 'b \<Rightarrow> 'b) \<Rightarrow> 'b \<Rightarrow> 'b" where
+  "rbt_set_fold Leaf f acc = acc"
+| "rbt_set_fold (Node l (a, _) r) f acc = rbt_set_fold r f (f a (rbt_set_fold l f acc))"
+
+lemma rbt_set_fold_revinorder: "rbt_set_fold T f acc = foldr f (rev (inorder T)) acc"
+ by(induction T f acc rule: rbt_set_fold.induct) auto
+
+fun rbt_map_fold :: "('a \<times> 'd) rbt \<Rightarrow> ('a \<Rightarrow> 'd \<Rightarrow> 'b \<Rightarrow> 'b) \<Rightarrow> 'b \<Rightarrow> 'b" where
+  "rbt_map_fold Leaf f acc = acc"
+| "rbt_map_fold (Node l ((a, d), _) r) f acc = rbt_map_fold r f (f a d (rbt_map_fold l f acc))"
+
+lemma rbt_map_fold_revinorder: "rbt_map_fold T f acc = foldr (\<lambda> (x, y) acc. f x y acc) (rev (inorder T)) acc"
+ by(induction T f acc rule: rbt_map_fold.induct) auto
+
+global_interpretation Kruskal_Graphs_Matroids: Graphs_Matroids_Encoding
+  where empty = RBT_Set.empty and update = update and delete = RBT_Map.delete and
+    lookup = lookup and adjmap_inv = "M.invar" and vset_empty = "\<langle>\<rangle>" and
+    insert = insert_rbt and vset_delete = delete_rbt and vset_inv = "rbt_inv::(('v::linorder) rbt \<Rightarrow> bool)" and
+    isin = isin and t_set = "Tree2.set_tree" and sel = rbt_sel and
+
+    set_empty = "\<langle>\<rangle>" and set_insert = insert_rbt and set_delete = delete_rbt and set_inv = "rbt_inv::(('e::linorder) rbt \<Rightarrow> bool)" and
+    set_isin = isin and to_set = "Tree2.set_tree" and union = "RBT.union" and inter = "RBT.inter" and diff = "RBT.diff" and
+    subseteq = rbt_subseteq and cardinality = size and 
+    set_of_sets_isin = "set_of_sets_isin :: ('e rbt \<Rightarrow> bool) \<Rightarrow> 'e rbt \<Rightarrow> bool" and
+
+    adjmap_fold = "rbt_map_fold" and vset_fold = "rbt_set_fold" and set_fold_adjmap = "rbt_set_fold" and
+    set_fold_vset = "rbt_set_fold"
+    for v1_of :: "('e::linorder) \<Rightarrow> ('v::linorder)" and v2_of :: "('e::linorder) \<Rightarrow> ('v::linorder)" and 
+        edge_of :: "('v::linorder) \<Rightarrow> 'v \<Rightarrow> ('e::linorder)" and c :: "('v set) \<Rightarrow> rat" and c' :: "'e \<Rightarrow> rat"
+      defines graph_to_edges = Kruskal_Graphs_Matroids.graph_to_edges
+and edges_to_graph = Kruskal_Graphs_Matroids.edges_to_graph
+and edges_to_vertices = Kruskal_Graphs_Matroids.edges_to_vertices
+  apply (subst Graphs_Matroids_Encoding_def)
+  using Pair_Graph_U_RBT.Pair_Graph_U_Specs_axioms Matroid_Specs_Inst.Matroid_Specs_axioms
+  by blast
+
+lemma map_of_dom_is:"set (map fst list) = {a. AList_Upd_Del.map_of list a \<noteq> None}"
+proof(induction list)
+  case Nil
+  then show ?case by simp
+next
+  case (Cons a list)
+  have "set (map fst (a # list)) = Set.insert (fst a) (set (map fst list))" by simp
+  also have "... = Set.insert (fst a) {a. AList_Upd_Del.map_of list a \<noteq> None}" 
+    using Cons by simp
+  also have "... =  {aa. AList_Upd_Del.map_of (a # list) aa \<noteq> None}"
+    by(cases a) auto
+  finally show ?case by simp
+qed
+
+lemma map_of_rev: "distinct (map fst xs) \<Longrightarrow> map_of (rev xs) x = map_of xs x"
+  by(induction xs)
+    (auto simp add: map_of_append map_of_dom_is[simplified] split: option.split)
+
+lemma  rbt_map_fold_correct: "M.invar G \<Longrightarrow>
+       \<exists>xs. distinct xs \<and>
+            set xs = dom (lookup G) \<and> rbt_map_fold G f S = foldr (\<lambda>x. f x (the (lookup G x))) xs S"
+proof(subst rbt_map_fold_revinorder, rule exI[of _ "map fst (rev (inorder G))"], goal_cases)
+  case 1
+  have invar_inorder:"rbt G \<and> sorted1 (Tree2.inorder G)"
+   using "1" M.invar_def by auto
+  define list where "list = Tree2.inorder G"
+  define list' where "list' = rev (inorder G)"
+  have distinct_list:"distinct (map fst (Tree2.inorder G))" 
+    using "1" M.invar_def strict_sorted_iff by blast
+  moreover have "set (map fst (Tree2.inorder G)) = dom (lookup G)"
+    using invar_inorder
+    by(subst dom_def, subst M.inorder_lookup, unfold list_def[symmetric] map_of_dom_is) simp+
+  moreover have "foldr (\<lambda>(x, y). f x y) (rev (Tree2.inorder G)) S =
+    foldr (\<lambda>x. f x (the (lookup G x))) (map fst (rev (Tree2.inorder G))) S"
+  proof-
+    have "distinct (map fst list')" 
+      by (metis distinct_list distinct_rev list'_def rev_map)
+    hence same_fold:"foldr (\<lambda>(x, y). f x y) list' S =
+    foldr (\<lambda>x. f x (the (AList_Upd_Del.map_of list' x))) (map fst list') S"
+    proof(induction list')
+      case Nil
+      then show ?case by simp
+    next
+      case (Cons a list')
+      show ?case 
+      proof(cases a)
+        case (Pair x y)
+        have distinct_fsts: "distinct (x # map fst list')" 
+          using Cons(2)[simplified Pair list.map(2) fst_conv] by fast
+        have first_f_apply:"foldr (\<lambda>a. case a of (x, y) \<Rightarrow> f x y) (a # list') S = f x y (foldr (\<lambda>(x, y). f x y) list' S)"
+          by(simp add: Pair)
+        have map_of_same:"(foldr (\<lambda>xa. f xa (the (AList_Upd_Del.map_of ((x, y) # list') xa))) (map fst list') S)
+              = (foldr (\<lambda>xa. f xa (the (AList_Upd_Del.map_of  list' xa))) (map fst list') S)"
+          apply(rule foldr_cong[OF refl refl])
+          subgoal for s t
+            using distinct_fsts[simplified distinct.simps(2)] 
+            by (subst map_of.simps, subst if_not_P)force+
+          done
+        have almost_result: "(foldr (\<lambda>(x, y). f x y) list' S) =
+                   (foldr (\<lambda>xa. f xa (the (AList_Upd_Del.map_of ((x, y) # list') xa))) (map fst list') S)"
+          using distinct_fsts[simplified distinct.simps(2)]
+          by (subst map_of_same, subst Cons(1)[symmetric])force+
+        show ?thesis
+          apply(subst  first_f_apply)
+          apply(subst Pair)+
+          apply(subst  list.map(2))
+          apply(subst foldr.simps)
+          apply(subst o_apply)
+          apply(subst map_of.simps)
+          apply(subst if_P)
+          apply simp
+          apply(subst option.sel)
+          apply(subst fst_conv)
+          by(subst almost_result[symmetric] ) force
+      qed
+    qed
+    show ?thesis
+    using invar_inorder 
+    by(simp add:  lookup_map_of map_of_rev[OF distinct_list, symmetric] list'_def[symmetric] same_fold)+  
+  qed
+ ultimately show ?case 
+   by (metis distinct_rev rev_map set_rev)
+qed
+
+lemma bst_distinct_inorder:"bst T \<Longrightarrow> distinct (inorder T)"
+  by(induction T rule: inorder.induct) fastforce+
+
+lemma rbt_set_fold_correct: "rbt_inv S \<Longrightarrow> \<exists>xs. distinct xs \<and> set xs = Tree2.set_tree S \<and> rbt_set_fold S f G = foldr f xs G"
+  apply(subst rbt_set_fold_revinorder)
+  apply(rule exI[of _ "rev (Tree2.inorder S)"])
+  using  bst_distinct_inorder[of S]
+  by (unfold set_inorder[symmetric] set_rev distinct_rev ) fastforce
+
+locale Transforms =
+fixes v1_of::"('e::linorder \<Rightarrow> 'v::linorder)" and v2_of::"'e \<Rightarrow> 'v" 
+and edge_of::"'v \<Rightarrow> 'v \<Rightarrow> 'e"
+and input_G :: "('v * ('v rbt)) rbt" 
+begin
+
+abbreviation Kruskal_G_to_E :: "(('v::linorder) \<times> ('v rbt)) rbt \<Rightarrow> 'e rbt" where
+  "Kruskal_G_to_E \<equiv> graph_to_edges edge_of"
+
+definition Kruskal_E_to_G :: "('e::linorder) rbt \<Rightarrow> ('v \<times> ('v rbt)) rbt" where
+  "Kruskal_E_to_G = edges_to_graph v1_of v2_of"
+
+definition Kruskal_E_to_V :: "('e::linorder) rbt \<Rightarrow> ('v rbt)" where
+  "Kruskal_E_to_V = edges_to_vertices v1_of v2_of"
+
+definition carrier_graph_matroid :: "('e::linorder) rbt" where
+  "carrier_graph_matroid = graph_to_edges edge_of input_G"
+
+fun indep_graph_matroid :: "('e::linorder) rbt \<Rightarrow> bool" where
+  "indep_graph_matroid E = 
+    (let
+      G = (Kruskal_E_to_G E);
+      V = (Kruskal_E_to_V E)
+    in
+      (if rbt_subseteq E carrier_graph_matroid then \<not>DFS_Cycles_state.cycle (DFS_Cycles' G V)
+      else False))"
+end
+
+global_interpretation transforms: Transforms
+  where v1_of = v1_of and v2_of = v2_of and edge_of = edge_of and input_G = input_G
+  for v1_of::"'e::linorder \<Rightarrow> 'a::linorder" and v2_of edge_of input_G
+  defines Kruskal_G_to_E = transforms.Kruskal_G_to_E
+   and Kruskal_E_to_G=transforms.Kruskal_E_to_G
+   and Kruskal_E_to_V=transforms.Kruskal_E_to_V
+   and carrier_graph_matroid=transforms.carrier_graph_matroid
+   and indep_graph_matroid=transforms.indep_graph_matroid
+  done
+
+
+
+global_interpretation Kruskal_Greedy: Best_In_Greedy
+  where set_empty = "\<langle>\<rangle>" and set_insert = insert_rbt and set_delete = delete_rbt 
+     and set_inv = "rbt_inv::(('e::linorder) rbt \<Rightarrow> bool)" and
+    set_isin = isin and to_set = "Tree2.set_tree" and union = "RBT.union" and inter = "RBT.inter" and diff = "RBT.diff" and
+    subseteq = rbt_subseteq and cardinality = size and
+    set_of_sets_isin = "set_of_sets_isin :: (('e::linorder) rbt \<Rightarrow> bool) \<Rightarrow> 'e rbt \<Rightarrow> bool" and 
+    carrier = "carrier_graph_matroid edge_of input_G" 
+and indep_set = "indep_graph_matroid v1_of v2_of edge_of input_G" and
+    sort_desc = insort_key_desc
+  for v1_of::"'e::linorder \<Rightarrow>'a::linorder" and v2_of edge_of input_G
+  (* TODO should we instantiate remaining parameters here or just outside? \<Rightarrow> probably should instantiate carrier and indep_set
+  here since they are specified in the locale, but cannot yet instantiate c and order *)
+  apply (subst Best_In_Greedy_def)
+  using Matroid_Specs_Inst.Matroid_Specs_axioms by blast
+
+abbreviation "indep'  == Kruskal_Greedy.indep' (TYPE ('a::linorder))"
+
+locale Kruskal_Proof_Matroid_Edges =
+Transforms +
+  assumes v1_never_v2:"\<And> e. v1_of (e::'e::linorder) \<noteq> v2_of e"
+and v1_of_edge_of: "x \<noteq> y \<Longrightarrow> v1_of (edge_of x y) = x \<or> v1_of (edge_of x y) = y"
+and v2_of_edge_of: "x \<noteq> y \<Longrightarrow> v2_of (edge_of x y) = x \<or> v2_of (edge_of x y) = y"
+begin
+
+interpretation Kruskal_Graphs_Matroids_Proofs: Graphs_Matroids_Encoding_Proofs
+  where empty = RBT_Set.empty and update = update and delete = RBT_Map.delete and
+    lookup = lookup and adjmap_inv = "M.invar" and vset_empty = "\<langle>\<rangle>" and
+    insert = insert_rbt and vset_delete = delete_rbt and vset_inv = "rbt_inv::(('a::linorder) rbt \<Rightarrow> bool)" and
+    isin = isin and t_set = "Tree2.set_tree" and sel = rbt_sel and
+
+    set_empty = "\<langle>\<rangle>" and set_insert = insert_rbt and set_delete = delete_rbt and set_inv = "rbt_inv::(('e::linorder) rbt \<Rightarrow> bool)" and
+    set_isin = isin and to_set = "Tree2.set_tree" and union = "RBT.union" and inter = "RBT.inter" and diff = "RBT.diff" and
+    subseteq = rbt_subseteq and cardinality = size and 
+    set_of_sets_isin = "set_of_sets_isin :: ('e rbt \<Rightarrow> bool) \<Rightarrow> 'e rbt \<Rightarrow> bool" and
+
+    adjmap_fold = "rbt_map_fold" and vset_fold = "rbt_set_fold" and set_fold_adjmap = "rbt_set_fold" and
+    set_fold_vset = "rbt_set_fold"
+  for c :: "('a set) \<Rightarrow> rat" and c' :: "'e \<Rightarrow> rat"
+ proof(rule Graphs_Matroids_Encoding_Proofs.intro, 
+     rule Kruskal_Graphs_Matroids.Graphs_Matroids_Encoding_axioms, 
+     rule Graphs_Matroids_Encoding_Proofs_axioms.intro, goal_cases)
+  case (1 G S f)
+  then show ?case by(auto intro:  rbt_map_fold_correct)
+next
+  case (2 G S f)
+  show ?case 
+  by(insert 2, rule rbt_set_fold_correct[of S f G]) fast
+next
+  case (3 V f S)
+  show ?case by(insert 3, rule rbt_set_fold_correct) fast
+next
+  case 5
+  then show ?case  by(auto intro: finite_set_tree simp add: Pair_Graph_Specs.finite_vsets_def[OF Pair_Graph_U_RBT.Pair_Graph_Specs_axioms])
+next
+  case (4 V f S)
+  show ?case  by(insert 4, rule rbt_set_fold_correct) fast
+next
+  case (6 e)
+  thus ?case 
+    by (simp add: v1_never_v2)
+next
+  case (7 x y)
+  thus ?case 
+    using v1_of_edge_of by blast
+next
+  case (8 x y)
+  thus ?case
+    using v2_of_edge_of by presburger
+qed
+
+term Kruskal_Graphs_Matroids.graph_to_edges
+
+definition "cost_nonnegative (c::(('v set) \<Rightarrow> rat)) = ( \<forall>e. c e \<ge> 0)"
+
+term Kruskal_Graphs_Matroids.graph_to_edges
+term Kruskal_Graphs_Matroids.edges_to_graph
+
+
+context
+    fixes c :: "('a set) \<Rightarrow> rat" and c' :: "'e \<Rightarrow> rat"
+begin
+
+
+lemma (* TODO instantiate assms directly using thms from encoding locale, maybe take the statement "further"*)
+  indep_graph_matroid_expr_1:
+  assumes "Pair_Graph_U_RBT.pair_graph_u_invar (Kruskal_E_to_G  (E::('e::linorder) rbt))" 
+          "rbt_inv (Kruskal_E_to_V   E)"
+    "Tree2.set_tree (Kruskal_E_to_V   E) =
+            dVs (Pair_Graph_U_RBT.digraph_abs (Kruskal_E_to_G   E))"
+  shows "indep_graph_matroid  E =
+    (rbt_subseteq E (carrier_graph_matroid ) \<and>
+ \<not>(\<exists>u c. decycle (Pair_Graph_U_RBT.ugraph_abs (Kruskal_E_to_G  E)) u c))"
+  apply (subst indep_graph_matroid.simps)
+  apply (subst Let_def)+
+  apply (subst DFS_Cycles_correct_final[OF assms]) by presburger
+
+lemma
+  indep_graph_matroid_expr_2:
+  assumes "rbt_inv (E::('e::linorder) rbt)"
+  shows "indep_graph_matroid  E =
+    (rbt_subseteq E (carrier_graph_matroid ) \<and> 
+\<not>(\<exists>u c. decycle (Pair_Graph_U_RBT.ugraph_abs (Kruskal_E_to_G E)) u c))"
+  using indep_graph_matroid_expr_1[of "E", unfolded Kruskal_E_to_G_def Kruskal_E_to_V_def]
+    Kruskal_Graphs_Matroids_Proofs.edges_invar_imp_graph_invar[OF assms]
+    Kruskal_Graphs_Matroids_Proofs.edges_invar_imp_vertices_props[OF assms]
+  by(unfold Kruskal_E_to_G_def  edges_to_graph_def edges_to_vertices_def) blast
+  
+
+term Kruskal_Greedy.valid_solution 
+term Kruskal_Greedy.nonnegative 
+term Kruskal_Greedy.valid_order
+
+thm Kruskal_Greedy.BestInGreedy_correct_1
+thm Kruskal_Greedy.BestInGreedy_correct_3
+thm Kruskal_Greedy.BestInGreedy_matroid_iff_opt
+
+
+
+term Matroid_Specs_Inst.indep
+term indep_graph_matroid
+
+lemma carrier_graph_matroid_inv:
+  assumes "Pair_Graph_U_RBT.pair_graph_u_invar input_G"
+  shows "rbt_inv  (carrier_graph_matroid)"
+  using Kruskal_Graphs_Matroids_Proofs.graph_invar_imp_edges_invar[OF assms] 
+  by(unfold carrier_graph_matroid_def graph_to_edges_def)
+
+lemma Kruskal_Greedy_indep':
+  "Kruskal_Greedy.indep'  v1_of v2_of edge_of input_G (X::('e \<times> color) tree) =
+ indep_graph_matroid X"
+  using Matroid_Specs_Inst.indep_def set_of_sets_isin_def
+  by (metis indep_graph_matroid_def)
+
+lemma indep_graph_matroid_abs_equal:
+  assumes "Pair_Graph_U_RBT.pair_graph_u_invar input_G" "rbt_inv X" "rbt_inv Y" "Tree2.set_tree X = Tree2.set_tree Y"
+  shows "indep_graph_matroid  X
+           = indep_graph_matroid  Y"
+proof-
+  have "rbt_subseteq X (carrier_graph_matroid) =
+        rbt_subseteq Y (carrier_graph_matroid )"
+    using rbt_subseteq_correct[OF \<open>rbt_inv X\<close> carrier_graph_matroid_inv[OF assms(1)]]
+    rbt_subseteq_correct[OF \<open>rbt_inv Y\<close> carrier_graph_matroid_inv[OF assms(1)]] assms(4)
+    by blast
+  with Kruskal_Graphs_Matroids_Proofs.to_set_equal_imp_ugraph_abs_equal[OF assms(2-4)]
+  show "indep_graph_matroid  X =
+        indep_graph_matroid  Y"
+    apply (subst indep_graph_matroid_expr_2[OF \<open>rbt_inv X\<close>])
+    apply (subst indep_graph_matroid_expr_2[OF \<open>rbt_inv Y\<close>])
+    unfolding Kruskal_E_to_G_def edges_to_graph_def using arg_cong2 .
+qed
+lemma Kruskal_BestInGreedy_axioms:
+  assumes "Pair_Graph_U_RBT.pair_graph_u_invar input_G"
+  shows "Best_In_Greedy.BestInGreedy_axioms rbt_inv Tree2.set_tree set_of_sets_isin 
+  (carrier_graph_matroid) (indep_graph_matroid )"
+  unfolding Kruskal_Greedy.BestInGreedy_axioms_def Matroid_Specs_Inst.invar_def
+    Matroid_Specs_Inst.finite_sets_def
+proof-
+  from carrier_graph_matroid_def Kruskal_Graphs_Matroids_Proofs.graph_invar_imp_edges_invar[OF assms]
+    have "rbt_inv  (carrier_graph_matroid )" 
+      using assms carrier_graph_matroid_inv by blast
+  with indep_graph_matroid_abs_equal[OF assms] Kruskal_Greedy_indep' finite_set_tree
+  have "(rbt_inv  (carrier_graph_matroid ) \<and>
+    (\<forall>X Y. rbt_inv X \<longrightarrow> rbt_inv Y \<longrightarrow> Tree2.set_tree X = Tree2.set_tree Y \<longrightarrow>
+      indep'  v1_of v2_of edge_of input_G X =
+      indep'  v1_of v2_of edge_of input_G Y)) \<and>
+    (\<forall>X. finite (Tree2.set_tree X))" by blast
+  thus ?thesis 
+    by (metis (mono_tags, lifting) Best_In_Greedy.BestInGreedy_axioms_def Kruskal_Greedy.Best_In_Greedy_axioms Matroid_Specs_Inst.finite_sets_def Matroid_Specs_Inst.invar_def indep_graph_matroid_def)
+qed
+
+
+lemma Kruskal_sort_desc_axioms:
+  "Best_In_Greedy.sort_desc_axioms Kruskal_Greedy.carrier_sorted"
+  unfolding Kruskal_Greedy.sort_desc_axioms_def
+  using set_insort_key_desc length_insort_key_desc sorted_desc_f_insort_key_desc insort_key_desc_stable
+  by metis
+
+
+context
+  assumes pair_graph_u: "Pair_Graph_U_RBT.pair_graph_u_invar input_G"
+begin
+
+lemmas carrier_inv = carrier_graph_matroid_inv[OF pair_graph_u]
+
+(*
+interpretation input_G_graph_abs: graph_abs
+  where G = "Pair_Graph_U_RBT.ugraph_abs input_G"
+  using Pair_Graph_U_RBT.graph_abs_ugraph[OF pair_graph_u] by simp
+
+interpretation (Pair_Graph_U_RBT.ugraph_abs (Kruskal_E_to_G carrier_graph_matroid))
+*)
+(*
+lemma carrier_converted_back:
+  "Kruskal_E_to_G carrier_graph_matroid = input_G"
+  unfolding Kruskal_E_to_G_def carrier_graph_matroid_def 
+  using Kruskal_Graphs_Matroids_Proofs.graph_to_edges_inverse[OF pair_graph_u] by simp
+*)
+
+lemma carrier_converted_graph_abs:
+  "graph_abs (Pair_Graph_U_RBT.ugraph_abs 
+(Kruskal_E_to_G  ( carrier_graph_matroid )))"
+  using (*carrier_converted_back*) Pair_Graph_U_RBT.graph_abs_ugraph[OF pair_graph_u]
+  sorry
+(* Put this into interpretation or not? *)
+
+lemma indep_graph_matroid_expr_3:
+  assumes "rbt_inv (E::('e::linorder) rbt)"
+  shows "indep_graph_matroid  E = 
+    graph_abs.has_no_cycle (Pair_Graph_U_RBT.ugraph_abs 
+(Kruskal_E_to_G  (carrier_graph_matroid)))
+    (Pair_Graph_U_RBT.ugraph_abs (Kruskal_E_to_G  E))"
+  unfolding graph_abs.has_no_cycle_def[OF carrier_converted_graph_abs]
+  (* (rbt_subseteq E carrier_graph_matroid \<and> \<not>(\<exists>u c. decycle (Pair_Graph_U_RBT.ugraph_abs (Kruskal_E_to_G E)) u c)) *)
+proof-
+  from indep_graph_matroid_expr_2[OF assms]
+  have "indep_graph_matroid  E =
+    (rbt_subseteq E (carrier_graph_matroid ) \<and>
+    (\<nexists>u c. decycle (Pair_Graph_U_RBT.ugraph_abs (Kruskal_E_to_G  E)) u c))" by blast
+  also have "... = 
+    (Pair_Graph_U_RBT.ugraph_abs (Kruskal_E_to_G  E) \<subseteq>
+ Pair_Graph_U_RBT.ugraph_abs (Kruskal_E_to_G  (carrier_graph_matroid )) \<and>
+    (\<nexists>u c. decycle (Pair_Graph_U_RBT.ugraph_abs (Kruskal_E_to_G  E)) u c))"
+    unfolding Kruskal_E_to_G_def
+    using Kruskal_Graphs_Matroids_Proofs.subset_iff_graph_to_edges_subset[OF assms carrier_inv]
+    sorry
+  finally show "indep_graph_matroid  E =
+    (Pair_Graph_U_RBT.ugraph_abs (Kruskal_E_to_G  E) \<subseteq>
+ Pair_Graph_U_RBT.ugraph_abs (Kruskal_E_to_G (carrier_graph_matroid )) \<and>
+     (\<nexists>u c. decycle (Pair_Graph_U_RBT.ugraph_abs (Kruskal_E_to_G  E)) u c))" .
+qed
+
+
+(* TODO maybe generalise some parts of these theorems? *)
+term indep'
+lemma Kruskal_indep'_eq_has_no_cycle:
+  assumes "rbt_inv (X::('e::linorder) rbt)"
+  shows "indep' v1_of v2_of edge_of input_G X = graph_abs.has_no_cycle 
+(Pair_Graph_U_RBT.ugraph_abs (Kruskal_E_to_G  (carrier_graph_matroid )))
+    (Pair_Graph_U_RBT.ugraph_abs (Kruskal_E_to_G  X))"
+  using Kruskal_Greedy_indep' indep_graph_matroid_expr_3[OF assms] by blast
+
+lemma Kruskal_indep_subset_carrier:
+  assumes "rbt_inv (X::('e::linorder) rbt)" "indep' v1_of v2_of edge_of input_G X"
+  shows "rbt_subseteq X (carrier_graph_matroid )"
+proof-
+  from assms(2) Kruskal_Greedy_indep' indep_graph_matroid_expr_3[OF assms(1)]
+  have "graph_abs.has_no_cycle (Pair_Graph_U_RBT.ugraph_abs 
+(Kruskal_E_to_G (carrier_graph_matroid )))
+    (Pair_Graph_U_RBT.ugraph_abs (Kruskal_E_to_G  X))" by blast
+  then have "Pair_Graph_U_RBT.ugraph_abs (Kruskal_E_to_G  X) \<subseteq>
+    Pair_Graph_U_RBT.ugraph_abs (Kruskal_E_to_G  (carrier_graph_matroid ))"
+    using graph_abs.has_no_cycle_indep_subset_carrier[OF carrier_converted_graph_abs] by blast
+  then have "Tree2.set_tree X \<subseteq> Tree2.set_tree ((carrier_graph_matroid ))"
+    unfolding Kruskal_E_to_G_def
+    using Kruskal_Graphs_Matroids_Proofs.edges_to_graph_subset_imp_subset[OF \<open>rbt_inv X\<close> carrier_inv]
+    sorry
+  with Custom_Set_RBT.set_subseteq[OF \<open>rbt_inv X\<close> carrier_inv]
+    show "rbt_subseteq X (carrier_graph_matroid )" by blast
+qed
+
+lemma Kruskal_indep_ex:
+  "(\<exists>X. rbt_inv (X::('e::linorder) rbt) \<and> indep' v1_of v2_of edge_of input_G X)"
+proof-
+  from graph_abs.has_no_cycle_indep_ex[OF carrier_converted_graph_abs]
+  obtain G where "graph_abs.has_no_cycle (Pair_Graph_U_RBT.ugraph_abs 
+(Kruskal_E_to_G  (carrier_graph_matroid ))) G"
+    by blast
+  from graph_abs.has_no_cycle_indep_subset_carrier[OF carrier_converted_graph_abs this]
+    have "G \<subseteq> (Pair_Graph_U_RBT.ugraph_abs (Kruskal_E_to_G  (carrier_graph_matroid )))"
+      sorry
+  from graph_abs_mono[OF carrier_converted_graph_abs this]
+    have "graph_abs G" by blast
+    obtain G_impl where G_impl_invar: "Pair_Graph_U_RBT.pair_graph_u_invar G_impl" and
+      G_impl_abs: "Pair_Graph_U_RBT.ugraph_abs G_impl = G"
+      sorry
+
+  (* If G satisfies ugraph_abs, there exists an impl graph satisfying pair_graph_u such that ugraph_abs (G_impl) = *)
+
+  from Kruskal_Graphs_Matroids_Proofs.graph_invar_imp_edges_invar[OF \<open>Pair_Graph_U_RBT.pair_graph_u_invar G_impl\<close>]
+    have "rbt_inv (Kruskal_Graphs_Matroids.graph_to_edges edge_of G_impl)" sorry
+
+
+  from \<open>graph_abs.has_no_cycle (Pair_Graph_U_RBT.ugraph_abs (Kruskal_E_to_G (carrier_graph_matroid ))) G\<close> G_impl_abs
+    have "graph_abs.has_no_cycle (Pair_Graph_U_RBT.ugraph_abs (Kruskal_E_to_G (carrier_graph_matroid )))
+      (Pair_Graph_U_RBT.ugraph_abs (Kruskal_E_to_G (Kruskal_Graphs_Matroids.graph_to_edges edge_of G_impl)))"
+    unfolding Kruskal_E_to_G_def sorry
+   (* apply (subst Kruskal_Graphs_Matroids_Proofs.graph_to_edges_inverse[OF G_impl_invar])
+    by (metis Kruskal_E_to_G_def carrier_converted_back)*)
+
+  with Kruskal_Greedy_indep' indep_graph_matroid_expr_3[OF \<open>rbt_inv (Kruskal_Graphs_Matroids.graph_to_edges edge_of G_impl)\<close>]
+    (* \<open>graph_abs.has_no_cycle (Pair_Graph_U_RBT.ugraph_abs (Kruskal_E_to_G carrier_graph_matroid)) G\<close>
+    \<open>Pair_Graph_U_RBT.ugraph_abs G_impl = G\<close>
+    Kruskal_Graphs_Matroids.graph_to_edges_inverse[OF G_impl_invar] *)
+    have "Kruskal_Greedy.indep' v1_of v2_of edge_of input_G (Kruskal_Graphs_Matroids.graph_to_edges edge_of G_impl)" by blast
+  with \<open>rbt_inv (Kruskal_Graphs_Matroids.graph_to_edges edge_of G_impl)\<close>
+    show ?thesis by blast
+qed
+
+
+lemma Kruskal_indep_subset:
+  assumes "rbt_inv X" "rbt_inv Y" "indep' v1_of v2_of edge_of input_G X" "rbt_subseteq Y X"
+  shows "indep' v1_of v2_of edge_of input_G Y"
+proof-
+  from Kruskal_indep'_eq_has_no_cycle[OF assms(1)] assms(3)
+  have no_cycle: "graph_abs.has_no_cycle
+ (Pair_Graph_U_RBT.ugraph_abs (Kruskal_E_to_G (carrier_graph_matroid)))
+      (Pair_Graph_U_RBT.ugraph_abs (Kruskal_E_to_G X))" by blast
+  have X_subset_Y: "Pair_Graph_U_RBT.ugraph_abs (Kruskal_E_to_G Y) \<subseteq>
+    Pair_Graph_U_RBT.ugraph_abs (Kruskal_E_to_G X)"
+   (* using Kruskal_Graphs_Matroids_Proofs.subset_iff_graph_to_edges_subset[OF assms(2,1), of v1_of v2_of]
+    assms(4) by(force simp add: Kruskal_E_to_G_def) *) sorry
+  from graph_abs.has_no_cycle_indep_subset[OF carrier_converted_graph_abs no_cycle X_subset_Y]
+  have "graph_abs.has_no_cycle (Pair_Graph_U_RBT.ugraph_abs
+ (Kruskal_E_to_G  (carrier_graph_matroid)))
+      (Pair_Graph_U_RBT.ugraph_abs (Kruskal_E_to_G Y))" by blast
+  with Kruskal_indep'_eq_has_no_cycle[OF \<open>rbt_inv Y\<close>]
+    show ?thesis by blast
+qed
+
+lemma Kruskal_augment:
+  assumes "rbt_inv X" "rbt_inv Y" "indep' v1_of v2_of edge_of input_G X" 
+"indep' v1_of v2_of edge_of input_G Y" "size X = Suc (size Y)"
+shows "(\<exists>x. Pair_Graph_U_RBT.isin' x (RBT.diff X Y) \<and>
+ indep' v1_of v2_of edge_of input_G (insert_rbt x Y))"
+proof-
+  from Kruskal_indep'_eq_has_no_cycle[OF assms(1)] assms(3)
+  have no_cycle_X: "graph_abs.has_no_cycle (Pair_Graph_U_RBT.ugraph_abs
+ (Kruskal_E_to_G  (carrier_graph_matroid )))
+      (Pair_Graph_U_RBT.ugraph_abs (Kruskal_E_to_G X))" by blast
+  from Kruskal_indep'_eq_has_no_cycle[OF assms(2)] assms(4)
+  have no_cycle_Y: "graph_abs.has_no_cycle (Pair_Graph_U_RBT.ugraph_abs
+ (Kruskal_E_to_G  (carrier_graph_matroid )))
+      (Pair_Graph_U_RBT.ugraph_abs (Kruskal_E_to_G  Y))" by blast
+
+  from Kruskal_Graphs_Matroids_Proofs.card_graph_to_edges[OF \<open>rbt_inv X\<close>]
+     Kruskal_Graphs_Matroids_Proofs.card_graph_to_edges[OF \<open>rbt_inv Y\<close>] assms(5)
+
+  have card_rel: "card (Pair_Graph_U_RBT.ugraph_abs (Kruskal_E_to_G  X)) 
+= Suc (card (Pair_Graph_U_RBT.ugraph_abs (Kruskal_E_to_G  Y))) "
+    unfolding Kruskal_E_to_G_def sorry
+
+  from graph_abs.has_no_cycle_augment[OF carrier_converted_graph_abs no_cycle_X no_cycle_Y card_rel]
+  obtain x where "x \<in> Pair_Graph_U_RBT.ugraph_abs (Kruskal_E_to_G X) 
+- Pair_Graph_U_RBT.ugraph_abs (Kruskal_E_to_G  Y)"
+      "graph_abs.has_no_cycle (Pair_Graph_U_RBT.ugraph_abs (Kruskal_E_to_G  
+(carrier_graph_matroid )))
+       (Set.insert x (Pair_Graph_U_RBT.ugraph_abs (Kruskal_E_to_G  Y)))" by blast
+find_theorems Pair_Graph_U_RBT.ugraph_abs Kruskal_E_to_G
+   (* TODO HERE !! *)
+  show ?thesis
+    apply(subst Kruskal_indep'_eq_has_no_cycle) sorry
+qed
+
+
+lemma Kruskal_indep_system_axioms:
+  "Matroid_Specs_Inst.indep_system_axioms (carrier_graph_matroid ) 
+(indep_graph_matroid)"
+  apply (subst Matroid_Specs_Inst.indep_system_axioms_def)
+  using Kruskal_indep_subset_carrier Kruskal_indep_ex Kruskal_indep_subset
+  by (smt (verit) indep_graph_matroid_def)
+
+lemma Kruskal_matroid_axioms:
+  "Matroid_Specs_Inst.matroid_axioms (carrier_graph_matroid )
+ (indep_graph_matroid )"
+  apply (subst Matroid_Specs_Inst.matroid_axioms_def)
+  using Kruskal_indep_system_axioms Kruskal_augment
+  by (metis (no_types, lifting) indep_graph_matroid_def)
+
+end
+
+
+(* thm Kruskal_Greedy.BestInGreedy_correct_1[OF Kruskal_BestInGreedy_axioms] *)
+(*thm Kruskal_Greedy.BestInGreedy_correct_1[OF Kruskal_BestInGreedy_axioms Kruskal_sort_desc_axioms Kruskal_indep_system_axioms]
+*)
+(* TODO NOW INSTANTIATE INDEP SYSTEM AXIOMS, CONNECT FINAL THEOREM 
+\<Rightarrow> assumptions on c and order can be left as-is for now *)
+
+
+
+(* !! TODO here assumption !! *)
+(*
+interpretation G_edges_abs: graph_abs
+  where G = "Pair_Graph_U_RBT.ugraph_abs input_G"
+  using Pair_Graph_U_RBT.graph_abs_ugraph[OF pair_graph_u] by simp
+*)
+
+term Kruskal_Greedy.initial_state 
+
+(* TODO define Kruskal_MST, maybe should parametrise with graph and define outside of context? \<Rightarrow> or parametrise
+with c and order? \<Longrightarrow> Don't need to put this function in context, only use use context when pair graph property
+is actually necessary
+\<Rightarrow> maybe parametrise with c and order? *)
+(*
+fun Kruskal_MST :: "(('v::linorder) * ('v rbt)) rbt" where
+  "Kruskal_MST = Kruskal_E_to_G (best_in_greedy_state.result (Kruskal_Greedy.BestInGreedy (Kruskal_Greedy.initial_state c order)))"
+*)
+find_theorems "_::_ itself"
+
+abbreviation "BestInGreedy == Kruskal_Greedy.BestInGreedy "
+
+fun Kruskal_MST :: "('e::linorder list) \<Rightarrow> (('a::linorder) * ('a rbt)) rbt" where
+  "Kruskal_MST order =
+    Kruskal_E_to_G  (
+best_in_greedy_state.result
+ (Kruskal_Greedy.BestInGreedy (TYPE ('a)) v1_of v2_of edge_of input_G  
+(Kruskal_Greedy.initial_state c' order)))"
+
+context
+  assumes pair_graph_u: "Pair_Graph_U_RBT.pair_graph_u_invar input_G"
+begin
+
+interpretation G_edges_abs: graph_abs
+  where G = "Pair_Graph_U_RBT.ugraph_abs input_G"
+  using Pair_Graph_U_RBT.graph_abs_ugraph[OF pair_graph_u] by simp
+
+(* thm spanning_tree_def *)
+thm G_edges_abs.is_spanning_forest_def
+(*
+thm Kruskal_Greedy.BestInGreedy_correct_3[OF Kruskal_BestInGreedy_axioms[OF pair_graph_u]
+    Kruskal_sort_desc_axioms Kruskal_indep_system_axioms[OF pair_graph_u]]
+*)
+lemma Kruskal_Greedy_valid_inst:
+  assumes "Kruskal_Greedy.nonnegative (TYPE ('a)) edge_of inut_G c'" 
+"Kruskal_Greedy.valid_order (TYPE ('a)) edge_of input_G order"
+shows "Kruskal_Greedy.valid_solution (TYPE ('a)) edge_of input_G v1_of v2_of
+ (result (Kruskal_Greedy.BestInGreedy (TYPE ('a)) v1_of v2_of edge_of input_G
+ (Kruskal_Greedy.initial_state c' order)))"
+(*proof-
+  from Kruskal_Greedy.BestInGreedy_correct_1[OF Kruskal_BestInGreedy_axioms[OF pair_graph_u]
+    Kruskal_sort_desc_axioms Kruskal_indep_system_axioms[OF pair_graph_u], OF assms]
+  show ?thesis by metis
+qed*) sorry
+
+lemma Kruskal_Greedy_opt_inst:
+  assumes "Kruskal_Greedy.nonnegative (TYPE ('a)) edge_of input_G c'" 
+"Kruskal_Greedy.valid_order (TYPE ('a)) edge_of input_G order"
+ "Kruskal_Greedy.valid_solution (TYPE ('a)) edge_of input_G v1_of v2_of X"
+  shows "sum c' (Tree2.set_tree X) \<le> sum c'
+           (Tree2.set_tree (result (Kruskal_Greedy.BestInGreedy (TYPE ('a))
+           v1_of v2_of edge_of input_G (Kruskal_Greedy.initial_state c' order))))"
+proof-
+ (* from Kruskal_Greedy.BestInGreedy_matroid_iff_opt[OF Kruskal_BestInGreedy_axioms[OF pair_graph_u]
+    Kruskal_sort_desc_axioms Kruskal_indep_system_axioms[OF pair_graph_u]]
+    Kruskal_matroid_axioms[OF pair_graph_u]
+    assms Kruskal_Greedy.c_set_def*)
+  have "Kruskal_Greedy.c_set c' (Tree2.set_tree X) \<le>
+    Kruskal_Greedy.c_set c' (Tree2.set_tree (result
+ (Kruskal_Greedy.BestInGreedy  (TYPE ('a))
+           v1_of v2_of edge_of input_G (Kruskal_Greedy.initial_state c' order))))"
+    sorry
+  with Kruskal_Greedy.c_set_def show ?thesis by metis
+qed
+
+
+
+lemma nonneg_conv:
+  "cost_nonnegative c \<Longrightarrow> Kruskal_Greedy.nonnegative (TYPE ('a)) edge_of input_G c'"
+  sorry
+
+
+lemma Kruskal_correct_final_1:
+  assumes "cost_nonnegative c" "Kruskal_Greedy.valid_order (TYPE ('a)) 
+edge_of input_G order" (* WRONG ASSUMPTIONS !! *)
+  shows "G_edges_abs.is_spanning_forest (Pair_Graph_U_RBT.ugraph_abs (Kruskal_MST order))"
+  sorry
+ 
+
+thm Kruskal_matroid_axioms[OF pair_graph_u]
+(*thm Kruskal_Greedy.BestInGreedy_matroid_iff_opt[OF Kruskal_BestInGreedy_axioms[OF pair_graph_u]
+    Kruskal_sort_desc_axioms Kruskal_indep_system_axioms[OF pair_graph_u]]
+*)
+term "(Pair_Graph_U_RBT.ugraph_abs (Kruskal_MST order))"
+lemma Kruskal_correct_final_2:
+  assumes "cost_nonnegative c" "Kruskal_Greedy.valid_order (TYPE ('a)) edge_of input_G order" (* WRONG ASSUMPTIONS !! *)
+    (* introduce new nonnegative predicate, maybe find some way to get order based on existing stuff or assume 
+    function*)
+    "Pair_Graph_U_RBT.pair_graph_u_invar G'"
+    "Pair_Graph_U_RBT.ugraph_abs G' \<subseteq> Pair_Graph_U_RBT.ugraph_abs input_G"
+    "G_edges_abs.is_spanning_forest (Pair_Graph_U_RBT.ugraph_abs G')"
+  (* shows "sum c (Pair_Graph_U_RBT.ugraph_abs (Kruskal_MST c order)) \<le> sum c (Pair_Graph_U_RBT.ugraph_abs G')"  *)
+  shows "sum c (Pair_Graph_U_RBT.ugraph_abs (Kruskal_MST order)) \<le>
+ sum c (Pair_Graph_U_RBT.ugraph_abs G')"
+proof-
+  from \<open>G_edges_abs.is_spanning_forest (Pair_Graph_U_RBT.ugraph_abs G')\<close>
+    have "graph_abs.has_no_cycle (Pair_Graph_U_RBT.ugraph_abs input_G) (Pair_Graph_U_RBT.ugraph_abs G')"
+    unfolding G_edges_abs.is_spanning_forest_def by blast
+
+  thm indep_graph_matroid_expr_3[OF pair_graph_u]
+
+ (* thm Kruskal_Greedy.BestInGreedy_matroid_iff_opt[OF Kruskal_BestInGreedy_axioms Kruskal_sort_desc_axioms
+      Kruskal_indep_system_axioms] pair_graph_u
+*)
+  have valid_soln: "Kruskal_Greedy.valid_solution (TYPE ('a)) edge_of input_G v1_of v2_of 
+          (Kruskal_G_to_E G')" sorry
+  from Kruskal_Greedy_opt_inst[OF nonneg_conv[OF assms(1)] assms(2) valid_soln]
+  have "sum c' (Tree2.set_tree (Kruskal_G_to_E G'))
+    \<le> sum c' (Tree2.set_tree (result (Kruskal_Greedy.BestInGreedy (TYPE ('a)) v1_of v2_of edge_of input_G 
+(Kruskal_Greedy.initial_state c' order))))"
+    by blast
+  then have
+      "sum c (Pair_Graph_U_RBT.ugraph_abs (Kruskal_E_to_G  (Kruskal_G_to_E G')))
+    \<ge> sum c (Pair_Graph_U_RBT.ugraph_abs (Kruskal_E_to_G 
+ (result (Kruskal_Greedy.BestInGreedy (TYPE ('a)) v1_of v2_of edge_of input_G (Kruskal_Greedy.initial_state c' order)))))"
+   (*   using Kruskal_Graphs_Matroids_Proofs.costs_transformation[where E' ="(Kruskal_G_to_E G')" and
+          E'' = "(result (Kruskal_Greedy.BestInGreedy (Kruskal_Greedy.initial_state c' order)))"]
+    by blast*) sorry
+  then
+    show "sum c (Pair_Graph_U_RBT.ugraph_abs (Kruskal_MST order)) \<le> sum c (Pair_Graph_U_RBT.ugraph_abs G')"
+    using Kruskal_Graphs_Matroids_Proofs.graph_to_edges_inverse[OF \<open>Pair_Graph_U_RBT.pair_graph_u_invar G'\<close>]
+    using Kruskal_E_to_G_def sorry
+qed
+  
+
+
+end
+
+end
+end
+(* Example: Edge is implemented as pair of vertices where first element is always less than or equal
+to second element *)
+definition edge_of :: "('v::linorder) \<Rightarrow> 'v \<Rightarrow> ('v \<times> 'v)" where
+  "edge_of u v = (if u \<le> v then (u, v) else (v, u))"
+
+definition v1_of :: "('v \<times> 'v) \<Rightarrow> ('v::linorder)" where
+  "v1_of e = fst e"
+
+definition v2_of :: "('v \<times> 'v) \<Rightarrow> ('v::linorder)" where
+  "v2_of e = snd e"
+(*
+definition "Kruskal_MST' input_G c' order = Kruskal_MST input_G v1_of v2_of edge_of c' order"
+*)
+(*
+definition c where "c e = 0"
+
+definition order where "order = []"
+
+value "Kruskal_MST' (Leaf::((nat \<times> nat rbt) rbt)) c order"
+*)
+
+
+end
